sep files, almost sem eq

aarch64/Asm.v
@@ -73,7 +73,7 @@ Inductive preg: Type :=
   | FR: freg -> preg   (**r double- or single-precision float registers *)
   | CR: crbit -> preg  (**r bits in the condition register *)
   | SP: preg           (**r register X31 used as stack pointer *)
-  | PC: preg.        (**r program counter *)
+  | PC: preg.          (**r program counter *)
 
 Coercion IR: ireg >-> preg.
 Coercion FR: freg >-> preg.
@@ -90,10 +90,7 @@ End PregEq.
 Module Pregmap := EMap(PregEq).
 
 Definition preg_of_iregsp (r: iregsp) : preg :=
-  match r with 
-  | RR1 r => IR r 
-  | XSP => SP 
-  end.
+  match r with RR1 r => IR r | XSP => SP end.
 
 Coercion preg_of_iregsp: iregsp >-> preg.
 
@@ -308,7 +305,6 @@ Inductive instruction: Type :=
   | Pnop                                                              (**r no operation *)
   | Pcfi_adjust (ofs: int)                                            (**r .cfi_adjust debug directive *)
   | Pcfi_rel_offset (ofs: int)                                        (**r .cfi_rel_offset debug directive *)
-  | Pincpc (** my own thing, represents incrementing PC*)
 .
 
 Definition code := list instruction.
@@ -337,10 +333,10 @@ Definition ir0x (rs: regset) (r: ireg0) : val :=
 
 (** Concise notations for accessing and updating the values of registers. *)
 
-Notation "a # b" := (a b) (at level 1, only parsing) : asm.
-Notation "a # b <- c" := (Pregmap.set b c a) (at level 1, b at next level) : asm.
-Notation "a ## b" := (ir0w a b) (at level 1, only parsing) : asm.
-Notation "a ### b" := (ir0x a b) (at level 1, only parsing) : asm.
+Notation "a # b" := (a b) (at level 1, only parsing).
+Notation "a # b <- c" := (Pregmap.set b c a) (at level 1, b at next level).
+Notation "a ## b" := (ir0w a b) (at level 1, only parsing).
+Notation "a ### b" := (ir0x a b) (at level 1, only parsing).
 
 Open Scope asm.
 
@@ -440,8 +436,8 @@ Inductive outcome: Type :=
 (** Manipulations over the [PC] register: continuing with the next
   instruction ([nextinstr]) or branching to a label ([goto_label]). *)
 
-Definition nextinstr (rs: regset) := rs.
-  (* rs#PC <- (Val.offset_ptr rs#PC Ptrofs.one). *)
+Definition nextinstr (rs: regset) :=
+  rs#PC <- (Val.offset_ptr rs#PC Ptrofs.one).
 
 Definition goto_label (f: function) (lbl: label) (rs: regset) (m: mem) :=
   match label_pos lbl 0 (fn_code f) with
@@ -690,450 +686,445 @@ Definition float64_of_bits (v: val): val :=
     survive the execution of the pseudo-instruction.
 *)
 
-Definition exec_instr (f: function) (i: instruction) (o: outcome) : outcome :=
-  match o with 
-    | Stuck => Stuck
-    | Next rs m =>
-    match i with
-    (** Branches *)
-    | Pb lbl =>
-        goto_label f lbl rs m
-    | Pbc cond lbl =>
+Definition exec_instr (f: function) (i: instruction) (rs: regset) (m: mem) : outcome :=
+  match i with
+  (** Branches *)
+  | Pb lbl =>
+      goto_label f lbl rs m
+  | Pbc cond lbl =>
+      match eval_testcond cond rs with
+      | Some true => goto_label f lbl rs m
+      | Some false => Next (nextinstr rs) m
+      | None => Stuck
+      end
+  | Pbl id sg =>
+      Next (rs#RA <- (Val.offset_ptr rs#PC Ptrofs.one) #PC <- (Genv.symbol_address ge id Ptrofs.zero)) m
+  | Pbs id sg =>
+      Next (rs#PC <- (Genv.symbol_address ge id Ptrofs.zero)) m
+  | Pblr r sg =>
+      Next (rs#RA <- (Val.offset_ptr rs#PC Ptrofs.one) #PC <- (rs#r)) m
+  | Pbr r sg =>
+      Next (rs#PC <- (rs#r)) m
+  | Pret r =>
+      Next (rs#PC <- (rs#r)) m
+  | Pcbnz sz r lbl =>
+      match eval_testzero sz rs#r m with
+      | Some true => Next (nextinstr rs) m
+      | Some false => goto_label f lbl rs m
+      | None => Stuck
+      end
+  | Pcbz sz r lbl =>
+      match eval_testzero sz rs#r m with
+      | Some true => goto_label f lbl rs m
+      | Some false => Next (nextinstr rs) m
+      | None => Stuck
+      end
+  | Ptbnz sz r n lbl =>
+      match eval_testbit sz rs#r n with
+      | Some true => goto_label f lbl rs m
+      | Some false => Next (nextinstr rs) m
+      | None => Stuck
+      end
+  | Ptbz sz r n lbl =>
+      match eval_testbit sz rs#r n with
+      | Some true => Next (nextinstr rs) m
+      | Some false => goto_label f lbl rs m
+      | None => Stuck
+      end
+  (** Memory loads and stores *)
+  | Pldrw rd a =>
+      exec_load Mint32 (fun v => v) a rd rs m
+  | Pldrw_a rd a =>
+      exec_load Many32 (fun v => v) a rd rs m
+  | Pldrx rd a =>
+      exec_load Mint64 (fun v => v) a rd rs m
+  | Pldrx_a rd a =>
+      exec_load Many64 (fun v => v) a rd rs m
+  | Pldrb W rd a =>
+      exec_load Mint8unsigned (fun v => v) a rd rs m
+  | Pldrb X rd a =>
+      exec_load Mint8unsigned Val.longofintu a rd rs m
+  | Pldrsb W rd a =>
+      exec_load Mint8signed (fun v => v) a rd rs m
+  | Pldrsb X rd a =>
+      exec_load Mint8signed Val.longofint a rd rs m
+  | Pldrh W rd a =>
+      exec_load Mint16unsigned (fun v => v) a rd rs m
+  | Pldrh X rd a =>
+      exec_load Mint16unsigned Val.longofintu a rd rs m
+  | Pldrsh W rd a =>
+      exec_load Mint16signed (fun v => v) a rd rs m
+  | Pldrsh X rd a =>
+      exec_load Mint16signed Val.longofint a rd rs m
+  | Pldrzw rd a =>
+      exec_load Mint32 Val.longofintu a rd rs m
+  | Pldrsw rd a =>
+      exec_load Mint32 Val.longofint a rd rs m
+  | Pstrw r a =>
+      exec_store Mint32 a rs#r rs m
+  | Pstrw_a r a =>
+      exec_store Many32 a rs#r rs m
+  | Pstrx r a =>
+      exec_store Mint64 a rs#r rs m
+  | Pstrx_a r a =>
+      exec_store Many64 a rs#r rs m
+  | Pstrb r a =>
+      exec_store Mint8unsigned a rs#r rs m
+  | Pstrh r a =>
+      exec_store Mint16unsigned a rs#r rs m
+  (** Integer arithmetic, immediate *)
+  | Paddimm W rd r1 n =>
+      Next (nextinstr (rs#rd <- (Val.add rs#r1 (Vint (Int.repr n))))) m
+  | Paddimm X rd r1 n =>
+      Next (nextinstr (rs#rd <- (Val.addl rs#r1 (Vlong (Int64.repr n))))) m
+  | Psubimm W rd r1 n =>
+      Next (nextinstr (rs#rd <- (Val.sub rs#r1 (Vint (Int.repr n))))) m
+  | Psubimm X rd r1 n =>
+      Next (nextinstr (rs#rd <- (Val.subl rs#r1 (Vlong (Int64.repr n))))) m
+  | Pcmpimm W r1 n =>
+      Next (nextinstr (compare_int rs rs#r1 (Vint (Int.repr n)) m)) m
+  | Pcmpimm X r1 n =>
+      Next (nextinstr (compare_long rs rs#r1 (Vlong (Int64.repr n)) m)) m
+  | Pcmnimm W r1 n =>
+      Next (nextinstr (compare_int rs rs#r1 (Vint (Int.neg (Int.repr n))) m)) m
+  | Pcmnimm X r1 n =>
+      Next (nextinstr (compare_long rs rs#r1 (Vlong (Int64.neg (Int64.repr n))) m)) m
+  (** Move integer register *)
+  | Pmov rd r1 =>
+      Next (nextinstr (rs#rd <- (rs#r1))) m
+  (** Logical, immediate *)
+  | Pandimm W rd r1 n =>
+      Next (nextinstr (rs#rd <- (Val.and rs##r1 (Vint (Int.repr n))))) m
+  | Pandimm X rd r1 n =>
+      Next (nextinstr (rs#rd <- (Val.andl rs###r1 (Vlong (Int64.repr n))))) m
+  | Peorimm W rd r1 n =>
+      Next (nextinstr (rs#rd <- (Val.xor rs##r1 (Vint (Int.repr n))))) m
+  | Peorimm X rd r1 n =>
+      Next (nextinstr (rs#rd <- (Val.xorl rs###r1 (Vlong (Int64.repr n))))) m
+  | Porrimm W rd r1 n =>
+      Next (nextinstr (rs#rd <- (Val.or rs##r1 (Vint (Int.repr n))))) m
+  | Porrimm X rd r1 n =>
+      Next (nextinstr (rs#rd <- (Val.orl rs###r1 (Vlong (Int64.repr n))))) m
+  | Ptstimm W r1 n =>
+      Next (nextinstr (compare_int rs (Val.and rs#r1 (Vint (Int.repr n))) (Vint Int.zero) m)) m
+  | Ptstimm X r1 n =>
+      Next (nextinstr (compare_long rs (Val.andl rs#r1 (Vlong (Int64.repr n))) (Vlong Int64.zero) m)) m
+  (** Move wide immediate *)
+  | Pmovz W rd n pos =>
+      Next (nextinstr (rs#rd <- (Vint (Int.repr (Z.shiftl n pos))))) m
+  | Pmovz X rd n pos =>
+      Next (nextinstr (rs#rd <- (Vlong (Int64.repr (Z.shiftl n pos))))) m
+  | Pmovn W rd n pos =>
+      Next (nextinstr (rs#rd <- (Vint (Int.repr (Z.lnot (Z.shiftl n pos)))))) m
+  | Pmovn X rd n pos =>
+      Next (nextinstr (rs#rd <- (Vlong (Int64.repr (Z.lnot (Z.shiftl n pos)))))) m
+  | Pmovk W rd n pos =>
+      Next (nextinstr (rs#rd <- (insert_in_int rs#rd n pos 16))) m
+  | Pmovk X rd n pos =>
+      Next (nextinstr (rs#rd <- (insert_in_long rs#rd n pos 16))) m
+  (** PC-relative addressing *)
+  | Padrp rd id ofs =>
+      Next (nextinstr (rs#rd <- (symbol_high ge id ofs))) m
+  | Paddadr rd r1 id ofs =>
+      Next (nextinstr (rs#rd <- (Val.addl rs#r1 (symbol_low ge id ofs)))) m
+  (** Bit-field operations *)
+  | Psbfiz W rd r1 r s =>
+      Next (nextinstr (rs#rd <- (Val.shl (Val.sign_ext s rs#r1) (Vint r)))) m
+  | Psbfiz X rd r1 r s =>
+      Next (nextinstr (rs#rd <- (Val.shll (Val.sign_ext_l s rs#r1) (Vint r)))) m
+  | Psbfx W rd r1 r s =>
+      Next (nextinstr (rs#rd <- (Val.sign_ext s (Val.shr rs#r1 (Vint r))))) m
+  | Psbfx X rd r1 r s =>
+      Next (nextinstr (rs#rd <- (Val.sign_ext_l s (Val.shrl rs#r1 (Vint r))))) m
+  | Pubfiz W rd r1 r s =>
+      Next (nextinstr (rs#rd <- (Val.shl (Val.zero_ext s rs#r1) (Vint r)))) m
+  | Pubfiz X rd r1 r s =>
+      Next (nextinstr (rs#rd <- (Val.shll (Val.zero_ext_l s rs#r1) (Vint r)))) m
+  | Pubfx W rd r1 r s =>
+      Next (nextinstr (rs#rd <- (Val.zero_ext s (Val.shru rs#r1 (Vint r))))) m
+  | Pubfx X rd r1 r s =>
+      Next (nextinstr (rs#rd <- (Val.zero_ext_l s (Val.shrlu rs#r1 (Vint r))))) m
+  (** Integer arithmetic, shifted register *)
+  | Padd W rd r1 r2 s =>
+      Next (nextinstr (rs#rd <- (Val.add rs##r1 (eval_shift_op_int rs#r2 s)))) m
+  | Padd X rd r1 r2 s =>
+      Next (nextinstr (rs#rd <- (Val.addl rs###r1 (eval_shift_op_long rs#r2 s)))) m
+  | Psub W rd r1 r2 s =>
+      Next (nextinstr (rs#rd <- (Val.sub rs##r1 (eval_shift_op_int rs#r2 s)))) m
+  | Psub X rd r1 r2 s =>
+      Next (nextinstr (rs#rd <- (Val.subl rs###r1 (eval_shift_op_long rs#r2 s)))) m
+  | Pcmp W r1 r2 s =>
+      Next (nextinstr (compare_int rs rs##r1 (eval_shift_op_int rs#r2 s) m)) m
+  | Pcmp X r1 r2 s =>
+      Next (nextinstr (compare_long rs rs###r1 (eval_shift_op_long rs#r2 s) m)) m
+  | Pcmn W r1 r2 s =>
+      Next (nextinstr (compare_int rs rs##r1 (Val.neg (eval_shift_op_int rs#r2 s)) m)) m
+  | Pcmn X r1 r2 s =>
+      Next (nextinstr (compare_long rs rs###r1 (Val.negl (eval_shift_op_long rs#r2 s)) m)) m
+  (** Integer arithmetic, extending register *)
+  | Paddext rd r1 r2 x =>
+      Next (nextinstr (rs#rd <- (Val.addl rs#r1 (eval_extend rs#r2 x)))) m
+  | Psubext rd r1 r2 x =>
+      Next (nextinstr (rs#rd <- (Val.subl rs#r1 (eval_extend rs#r2 x)))) m
+  | Pcmpext r1 r2 x =>
+      Next (nextinstr (compare_long rs rs#r1 (eval_extend rs#r2 x) m)) m
+  | Pcmnext r1 r2 x =>
+      Next (nextinstr (compare_long rs rs#r1 (Val.negl (eval_extend rs#r2 x)) m)) m
+  (** Logical, shifted register *)
+  | Pand W rd r1 r2 s =>
+      Next (nextinstr (rs#rd <- (Val.and rs##r1 (eval_shift_op_int rs#r2 s)))) m
+  | Pand X rd r1 r2 s =>
+      Next (nextinstr (rs#rd <- (Val.andl rs###r1 (eval_shift_op_long rs#r2 s)))) m
+  | Pbic W rd r1 r2 s =>
+      Next (nextinstr (rs#rd <- (Val.and rs##r1 (Val.notint (eval_shift_op_int rs#r2 s))))) m
+  | Pbic X rd r1 r2 s =>
+      Next (nextinstr (rs#rd <- (Val.andl rs###r1 (Val.notl (eval_shift_op_long rs#r2 s))))) m
+  | Peon W rd r1 r2 s =>
+      Next (nextinstr (rs#rd <- (Val.xor rs##r1 (Val.notint (eval_shift_op_int rs#r2 s))))) m
+  | Peon X rd r1 r2 s =>
+      Next (nextinstr (rs#rd <- (Val.xorl rs###r1 (Val.notl (eval_shift_op_long rs#r2 s))))) m
+  | Peor W rd r1 r2 s =>
+      Next (nextinstr (rs#rd <- (Val.xor rs##r1 (eval_shift_op_int rs#r2 s)))) m
+  | Peor X rd r1 r2 s =>
+      Next (nextinstr (rs#rd <- (Val.xorl rs###r1 (eval_shift_op_long rs#r2 s)))) m
+  | Porr W rd r1 r2 s =>
+      Next (nextinstr (rs#rd <- (Val.or rs##r1 (eval_shift_op_int rs#r2 s)))) m
+  | Porr X rd r1 r2 s =>
+      Next (nextinstr (rs#rd <- (Val.orl rs###r1 (eval_shift_op_long rs#r2 s)))) m
+  | Porn W rd r1 r2 s =>
+      Next (nextinstr (rs#rd <- (Val.or rs##r1 (Val.notint (eval_shift_op_int rs#r2 s))))) m
+  | Porn X rd r1 r2 s =>
+      Next (nextinstr (rs#rd <- (Val.orl rs###r1 (Val.notl (eval_shift_op_long rs#r2 s))))) m
+  | Ptst W r1 r2 s =>
+      Next (nextinstr (compare_int rs (Val.and rs##r1 (eval_shift_op_int rs#r2 s)) (Vint Int.zero) m)) m
+  | Ptst X r1 r2 s =>
+      Next (nextinstr (compare_long rs (Val.andl rs###r1 (eval_shift_op_long rs#r2 s)) (Vlong Int64.zero) m)) m
+  (** Variable shifts *)
+  | Pasrv W rd r1 r2 =>
+      Next (nextinstr (rs#rd <- (Val.shr rs#r1 rs#r2))) m
+  | Pasrv X rd r1 r2 =>
+      Next (nextinstr (rs#rd <- (Val.shrl rs#r1 rs#r2))) m
+  | Plslv W rd r1 r2 =>
+      Next (nextinstr (rs#rd <- (Val.shl rs#r1 rs#r2))) m
+  | Plslv X rd r1 r2 =>
+      Next (nextinstr (rs#rd <- (Val.shll rs#r1 rs#r2))) m
+  | Plsrv W rd r1 r2 =>
+      Next (nextinstr (rs#rd <- (Val.shru rs#r1 rs#r2))) m
+  | Plsrv X rd r1 r2 =>
+      Next (nextinstr (rs#rd <- (Val.shrlu rs#r1 rs#r2))) m
+  | Prorv W rd r1 r2 =>
+      Next (nextinstr (rs#rd <- (Val.ror rs#r1 rs#r2))) m
+  | Prorv X rd r1 r2 =>
+      Next (nextinstr (rs#rd <- (Val.rorl rs#r1 rs#r2))) m
+  (** Conditional data processing *)
+  | Pcsel rd r1 r2 cond =>
+      let v :=
         match eval_testcond cond rs with
-        | Some true => goto_label f lbl rs m
-        | Some false => Next (nextinstr rs) m
-        | None => Stuck
-        end
-    | Pbl id sg =>
-        Next (rs#RA <- (Val.offset_ptr rs#PC Ptrofs.one) #PC <- (Genv.symbol_address ge id Ptrofs.zero)) m
-    | Pbs id sg =>
-        Next (rs#PC <- (Genv.symbol_address ge id Ptrofs.zero)) m
-    | Pblr r sg =>
-        Next (rs#RA <- (Val.offset_ptr rs#PC Ptrofs.one) #PC <- (rs#r)) m
-    | Pbr r sg =>
-        Next (rs#PC <- (rs#r)) m
-    | Pret r =>
-        Next (rs#PC <- (rs#r)) m
-    | Pcbnz sz r lbl =>
-        match eval_testzero sz rs#r m with
-        | Some true => Next (nextinstr rs) m
-        | Some false => goto_label f lbl rs m
-        | None => Stuck
-        end
-    | Pcbz sz r lbl =>
-        match eval_testzero sz rs#r m with
-        | Some true => goto_label f lbl rs m
-        | Some false => Next (nextinstr rs) m
-        | None => Stuck
-        end
-    | Ptbnz sz r n lbl =>
-        match eval_testbit sz rs#r n with
-        | Some true => goto_label f lbl rs m
-        | Some false => Next (nextinstr rs) m
-        | None => Stuck
-        end
-    | Ptbz sz r n lbl =>
-        match eval_testbit sz rs#r n with
-        | Some true => Next (nextinstr rs) m
-        | Some false => goto_label f lbl rs m
-        | None => Stuck
-        end
-    (** Memory loads and stores *)
-    | Pldrw rd a =>
-        exec_load Mint32 (fun v => v) a rd rs m
-    | Pldrw_a rd a =>
-        exec_load Many32 (fun v => v) a rd rs m
-    | Pldrx rd a =>
-        exec_load Mint64 (fun v => v) a rd rs m
-    | Pldrx_a rd a =>
-        exec_load Many64 (fun v => v) a rd rs m
-    | Pldrb W rd a =>
-        exec_load Mint8unsigned (fun v => v) a rd rs m
-    | Pldrb X rd a =>
-        exec_load Mint8unsigned Val.longofintu a rd rs m
-    | Pldrsb W rd a =>
-        exec_load Mint8signed (fun v => v) a rd rs m
-    | Pldrsb X rd a =>
-        exec_load Mint8signed Val.longofint a rd rs m
-    | Pldrh W rd a =>
-        exec_load Mint16unsigned (fun v => v) a rd rs m
-    | Pldrh X rd a =>
-        exec_load Mint16unsigned Val.longofintu a rd rs m
-    | Pldrsh W rd a =>
-        exec_load Mint16signed (fun v => v) a rd rs m
-    | Pldrsh X rd a =>
-        exec_load Mint16signed Val.longofint a rd rs m
-    | Pldrzw rd a =>
-        exec_load Mint32 Val.longofintu a rd rs m
-    | Pldrsw rd a =>
-        exec_load Mint32 Val.longofint a rd rs m
-    | Pstrw r a =>
-        exec_store Mint32 a rs#r rs m
-    | Pstrw_a r a =>
-        exec_store Many32 a rs#r rs m
-    | Pstrx r a =>
-        exec_store Mint64 a rs#r rs m
-    | Pstrx_a r a =>
-        exec_store Many64 a rs#r rs m
-    | Pstrb r a =>
-        exec_store Mint8unsigned a rs#r rs m
-    | Pstrh r a =>
-        exec_store Mint16unsigned a rs#r rs m
-    (** Integer arithmetic, immediate *)
-    | Paddimm W rd r1 n =>
-        Next (nextinstr (rs#rd <- (Val.add rs#r1 (Vint (Int.repr n))))) m
-    | Paddimm X rd r1 n =>
-        Next (nextinstr (rs#rd <- (Val.addl rs#r1 (Vlong (Int64.repr n))))) m
-    | Psubimm W rd r1 n =>
-        Next (nextinstr (rs#rd <- (Val.sub rs#r1 (Vint (Int.repr n))))) m
-    | Psubimm X rd r1 n =>
-        Next (nextinstr (rs#rd <- (Val.subl rs#r1 (Vlong (Int64.repr n))))) m
-    | Pcmpimm W r1 n =>
-        Next (nextinstr (compare_int rs rs#r1 (Vint (Int.repr n)) m)) m
-    | Pcmpimm X r1 n =>
-        Next (nextinstr (compare_long rs rs#r1 (Vlong (Int64.repr n)) m)) m
-    | Pcmnimm W r1 n =>
-        Next (nextinstr (compare_int rs rs#r1 (Vint (Int.neg (Int.repr n))) m)) m
-    | Pcmnimm X r1 n =>
-        Next (nextinstr (compare_long rs rs#r1 (Vlong (Int64.neg (Int64.repr n))) m)) m
-    (** Move integer register *)
-    | Pmov rd r1 =>
-        Next ( nextinstr (rs#rd <- (rs#r1))) m
-    (** Logical, immediate *)
-    | Pandimm W rd r1 n =>
-        Next (nextinstr (rs#rd <- (Val.and rs##r1 (Vint (Int.repr n))))) m
-    | Pandimm X rd r1 n =>
-        Next (nextinstr (rs#rd <- (Val.andl rs###r1 (Vlong (Int64.repr n))))) m
-    | Peorimm W rd r1 n =>
-        Next (nextinstr (rs#rd <- (Val.xor rs##r1 (Vint (Int.repr n))))) m
-    | Peorimm X rd r1 n =>
-        Next (nextinstr (rs#rd <- (Val.xorl rs###r1 (Vlong (Int64.repr n))))) m
-    | Porrimm W rd r1 n =>
-        Next (nextinstr (rs#rd <- (Val.or rs##r1 (Vint (Int.repr n))))) m
-    | Porrimm X rd r1 n =>
-        Next (nextinstr (rs#rd <- (Val.orl rs###r1 (Vlong (Int64.repr n))))) m
-    | Ptstimm W r1 n =>
-        Next (nextinstr (compare_int rs (Val.and rs#r1 (Vint (Int.repr n))) (Vint Int.zero) m)) m
-    | Ptstimm X r1 n =>
-        Next (nextinstr (compare_long rs (Val.andl rs#r1 (Vlong (Int64.repr n))) (Vlong Int64.zero) m)) m
-    (** Move wide immediate *)
-    | Pmovz W rd n pos =>
-        Next (nextinstr (rs#rd <- (Vint (Int.repr (Z.shiftl n pos))))) m
-    | Pmovz X rd n pos =>
-        Next (nextinstr (rs#rd <- (Vlong (Int64.repr (Z.shiftl n pos))))) m
-    | Pmovn W rd n pos =>
-        Next (nextinstr (rs#rd <- (Vint (Int.repr (Z.lnot (Z.shiftl n pos)))))) m
-    | Pmovn X rd n pos =>
-        Next (nextinstr (rs#rd <- (Vlong (Int64.repr (Z.lnot (Z.shiftl n pos)))))) m
-    | Pmovk W rd n pos =>
-        Next (nextinstr (rs#rd <- (insert_in_int rs#rd n pos 16))) m
-    | Pmovk X rd n pos =>
-        Next (nextinstr (rs#rd <- (insert_in_long rs#rd n pos 16))) m
-    (** PC-relative addressing *)
-    | Padrp rd id ofs =>
-        Next (nextinstr (rs#rd <- (symbol_high ge id ofs))) m
-    | Paddadr rd r1 id ofs =>
-        Next (nextinstr (rs#rd <- (Val.addl rs#r1 (symbol_low ge id ofs)))) m
-    (** Bit-field operations *)
-    | Psbfiz W rd r1 r s =>
-        Next (nextinstr (rs#rd <- (Val.shl (Val.sign_ext s rs#r1) (Vint r)))) m
-    | Psbfiz X rd r1 r s =>
-        Next (nextinstr (rs#rd <- (Val.shll (Val.sign_ext_l s rs#r1) (Vint r)))) m
-    | Psbfx W rd r1 r s =>
-        Next (nextinstr (rs#rd <- (Val.sign_ext s (Val.shr rs#r1 (Vint r))))) m
-    | Psbfx X rd r1 r s =>
-        Next (nextinstr (rs#rd <- (Val.sign_ext_l s (Val.shrl rs#r1 (Vint r))))) m
-    | Pubfiz W rd r1 r s =>
-        Next (nextinstr (rs#rd <- (Val.shl (Val.zero_ext s rs#r1) (Vint r)))) m
-    | Pubfiz X rd r1 r s =>
-        Next (nextinstr (rs#rd <- (Val.shll (Val.zero_ext_l s rs#r1) (Vint r)))) m
-    | Pubfx W rd r1 r s =>
-        Next (nextinstr (rs#rd <- (Val.zero_ext s (Val.shru rs#r1 (Vint r))))) m
-    | Pubfx X rd r1 r s =>
-        Next (nextinstr (rs#rd <- (Val.zero_ext_l s (Val.shrlu rs#r1 (Vint r))))) m
-    (** Integer arithmetic, shifted register *)
-    | Padd W rd r1 r2 s =>
-        Next (nextinstr (rs#rd <- (Val.add rs##r1 (eval_shift_op_int rs#r2 s)))) m
-    | Padd X rd r1 r2 s =>
-        Next (nextinstr (rs#rd <- (Val.addl rs###r1 (eval_shift_op_long rs#r2 s)))) m
-    | Psub W rd r1 r2 s =>
-        Next (nextinstr (rs#rd <- (Val.sub rs##r1 (eval_shift_op_int rs#r2 s)))) m
-    | Psub X rd r1 r2 s =>
-        Next (nextinstr (rs#rd <- (Val.subl rs###r1 (eval_shift_op_long rs#r2 s)))) m
-    | Pcmp W r1 r2 s =>
-        Next (nextinstr (compare_int rs rs##r1 (eval_shift_op_int rs#r2 s) m)) m
-    | Pcmp X r1 r2 s =>
-        Next (nextinstr (compare_long rs rs###r1 (eval_shift_op_long rs#r2 s) m)) m
-    | Pcmn W r1 r2 s =>
-        Next (nextinstr (compare_int rs rs##r1 (Val.neg (eval_shift_op_int rs#r2 s)) m)) m
-    | Pcmn X r1 r2 s =>
-        Next (nextinstr (compare_long rs rs###r1 (Val.negl (eval_shift_op_long rs#r2 s)) m)) m
-    (** Integer arithmetic, extending register *)
-    | Paddext rd r1 r2 x =>
-        Next (nextinstr (rs#rd <- (Val.addl rs#r1 (eval_extend rs#r2 x)))) m
-    | Psubext rd r1 r2 x =>
-        Next (nextinstr (rs#rd <- (Val.subl rs#r1 (eval_extend rs#r2 x)))) m
-    | Pcmpext r1 r2 x =>
-        Next (nextinstr (compare_long rs rs#r1 (eval_extend rs#r2 x) m)) m
-    | Pcmnext r1 r2 x =>
-        Next (nextinstr (compare_long rs rs#r1 (Val.negl (eval_extend rs#r2 x)) m)) m
-    (** Logical, shifted register *)
-    | Pand W rd r1 r2 s =>
-        Next (nextinstr (rs#rd <- (Val.and rs##r1 (eval_shift_op_int rs#r2 s)))) m
-    | Pand X rd r1 r2 s =>
-        Next (nextinstr (rs#rd <- (Val.andl rs###r1 (eval_shift_op_long rs#r2 s)))) m
-    | Pbic W rd r1 r2 s =>
-        Next (nextinstr (rs#rd <- (Val.and rs##r1 (Val.notint (eval_shift_op_int rs#r2 s))))) m
-    | Pbic X rd r1 r2 s =>
-        Next (nextinstr (rs#rd <- (Val.andl rs###r1 (Val.notl (eval_shift_op_long rs#r2 s))))) m
-    | Peon W rd r1 r2 s =>
-        Next (nextinstr (rs#rd <- (Val.xor rs##r1 (Val.notint (eval_shift_op_int rs#r2 s))))) m
-    | Peon X rd r1 r2 s =>
-        Next (nextinstr (rs#rd <- (Val.xorl rs###r1 (Val.notl (eval_shift_op_long rs#r2 s))))) m
-    | Peor W rd r1 r2 s =>
-        Next (nextinstr (rs#rd <- (Val.xor rs##r1 (eval_shift_op_int rs#r2 s)))) m
-    | Peor X rd r1 r2 s =>
-        Next (nextinstr (rs#rd <- (Val.xorl rs###r1 (eval_shift_op_long rs#r2 s)))) m
-    | Porr W rd r1 r2 s =>
-        Next (nextinstr (rs#rd <- (Val.or rs##r1 (eval_shift_op_int rs#r2 s)))) m
-    | Porr X rd r1 r2 s =>
-        Next (nextinstr (rs#rd <- (Val.orl rs###r1 (eval_shift_op_long rs#r2 s)))) m
-    | Porn W rd r1 r2 s =>
-        Next (nextinstr (rs#rd <- (Val.or rs##r1 (Val.notint (eval_shift_op_int rs#r2 s))))) m
-    | Porn X rd r1 r2 s =>
-        Next (nextinstr (rs#rd <- (Val.orl rs###r1 (Val.notl (eval_shift_op_long rs#r2 s))))) m
-    | Ptst W r1 r2 s =>
-        Next (nextinstr (compare_int rs (Val.and rs##r1 (eval_shift_op_int rs#r2 s)) (Vint Int.zero) m)) m
-    | Ptst X r1 r2 s =>
-        Next (nextinstr (compare_long rs (Val.andl rs###r1 (eval_shift_op_long rs#r2 s)) (Vlong Int64.zero) m)) m
-    (** Variable shifts *)
-    | Pasrv W rd r1 r2 =>
-        Next (nextinstr (rs#rd <- (Val.shr rs#r1 rs#r2))) m
-    | Pasrv X rd r1 r2 =>
-        Next (nextinstr (rs#rd <- (Val.shrl rs#r1 rs#r2))) m
-    | Plslv W rd r1 r2 =>
-        Next (nextinstr (rs#rd <- (Val.shl rs#r1 rs#r2))) m
-    | Plslv X rd r1 r2 =>
-        Next (nextinstr (rs#rd <- (Val.shll rs#r1 rs#r2))) m
-    | Plsrv W rd r1 r2 =>
-        Next (nextinstr (rs#rd <- (Val.shru rs#r1 rs#r2))) m
-    | Plsrv X rd r1 r2 =>
-        Next (nextinstr (rs#rd <- (Val.shrlu rs#r1 rs#r2))) m
-    | Prorv W rd r1 r2 =>
-        Next (nextinstr (rs#rd <- (Val.ror rs#r1 rs#r2))) m
-    | Prorv X rd r1 r2 =>
-        Next (nextinstr (rs#rd <- (Val.rorl rs#r1 rs#r2))) m
-    (** Conditional data processing *)
-    | Pcsel rd r1 r2 cond =>
-        let v :=
-            match eval_testcond cond rs with
-            | Some true => rs#r1
-            | Some false => rs#r2
-            | None => Vundef
-            end in
-        Next (nextinstr (rs#rd <- v)) m
-    | Pcset rd cond =>
-        let v :=
-            match eval_testcond cond rs with
-            | Some true => Vint Int.one
-            | Some false => Vint Int.zero
-            | None => Vundef
-            end in
-        Next (nextinstr (rs#rd <- v)) m
-    (** Integer multiply/divide *)
-    | Pmadd W rd r1 r2 r3 =>
-        Next (nextinstr (rs#rd <- (Val.add rs##r3 (Val.mul rs#r1 rs#r2)))) m
-    | Pmadd X rd r1 r2 r3 =>
-        Next (nextinstr (rs#rd <- (Val.addl rs###r3 (Val.mull rs#r1 rs#r2)))) m
-    | Pmsub W rd r1 r2 r3 =>
-        Next (nextinstr (rs#rd <- (Val.sub rs##r3 (Val.mul rs#r1 rs#r2)))) m
-    | Pmsub X rd r1 r2 r3 =>
-        Next (nextinstr (rs#rd <- (Val.subl rs###r3 (Val.mull rs#r1 rs#r2)))) m
-    | Psmulh rd r1 r2 =>
-        Next (nextinstr (rs#rd <- (Val.mullhs rs#r1 rs#r2))) m
-    | Pumulh rd r1 r2 =>
-        Next (nextinstr (rs#rd <- (Val.mullhu rs#r1 rs#r2))) m
-    | Psdiv W rd r1 r2 =>
-        Next (nextinstr (rs#rd <- (Val.maketotal (Val.divs rs#r1 rs#r2)))) m
-    | Psdiv X rd r1 r2 =>
-        Next (nextinstr (rs#rd <- (Val.maketotal (Val.divls rs#r1 rs#r2)))) m
-    | Pudiv W rd r1 r2 =>
-        Next (nextinstr (rs#rd <- (Val.maketotal (Val.divu rs#r1 rs#r2)))) m
-    | Pudiv X rd r1 r2 =>
-        Next (nextinstr (rs#rd <- (Val.maketotal (Val.divlu rs#r1 rs#r2)))) m
-    (** Floating-point loads and stores *)
-    | Pldrs rd a =>
-        exec_load Mfloat32 (fun v => v) a rd rs m
-    | Pldrd rd a =>
-        exec_load Mfloat64 (fun v => v) a rd rs m
-    | Pldrd_a rd a =>
-        exec_load Many64 (fun v => v) a rd rs m
-    | Pstrs r a =>
-        exec_store Mfloat32 a rs#r rs m
-    | Pstrd r a =>
-        exec_store Mfloat64 a rs#r rs m
-    | Pstrd_a r a =>
-        exec_store Many64 a rs#r rs m
-    (** Floating-point move *)
-    | Pfmov rd r1 =>
-        Next (nextinstr (rs#rd <- (rs#r1))) m
-    | Pfmovimms rd f =>
-        Next (nextinstr (rs#X16 <- Vundef #rd <- (Vsingle f))) m
-    | Pfmovimmd rd f =>
-        Next (nextinstr (rs#X16 <- Vundef #rd <- (Vfloat f))) m
-    | Pfmovi S rd r1 =>
-        Next (nextinstr (rs#rd <- (float32_of_bits rs##r1))) m
-    | Pfmovi D rd r1 =>
-        Next (nextinstr (rs#rd <- (float64_of_bits rs###r1))) m
-    (** Floating-point conversions *)
-    | Pfcvtds rd r1 =>
-        Next (nextinstr (rs#rd <- (Val.floatofsingle rs#r1))) m
-    | Pfcvtsd rd r1 =>
-        Next (nextinstr (rs#rd <- (Val.singleoffloat rs#r1))) m
-    | Pfcvtzs W S rd r1 =>
-        Next (nextinstr (rs#rd <- (Val.maketotal (Val.intofsingle rs#r1)))) m
-    | Pfcvtzs W D rd r1 =>
-        Next (nextinstr (rs#rd <- (Val.maketotal (Val.intoffloat rs#r1)))) m
-    | Pfcvtzs X S rd r1 =>
-        Next (nextinstr (rs#rd <- (Val.maketotal (Val.longofsingle rs#r1)))) m
-    | Pfcvtzs X D rd r1 =>
-        Next (nextinstr (rs#rd <- (Val.maketotal (Val.longoffloat rs#r1)))) m
-    | Pfcvtzu W S rd r1 =>
-        Next (nextinstr (rs#rd <- (Val.maketotal (Val.intuofsingle rs#r1)))) m
-    | Pfcvtzu W D rd r1 =>
-        Next (nextinstr (rs#rd <- (Val.maketotal (Val.intuoffloat rs#r1)))) m
-    | Pfcvtzu X S rd r1 =>
-        Next (nextinstr (rs#rd <- (Val.maketotal (Val.longuofsingle rs#r1)))) m
-    | Pfcvtzu X D rd r1 =>
-        Next (nextinstr (rs#rd <- (Val.maketotal (Val.longuoffloat rs#r1)))) m
-    | Pscvtf S W rd r1 =>
-        Next (nextinstr (rs#rd <- (Val.maketotal (Val.singleofint rs#r1)))) m
-    | Pscvtf D W rd r1 =>
-        Next (nextinstr (rs#rd <- (Val.maketotal (Val.floatofint rs#r1)))) m
-    | Pscvtf S X rd r1 =>
-        Next (nextinstr (rs#rd <- (Val.maketotal (Val.singleoflong rs#r1)))) m
-    | Pscvtf D X rd r1 =>
-        Next (nextinstr (rs#rd <- (Val.maketotal (Val.floatoflong rs#r1)))) m
-    | Pucvtf S W rd r1 =>
-        Next (nextinstr (rs#rd <- (Val.maketotal (Val.singleofintu rs#r1)))) m
-    | Pucvtf D W rd r1 =>
-        Next (nextinstr (rs#rd <- (Val.maketotal (Val.floatofintu rs#r1)))) m
-    | Pucvtf S X rd r1 =>
-        Next (nextinstr (rs#rd <- (Val.maketotal (Val.singleoflongu rs#r1)))) m
-    | Pucvtf D X rd r1 =>
-        Next (nextinstr (rs#rd <- (Val.maketotal (Val.floatoflongu rs#r1)))) m
-    (** Floating-point arithmetic *)
-    | Pfabs S rd r1 =>
-        Next (nextinstr (rs#rd <- (Val.absfs rs#r1))) m
-    | Pfabs D rd r1 =>
-        Next (nextinstr (rs#rd <- (Val.absf rs#r1))) m
-    | Pfneg S rd r1 =>
-        Next (nextinstr (rs#rd <- (Val.negfs rs#r1))) m
-    | Pfneg D rd r1 =>
-        Next (nextinstr (rs#rd <- (Val.negf rs#r1))) m
-    | Pfadd S rd r1 r2 =>
-        Next (nextinstr (rs#rd <- (Val.addfs rs#r1 rs#r2))) m
-    | Pfadd D rd r1 r2 =>
-        Next (nextinstr (rs#rd <- (Val.addf rs#r1 rs#r2))) m
-    | Pfdiv S rd r1 r2 =>
-        Next (nextinstr (rs#rd <- (Val.divfs rs#r1 rs#r2))) m
-    | Pfdiv D rd r1 r2 =>
-        Next (nextinstr (rs#rd <- (Val.divf rs#r1 rs#r2))) m
-    | Pfmul S rd r1 r2 =>
-        Next (nextinstr (rs#rd <- (Val.mulfs rs#r1 rs#r2))) m
-    | Pfmul D rd r1 r2 =>
-        Next (nextinstr (rs#rd <- (Val.mulf rs#r1 rs#r2))) m
-    | Pfnmul S rd r1 r2 =>
-        Next (nextinstr (rs#rd <- (Val.negfs (Val.mulfs rs#r1 rs#r2)))) m
-    | Pfnmul D rd r1 r2 =>
-        Next (nextinstr (rs#rd <- (Val.negf (Val.mulf rs#r1 rs#r2)))) m
-    | Pfsub S rd r1 r2 =>
-        Next (nextinstr (rs#rd <- (Val.subfs rs#r1 rs#r2))) m
-    | Pfsub D rd r1 r2 =>
-        Next (nextinstr (rs#rd <- (Val.subf rs#r1 rs#r2))) m
-    (** Floating-point comparison *)
-    | Pfcmp S r1 r2 =>
-        Next (nextinstr (compare_single rs rs#r1 rs#r2)) m
-    | Pfcmp D r1 r2 =>
-        Next (nextinstr (compare_float rs rs#r1 rs#r2)) m
-    | Pfcmp0 S r1 =>
-        Next (nextinstr (compare_single rs rs#r1 (Vsingle Float32.zero))) m
-    | Pfcmp0 D r1 =>
-        Next (nextinstr (compare_float rs rs#r1 (Vfloat Float.zero))) m
-    (** Floating-point conditional select *)
-    | Pfsel rd r1 r2 cond =>
-        let v :=
-            match eval_testcond cond rs with
-            | Some true => rs#r1
-            | Some false => rs#r2
-            | None => Vundef
-            end in
-        Next (nextinstr (rs#rd <- v)) m
-    (** Pseudo-instructions *)
-    | Pallocframe sz pos =>
-        let (m1, stk) := Mem.alloc m 0 sz in
-        let sp := (Vptr stk Ptrofs.zero) in
-        match Mem.storev Mint64 m1 (Val.offset_ptr sp pos) rs#SP with
-        | None => Stuck
-        | Some m2 => Next (nextinstr (rs #X15 <- (rs#SP) #SP <- sp #X16 <- Vundef)) m2
-        end
-    | Pfreeframe sz pos =>
-        match Mem.loadv Mint64 m (Val.offset_ptr rs#SP pos) with
-        | None => Stuck
-        | Some v =>
-            match rs#SP with
-            | Vptr stk ofs =>
-                match Mem.free m stk 0 sz with
-                | None => Stuck
-                | Some m' => Next (nextinstr (rs#SP <- v #X16 <- Vundef)) m'
-                end
-            | _ => Stuck
-            end
-        end
-    | Plabel lbl =>
-        Next (nextinstr rs) m
-    | Ploadsymbol rd id =>
-        Next (nextinstr (rs#rd <- (Genv.symbol_address ge id Ptrofs.zero))) m
-    | Pcvtsw2x rd r1 =>
-        Next (nextinstr (rs#rd <- (Val.longofint rs#r1))) m
-    | Pcvtuw2x rd r1 =>
-        Next (nextinstr (rs#rd <- (Val.longofintu rs#r1))) m
-    | Pcvtx2w rd =>
-        Next (nextinstr (rs#rd <- (Val.loword rs#rd))) m
-    | Pbtbl r tbl =>
-        match (rs#X16 <- Vundef)#r with
-        | Vint n =>
-            match list_nth_z tbl (Int.unsigned n) with
-            | None => Stuck
-            | Some lbl => goto_label f lbl (rs#X16 <- Vundef) m
-            end
-        | _ => Stuck
-        end
-    | Pcfi_rel_offset _ =>
-        Next (nextinstr rs) m
-    | Pbuiltin ef args res => Stuck    (**r treated specially below *)
-    (** The following instructions and directives are not generated directly
-        by Asmgen, so we do not model them. *)
-    | Pldp _ _ _
-    | Pstp _ _ _
-    | Pcls _ _ _
-    | Pclz _ _ _
-    | Prev _ _ _
-    | Prev16 _ _ _
-    | Prbit _ _ _
-    | Pfsqrt _ _ _
-    | Pfmadd _ _ _ _ _
-    | Pfmsub _ _ _ _ _
-    | Pfnmadd _ _ _ _ _
-    | Pfnmsub _ _ _ _ _
-    | Pfmax _ _ _ _
-    | Pfmin _ _ _ _
-    | Pnop
-    | Pincpc => Next (nextinstr rs) m
-    | Pcfi_adjust _ =>
-        Stuck
-    end
-    end.
+        | Some true => rs#r1
+        | Some false => rs#r2
+        | None => Vundef
+        end in
+      Next (nextinstr (rs#rd <- v)) m
+  | Pcset rd cond =>
+      let v :=
+        match eval_testcond cond rs with
+        | Some true => Vint Int.one
+        | Some false => Vint Int.zero
+        | None => Vundef
+        end in
+      Next (nextinstr (rs#rd <- v)) m
+  (** Integer multiply/divide *)
+  | Pmadd W rd r1 r2 r3 =>
+      Next (nextinstr (rs#rd <- (Val.add rs##r3 (Val.mul rs#r1 rs#r2)))) m
+  | Pmadd X rd r1 r2 r3 =>
+      Next (nextinstr (rs#rd <- (Val.addl rs###r3 (Val.mull rs#r1 rs#r2)))) m
+  | Pmsub W rd r1 r2 r3 =>
+      Next (nextinstr (rs#rd <- (Val.sub rs##r3 (Val.mul rs#r1 rs#r2)))) m
+  | Pmsub X rd r1 r2 r3 =>
+      Next (nextinstr (rs#rd <- (Val.subl rs###r3 (Val.mull rs#r1 rs#r2)))) m
+  | Psmulh rd r1 r2 =>
+      Next (nextinstr (rs#rd <- (Val.mullhs rs#r1 rs#r2))) m
+  | Pumulh rd r1 r2 =>
+      Next (nextinstr (rs#rd <- (Val.mullhu rs#r1 rs#r2))) m
+  | Psdiv W rd r1 r2 =>
+      Next (nextinstr (rs#rd <- (Val.maketotal (Val.divs rs#r1 rs#r2)))) m
+  | Psdiv X rd r1 r2 =>
+      Next (nextinstr (rs#rd <- (Val.maketotal (Val.divls rs#r1 rs#r2)))) m
+  | Pudiv W rd r1 r2 =>
+      Next (nextinstr (rs#rd <- (Val.maketotal (Val.divu rs#r1 rs#r2)))) m
+  | Pudiv X rd r1 r2 =>
+      Next (nextinstr (rs#rd <- (Val.maketotal (Val.divlu rs#r1 rs#r2)))) m
+  (** Floating-point loads and stores *)
+  | Pldrs rd a =>
+      exec_load Mfloat32 (fun v => v) a rd rs m
+  | Pldrd rd a =>
+      exec_load Mfloat64 (fun v => v) a rd rs m
+  | Pldrd_a rd a =>
+      exec_load Many64 (fun v => v) a rd rs m
+  | Pstrs r a =>
+      exec_store Mfloat32 a rs#r rs m
+  | Pstrd r a =>
+      exec_store Mfloat64 a rs#r rs m
+  | Pstrd_a r a =>
+      exec_store Many64 a rs#r rs m
+  (** Floating-point move *)
+  | Pfmov rd r1 =>
+      Next (nextinstr (rs#rd <- (rs#r1))) m
+  | Pfmovimms rd f =>
+      Next (nextinstr (rs#X16 <- Vundef #rd <- (Vsingle f))) m
+  | Pfmovimmd rd f =>
+      Next (nextinstr (rs#X16 <- Vundef #rd <- (Vfloat f))) m
+  | Pfmovi S rd r1 =>
+      Next (nextinstr (rs#rd <- (float32_of_bits rs##r1))) m
+  | Pfmovi D rd r1 =>
+      Next (nextinstr (rs#rd <- (float64_of_bits rs###r1))) m
+  (** Floating-point conversions *)
+  | Pfcvtds rd r1 =>
+      Next (nextinstr (rs#rd <- (Val.floatofsingle rs#r1))) m
+  | Pfcvtsd rd r1 =>
+      Next (nextinstr (rs#rd <- (Val.singleoffloat rs#r1))) m
+  | Pfcvtzs W S rd r1 =>
+      Next (nextinstr (rs#rd <- (Val.maketotal (Val.intofsingle rs#r1)))) m
+  | Pfcvtzs W D rd r1 =>
+      Next (nextinstr (rs#rd <- (Val.maketotal (Val.intoffloat rs#r1)))) m
+  | Pfcvtzs X S rd r1 =>
+      Next (nextinstr (rs#rd <- (Val.maketotal (Val.longofsingle rs#r1)))) m
+  | Pfcvtzs X D rd r1 =>
+      Next (nextinstr (rs#rd <- (Val.maketotal (Val.longoffloat rs#r1)))) m
+  | Pfcvtzu W S rd r1 =>
+      Next (nextinstr (rs#rd <- (Val.maketotal (Val.intuofsingle rs#r1)))) m
+  | Pfcvtzu W D rd r1 =>
+      Next (nextinstr (rs#rd <- (Val.maketotal (Val.intuoffloat rs#r1)))) m
+  | Pfcvtzu X S rd r1 =>
+      Next (nextinstr (rs#rd <- (Val.maketotal (Val.longuofsingle rs#r1)))) m
+  | Pfcvtzu X D rd r1 =>
+      Next (nextinstr (rs#rd <- (Val.maketotal (Val.longuoffloat rs#r1)))) m
+  | Pscvtf S W rd r1 =>
+      Next (nextinstr (rs#rd <- (Val.maketotal (Val.singleofint rs#r1)))) m
+  | Pscvtf D W rd r1 =>
+      Next (nextinstr (rs#rd <- (Val.maketotal (Val.floatofint rs#r1)))) m
+  | Pscvtf S X rd r1 =>
+      Next (nextinstr (rs#rd <- (Val.maketotal (Val.singleoflong rs#r1)))) m
+  | Pscvtf D X rd r1 =>
+      Next (nextinstr (rs#rd <- (Val.maketotal (Val.floatoflong rs#r1)))) m
+  | Pucvtf S W rd r1 =>
+      Next (nextinstr (rs#rd <- (Val.maketotal (Val.singleofintu rs#r1)))) m
+  | Pucvtf D W rd r1 =>
+      Next (nextinstr (rs#rd <- (Val.maketotal (Val.floatofintu rs#r1)))) m
+  | Pucvtf S X rd r1 =>
+      Next (nextinstr (rs#rd <- (Val.maketotal (Val.singleoflongu rs#r1)))) m
+  | Pucvtf D X rd r1 =>
+      Next (nextinstr (rs#rd <- (Val.maketotal (Val.floatoflongu rs#r1)))) m
+  (** Floating-point arithmetic *)
+  | Pfabs S rd r1 =>
+      Next (nextinstr (rs#rd <- (Val.absfs rs#r1))) m
+  | Pfabs D rd r1 =>
+      Next (nextinstr (rs#rd <- (Val.absf rs#r1))) m
+  | Pfneg S rd r1 =>
+      Next (nextinstr (rs#rd <- (Val.negfs rs#r1))) m
+  | Pfneg D rd r1 =>
+      Next (nextinstr (rs#rd <- (Val.negf rs#r1))) m
+  | Pfadd S rd r1 r2 =>
+      Next (nextinstr (rs#rd <- (Val.addfs rs#r1 rs#r2))) m
+  | Pfadd D rd r1 r2 =>
+      Next (nextinstr (rs#rd <- (Val.addf rs#r1 rs#r2))) m
+  | Pfdiv S rd r1 r2 =>
+      Next (nextinstr (rs#rd <- (Val.divfs rs#r1 rs#r2))) m
+  | Pfdiv D rd r1 r2 =>
+      Next (nextinstr (rs#rd <- (Val.divf rs#r1 rs#r2))) m
+  | Pfmul S rd r1 r2 =>
+      Next (nextinstr (rs#rd <- (Val.mulfs rs#r1 rs#r2))) m
+  | Pfmul D rd r1 r2 =>
+      Next (nextinstr (rs#rd <- (Val.mulf rs#r1 rs#r2))) m
+  | Pfnmul S rd r1 r2 =>
+      Next (nextinstr (rs#rd <- (Val.negfs (Val.mulfs rs#r1 rs#r2)))) m
+  | Pfnmul D rd r1 r2 =>
+      Next (nextinstr (rs#rd <- (Val.negf (Val.mulf rs#r1 rs#r2)))) m
+  | Pfsub S rd r1 r2 =>
+      Next (nextinstr (rs#rd <- (Val.subfs rs#r1 rs#r2))) m
+  | Pfsub D rd r1 r2 =>
+      Next (nextinstr (rs#rd <- (Val.subf rs#r1 rs#r2))) m
+  (** Floating-point comparison *)
+  | Pfcmp S r1 r2 =>
+      Next (nextinstr (compare_single rs rs#r1 rs#r2)) m
+  | Pfcmp D r1 r2 =>
+      Next (nextinstr (compare_float rs rs#r1 rs#r2)) m
+  | Pfcmp0 S r1 =>
+      Next (nextinstr (compare_single rs rs#r1 (Vsingle Float32.zero))) m
+  | Pfcmp0 D r1 =>
+      Next (nextinstr (compare_float rs rs#r1 (Vfloat Float.zero))) m
+  (** Floating-point conditional select *)
+  | Pfsel rd r1 r2 cond =>
+      let v :=
+        match eval_testcond cond rs with
+        | Some true => rs#r1
+        | Some false => rs#r2
+        | None => Vundef
+        end in
+      Next (nextinstr (rs#rd <- v)) m
+  (** Pseudo-instructions *)
+  | Pallocframe sz pos =>
+      let (m1, stk) := Mem.alloc m 0 sz in
+      let sp := (Vptr stk Ptrofs.zero) in
+      match Mem.storev Mint64 m1 (Val.offset_ptr sp pos) rs#SP with
+      | None => Stuck
+      | Some m2 => Next (nextinstr (rs #X15 <- (rs#SP) #SP <- sp #X16 <- Vundef)) m2
+      end
+  | Pfreeframe sz pos =>
+      match Mem.loadv Mint64 m (Val.offset_ptr rs#SP pos) with
+      | None => Stuck
+      | Some v =>
+          match rs#SP with
+          | Vptr stk ofs =>
+              match Mem.free m stk 0 sz with
+              | None => Stuck
+              | Some m' => Next (nextinstr (rs#SP <- v #X16 <- Vundef)) m'
+              end
+          | _ => Stuck
+          end
+      end
+  | Plabel lbl =>
+      Next (nextinstr rs) m
+  | Ploadsymbol rd id =>
+      Next (nextinstr (rs#rd <- (Genv.symbol_address ge id Ptrofs.zero))) m
+  | Pcvtsw2x rd r1 =>
+      Next (nextinstr (rs#rd <- (Val.longofint rs#r1))) m
+  | Pcvtuw2x rd r1 =>
+      Next (nextinstr (rs#rd <- (Val.longofintu rs#r1))) m
+  | Pcvtx2w rd =>
+      Next (nextinstr (rs#rd <- (Val.loword rs#rd))) m
+  | Pbtbl r tbl =>
+      match (rs#X16 <- Vundef)#r with
+      | Vint n =>
+          match list_nth_z tbl (Int.unsigned n) with
+          | None => Stuck
+          | Some lbl => goto_label f lbl (rs#X16 <- Vundef) m
+          end
+      | _ => Stuck
+      end
+  | Pcfi_rel_offset _ =>
+      Next (nextinstr rs) m
+  | Pbuiltin ef args res => Stuck    (**r treated specially below *)
+  (** The following instructions and directives are not generated directly
+      by Asmgen, so we do not model them. *)
+  | Pldp _ _ _
+  | Pstp _ _ _
+  | Pcls _ _ _
+  | Pclz _ _ _
+  | Prev _ _ _
+  | Prev16 _ _ _
+  | Prbit _ _ _
+  | Pfsqrt _ _ _
+  | Pfmadd _ _ _ _ _
+  | Pfmsub _ _ _ _ _
+  | Pfnmadd _ _ _ _ _
+  | Pfnmsub _ _ _ _ _
+  | Pfmax _ _ _ _
+  | Pfmin _ _ _ _
+  | Pnop
+  | Pcfi_adjust _ =>
+      Stuck
+  end.
 
 (** Translation of the LTL/Linear/Mach view of machine registers
   to the AArch64 view.  Note that no LTL register maps to [X16],
@@ -1212,7 +1203,7 @@ Inductive step: state -> trace -> state -> Prop :=
       rs PC = Vptr b ofs ->
       Genv.find_funct_ptr ge b = Some (Internal f) ->
       find_instr (Ptrofs.unsigned ofs) f.(fn_code) = Some i ->
-      exec_instr f i (Next rs m) = Next rs' m' ->
+      exec_instr f i rs m = Next rs' m' ->
       step (State rs m) E0 (State rs' m')
   | exec_step_builtin:
       forall b ofs f ef args res rs m vargs t vres rs' m',
@@ -1282,15 +1273,14 @@ Proof.
   intros. eapply C; eauto.
 Qed.
 
+Lemma semantics_determinate: forall p, determinate (semantics p).
+Proof.
 Ltac Equalities :=
   match goal with
   | [ H1: ?a = ?b, H2: ?a = ?c |- _ ] =>
       rewrite H1 in H2; inv H2; Equalities
   | _ => idtac
   end.
-
-Lemma semantics_determinate: forall p, determinate (semantics p).
-Proof.
   intros; constructor; simpl; intros.
 - (* determ *)
   inv H; inv H0; Equalities.
@@ -1328,616 +1318,3 @@ Definition data_preg (r: preg) : bool :=
   | SP => true
   | PC => false
   end.
-
-Lemma vptr_equality: forall b1 b2 o1 o2, b1=b2 /\ o1 = o2 -> Vptr b1 o1 = Vptr b2 o2.
-Proof. intros. destruct H. rewrite H. rewrite H0. reflexivity. Qed.
-
-Lemma inverse_vptr_equality: forall b1 b2 o1 o2,  Vptr b1 o1 = Vptr b2 o2 -> b1=b2 /\ o1 = o2.
-Proof. intros. inversion H. split; reflexivity. Qed.
-
-(* (* 
-(Val.offset_ptr (rs_i # rd0 <- (rs_i r0) PC) Ptrofs.one) *)
-Lemma invertible_increment: forall m_i1 m_i2 m_t1 m_t2 key delta b1 o1 b2 o2, Pregmap.get key m_i1 = Vptr b1 o1 -> Pregmap.get key m_i2 = Vptr b2 o2 -> m_t1 = Pregmap.set key (Val.offset_ptr (Pregmap.get key m_i1) delta) m_i1 -> m_t2 = Pregmap.set key (Val.offset_ptr (Pregmap.get key m_i2) delta) m_i2 -> Pregmap.get key m_t2 = Pregmap.get key m_t1 -> Pregmap.get key m_i1 = Pregmap.get key m_i2.
-Proof.
-intros.
-rewrite H1 in H3. rewrite H2 in H3. unfold Pregmap.get, Pregmap.set, Pregmap.elt_eq. unfold Pregmap.get, Pregmap.set, Pregmap.elt_eq in H, H0, H3. destruct PregEq.eq.  destruct (m_i1 key) eqn: Hmi1, (m_i2 key) eqn: Hmi2; try discriminate. simpl in H3. apply inverse_vptr_equality in H3. destruct H3. apply vptr_equality. split. rewrite <- H3. reflexivity. auto with va. simpl in H4. apply H3.   apply vptr_equality.
-Admitted.  *)
-
-Lemma outcome_equality: forall (rs1 rs2: regset)(m1 m2: mem),  Next rs1 m1 = Next rs2 m2 -> rs1 = rs2 /\ m1 = m2. 
-    Proof. intros. inversion H. split; reflexivity. Qed.
-
-Lemma inverse_outcome_equality: forall (rs1 rs2: regset)(m1 m2: mem), rs1 = rs2 /\ m1 = m2 -> Next rs1 m1 = Next rs2 m2.
-Proof. intros. destruct H. rewrite H. rewrite H0. reflexivity. Qed.
-
-(* need some way of abstracting 
-for a given instruction if an argument is a data source/data sink*)
-Inductive data_resource: Type :=
-    | SingleReg: preg -> data_resource
-    | SingleMemAddr: memory_chunk -> val -> data_resource.
-Definition data_res_eq (d1 d2: data_resource): Prop :=
-    match d1, d2 with
-    | SingleReg r1, SingleReg r2 => r1 = r2
-    | SingleMemAddr c1 a1, SingleMemAddr c2 a2 => c1 = c2 /\ a1 = a2
-    | _, _ => False
-    end.
-
-Definition iregz_same_resource (dr: data_resource) (r: ireg0) : Prop :=
-    match r with 
-    | RR0 r1 => data_res_eq dr (SingleReg r1) 
-    | XZR => False
-    end.
-    
-    
-Remark data_res_isomorphism: forall r, data_res_eq r r.
-Proof.
-    intros. destruct r. unfold data_res_eq. reflexivity. unfold data_res_eq. split; reflexivity. 
-Qed.
-
-Lemma symb_data_eq: forall (x y: data_resource), {x=y} + {x<>y}.
-Proof. decide equality. apply preg_eq. apply Val.eq. apply AST.chunk_eq.
-Qed.
-
-(* TODO Check if data resource d is an input for address a. Requires checking the regs of A*)
-Definition data_address_src(a: addressing) (d: data_resource) : Prop := 
-   match a with
-   | ADimm base n => data_res_eq d (SingleReg (preg_of_iregsp base))
-   | ADreg base r => data_res_eq d (SingleReg (preg_of_iregsp base)) \/  data_res_eq d (SingleReg r) 
-   | ADlsl base r n => data_res_eq d  ( SingleReg (preg_of_iregsp base)) \/ data_res_eq d (SingleReg r) 
-   | ADsxt base r n => data_res_eq d (SingleReg (preg_of_iregsp base)) \/ data_res_eq d (SingleReg r) 
-   | ADuxt base r n => data_res_eq d (SingleReg (preg_of_iregsp base)) \/ data_res_eq d (SingleReg r) 
-   | ADadr base id ofs => data_res_eq d (SingleReg (preg_of_iregsp base))
-   | ADpostincr base n => True (* not modeled in CompCert*) 
-   end.
-
-
-
- (* Check if data resource d is overwritten by a. Requires checking the evaluated expr*)
- Definition data_address_sink (a: addressing) (d: data_resource) (g: genv) (r: regset): Prop := 
-    match d with
-    | SingleMemAddr _ val => eval_addressing g a r = val
-    | _ => False
-    end.
-
-(* TODO: change all instances of NoResource to false? kinda based*)
-
-(* Get a proposition representing if an instruction has a dependency on dr*)
-Definition data_source(i: instruction) (dr: data_resource): Prop := 
-    match i with 
-   (* Jump to*)
-   | Pb lbl => False                                                    (**r branch *)
-   | Pbc c lbl  => data_res_eq dr (SingleReg (CR CZ))                                    (**r conditional branch *)
-   | Pbl id sg => data_res_eq dr (SingleReg PC)                                  (**r jump to function and link *)
-   | Pbs id sg => False                              (**r jump to function *)
-   | Pblr r sg  => data_res_eq dr (SingleReg PC)                                   (**r indirect jump and link *)
-   | Pbr r sg   => data_res_eq dr (SingleReg PC)                                   (**r indirect jump *)
-   | Pret r => False                                              (**r return *)
-   | Pcbnz sz r lbl    => data_res_eq dr (SingleReg r)                      (**r branch if not zero *)
-   | Pcbz sz r lbl => data_res_eq dr (SingleReg r)                         (**r branch if zero *)
-   | Ptbnz sz r n lbl   => data_res_eq dr (SingleReg r)               (**r branch if bit n is not zero *)
-   | Ptbz sz r n lbl => data_res_eq dr (SingleReg r)                  (**r branch if bit n is zero *)
-   (** Memory loads and stores *)
-   | Pldrw rd a => data_address_src a dr                             (**r load int32 *)
-   | Pldrw_a rd a => data_address_src a dr                                 (**r load int32 as any32 *)
-   | Pldrx rd a => data_address_src a dr                                  (**r load int64 *)
-   | Pldrx_a rd a => data_address_src a dr                                 (**r load int64 as any64 *)
-   | Pldrb sz rd a => data_address_src a dr                         (**r load int8, zero-extend *)
-   | Pldrsb sz rd a => data_address_src a dr                        (**r load int8, sign-extend *)
-   | Pldrh sz rd a => data_address_src a dr                        (**r load int16, zero-extend *)
-   | Pldrsh sz rd a => data_address_src a dr                        (**r load int16, sign-extend *)
-   | Pldrzw rd a  => data_address_src a dr                                  (**r load int32, zero-extend to int64 *)
-   | Pldrsw rd a => data_res_eq dr (SingleReg rd)                                 (**r load int32, sign-extend to int64 *)
-   | Pldp rd1 rd2 a => data_res_eq dr (SingleReg rd1) \/ data_res_eq dr (SingleReg rd2)                               (**r load two int64 *)
-   (** Stores *)
-   | Pstrw rs a => data_res_eq dr (SingleReg rs)                               (**r store int32 *)
-   | Pstrw_a rs a => data_res_eq dr (SingleReg rs)                                     (**r store int32 as any32 *)
-   | Pstrx rs a => data_res_eq dr (SingleReg rs)                                      (**r store int64 *)
-   | Pstrx_a rs a => data_res_eq dr (SingleReg rs)                                   (**r store int64 as any64 *)
-   | Pstrb rs a => data_res_eq dr (SingleReg rs)                                    (**r store int8 *)
-   | Pstrh rs a => data_res_eq dr (SingleReg rs)                                    (**r store int16 *)
-   | Pstp rs1 rs2 a => data_res_eq dr (SingleReg rs1)  \/ data_res_eq dr (SingleReg rs2)                               (**r store two int64 *)
-   (** Integer arithmetic, immediate *)
-   | Paddimm sz rd r1 n  => data_res_eq dr (SingleReg (preg_of_iregsp r1))            (**r addition *)
-   | Psubimm sz rd r1 n => data_res_eq dr (SingleReg (preg_of_iregsp r1))               (**r subtraction *)
-   | Pcmpimm sz r1 n => data_res_eq dr (SingleReg r1)                             (**r compare *)
-   | Pcmnimm sz r1 n => data_res_eq dr (SingleReg r1)                              (**r compare negative *)
-   (** Move integer register *)
-   | Pmov rd r1 => data_res_eq dr (SingleReg (preg_of_iregsp r1)) 
-   (** Logical, immediate *)
-   | Pandimm sz rd r1 n => iregz_same_resource dr r1                 (**r and *)
-   | Peorimm sz rd r1 n => iregz_same_resource dr r1                  (**r xor *)
-   | Porrimm sz rd r1 n => iregz_same_resource dr r1                  (**r or *)
-   | Ptstimm sz r1 n => data_res_eq dr (SingleReg r1)                             (**r and, then set flags *)
-   (** Move wide immediate *)
-   | Pmovz sz rd n pos  => False                (**r move [n << pos] to [rd] *)
-   | Pmovn sz rd n pos  => False                (**r move [NOT(n << pos)] to [rd] *)
-   | Pmovk sz rd n pos  => False                (**r insert 16 bits of [n] at [pos] in rd *)
-   (** PC-relative addressing *)
-   | Padrp rd id ofs => False                   (**r set [rd] to high address of [id + ofs] *)
-   | Paddadr rd r1 id ofs => data_res_eq dr (SingleReg r1)             (**r add the low address of [id + ofs] *)
-   (** Bit-field operations *)
-   | Psbfiz sz rd r1 r s => data_res_eq dr (SingleReg r1)           (**r sign extend and shift left *)
-   | Psbfx sz rd r1 r s => data_res_eq dr (SingleReg r1)           (**r shift right and sign extend *)
-   | Pubfiz sz rd r1 r s => data_res_eq dr (SingleReg r1)           (**r zero extend and shift left *)
-   | Pubfx sz rd r1 r s => data_res_eq dr (SingleReg r1)           (**r shift right and zero extend *)
-   (** Integer arithmetic, shifted register *)
-   | Padd sz rd r1 r2 s => iregz_same_resource dr r1 \/ data_res_eq dr (SingleReg r2)    (**r addition *)
-   | Psub sz rd r1 r2 s => iregz_same_resource dr r1 \/ data_res_eq dr (SingleReg r2)   (**r subtraction *)
-   | Pcmp sz r1 r2 s => iregz_same_resource dr r1 \/ data_res_eq dr (SingleReg r2)              (**r compare *)
-   | Pcmn sz r1 r2 s => iregz_same_resource dr r1 \/ data_res_eq dr (SingleReg r2)              (**r compare negative *)
-   (** Integer arithmetic, extending register *)
-   | Paddext rd r1 r2 x => data_res_eq dr (SingleReg r1) \/ data_res_eq dr (SingleReg r2)        (**r int64-int32 add *)
-   | Psubext rd r1 r2 x => data_res_eq dr (SingleReg r1) \/ data_res_eq dr (SingleReg r2)        (**r int64-int32 sub *)
-   | Pcmpext r1 r2 x => data_res_eq dr (SingleReg r1) \/ data_res_eq dr (SingleReg r2)                     (**r int64-int32 cmp *)
-   | Pcmnext r1 r2 x => data_res_eq dr (SingleReg r1) \/ data_res_eq dr (SingleReg r2)                       (**r int64-int32 cmn *)
-   (** Logical, shifted register *)
-   | Pand sz rd r1 r2 s => iregz_same_resource dr r1 \/ data_res_eq dr (SingleReg r2)   (**r and *)
-   | Pbic sz rd r1 r2 s => iregz_same_resource dr r1 \/ data_res_eq dr (SingleReg r2)   (**r and-not *)
-   | Peon sz rd r1 r2 s => iregz_same_resource dr r1 \/ data_res_eq dr (SingleReg r2)   (**r xor-not *)
-   | Peor sz rd r1 r2 s => iregz_same_resource dr r1 \/ data_res_eq dr (SingleReg r2)   (**r xor *)
-   | Porr sz rd r1 r2 s => iregz_same_resource dr r1 \/ data_res_eq dr (SingleReg r2)   (**r or *)
-   | Porn sz rd r1 r2 s => iregz_same_resource dr r1 \/ data_res_eq dr (SingleReg r2)   (**r or-not *)
-   | Ptst sz r1 r2 s => iregz_same_resource dr r1 \/ data_res_eq dr (SingleReg r2)                (**r and, then set flags *)
-   (** Variable shifts *)
-   | Pasrv sz rd r1 r2 => data_res_eq dr (SingleReg r1) \/ data_res_eq dr (SingleReg r2)                         (**r arithmetic right shift *)
-   | Plslv sz rd r1 r2 => data_res_eq dr (SingleReg r1) \/ data_res_eq dr (SingleReg r2)                         (**r left shift *)
-   | Plsrv sz rd r1 r2 => data_res_eq dr (SingleReg r1) \/ data_res_eq dr (SingleReg r2)                         (**r logical right shift *)
-   | Prorv sz rd r1 r2 => data_res_eq dr (SingleReg r1) \/ data_res_eq dr (SingleReg r2)                        (**r rotate right *)
-   (** Bit operations *)
-   | Pcls sz rd r1 => data_res_eq dr (SingleReg r1)                                    (**r count leading sign bits *)
-   | Pclz sz rd r1 => data_res_eq dr (SingleReg r1)                                     (**r count leading zero bits *)
-   | Prev sz rd r1 => data_res_eq dr (SingleReg r1)                                    (**r reverse bytes *)
-   | Prev16 sz rd r1 => data_res_eq dr (SingleReg r1)                                   (**r reverse bytes in each 16-bit word *)
-   | Prbit sz rd r1  => data_res_eq dr (SingleReg r1)                                   (**r reverse bits *)
-   (** Conditional data processing *)
-   | Pcsel rd r1 r2 c  => data_res_eq dr (SingleReg r1)  \/ data_res_eq dr (SingleReg r2)                      (**r int conditional move *)
-    (*TODO: anything more to handle conditions?*)
-   | Pcset rd c => False                               (**r set to 1/0 if cond is true/false *)
-   (*
-   | Pcsetm rd c                                   (**r set to -1/0 if cond is true/false *)
-   *)
-   (** Integer multiply/divide *)
-   | Pmadd sz rd r1 r2 r3 =>  data_res_eq dr (SingleReg r1) \/ data_res_eq dr (SingleReg r2) \/ iregz_same_resource dr r3              (**r multiply-add *)
-   | Pmsub sz rd r1 r2 r3 => data_res_eq dr (SingleReg r1) \/ data_res_eq dr (SingleReg r2) \/ iregz_same_resource dr r3            (**r multiply-sub *)
-   | Psmulh rd r1 r2 => data_res_eq dr (SingleReg r1) \/ data_res_eq dr (SingleReg r2)                                   (**r signed multiply high *)
-   | Pumulh rd r1 r2 => data_res_eq dr (SingleReg r1) \/ data_res_eq dr (SingleReg r2)                                   (**r unsigned multiply high *)
-   | Psdiv sz rd r1 r2 => data_res_eq dr (SingleReg r1) \/ data_res_eq dr (SingleReg r2)                       (**r signed division *)
-   | Pudiv sz rd r1 r2 => data_res_eq dr (SingleReg r1) \/ data_res_eq dr (SingleReg r2)                       (**r unsigned division *)
-   (** Floating-point loads and stores *)
-   | Pldrs rd a => data_address_src a dr                                   (**r load float32 (single precision) *)
-   | Pldrd rd a => data_address_src a dr                                  (**r load float64 (double precision) *)
-   | Pldrd_a rd a => data_address_src a dr                                (**r load float64 as any64 *)
-   | Pstrs rs a => data_res_eq dr (SingleReg rs)                                   (**r store float32 *)
-   | Pstrd rs a => data_res_eq dr (SingleReg rs)                                   (**r store float64 *)
-   | Pstrd_a rs a => data_res_eq dr (SingleReg rs)                                (**r store float64 as any64 *)
-   (** Floating-point move *)
-   | Pfmov rd r1 => data_res_eq dr (SingleReg r1) 
-   | Pfmovimms rd f  => False                                (**r load float32 constant *)
-   | Pfmovimmd rd f  => False                                  (**r load float64 constant *)
-   | Pfmovi fsz rd r1 => iregz_same_resource dr r1                         (**r copy int reg to FP reg *)
-   (** Floating-point conversions *)
-   | Pfcvtds rd r1  => data_res_eq dr (SingleReg r1)                                            (**r convert float32 to float64 *)
-   | Pfcvtsd rd r1  => data_res_eq dr (SingleReg r1)                                           (**r convert float64 to float32 *)
-   | Pfcvtzs isz fsz rd r1 => data_res_eq dr (SingleReg r1)            (**r convert float to signed int *)
-   | Pfcvtzu isz fsz rd r1 => data_res_eq dr (SingleReg r1)           (**r convert float to unsigned int *)
-   | Pscvtf fsz isz rd r1 => data_res_eq dr (SingleReg r1)             (**r convert signed int to float *)
-   | Pucvtf fsz isz rd r1 => data_res_eq dr (SingleReg r1)            (**r convert unsigned int to float *)
-   (** Floating-point arithmetic *)
-   | Pfabs sz rd r1 => data_res_eq dr (SingleReg r1)                                    (**r absolute value *)
-   | Pfneg sz rd r1 => data_res_eq dr (SingleReg r1)                                    (**r negation *)
-   | Pfsqrt sz rd r1 => data_res_eq dr (SingleReg r1)                                   (**r square root *)
-   | Pfadd sz rd r1 r2 => data_res_eq dr (SingleReg r1) \/ data_res_eq dr (SingleReg r2)                                 (**r addition *)
-   | Pfdiv sz rd r1 r2  => data_res_eq dr (SingleReg r1) \/ data_res_eq dr (SingleReg r2)                               (**r division *)
-   | Pfmul sz rd r1 r2  => data_res_eq dr (SingleReg r1)  \/ data_res_eq dr (SingleReg r2)                             (**r multiplication *)
-   | Pfnmul sz rd r1 r2 => data_res_eq dr (SingleReg r1)  \/ data_res_eq dr (SingleReg r2)                             (**r multiply-negate *)
-   | Pfsub sz rd r1 r2 => data_res_eq dr (SingleReg r1)   \/ data_res_eq dr (SingleReg r2)                              (**r subtraction *)
-   | Pfmadd sz rd r1 r2 r3 => data_res_eq dr (SingleReg r1) \/ data_res_eq dr (SingleReg r2) \/ data_res_eq dr (SingleReg r3)                            (**r [rd = r3 + r1 * r2] *)
-   | Pfmsub sz rd r1 r2 r3 => data_res_eq dr (SingleReg r1) \/ data_res_eq dr (SingleReg r2) \/ data_res_eq dr (SingleReg r3)                            (**r [rd = r3 - r1 * r2] *)
-   | Pfnmadd sz rd r1 r2 r3 => data_res_eq dr (SingleReg r1) \/ data_res_eq dr (SingleReg r2) \/ data_res_eq dr (SingleReg r3)                           (**r [rd = - r3 - r1 * r2] *)
-   | Pfnmsub sz rd r1 r2 r3 => data_res_eq dr (SingleReg r1) \/ data_res_eq dr (SingleReg r2) \/ data_res_eq dr (SingleReg r3)                           (**r [rd = - r3 + r1 * r2] *)
-   | Pfmax sz rd r1 r2 => data_res_eq dr (SingleReg r1) \/ data_res_eq dr (SingleReg r2)                                (**r maximum *)
-   | Pfmin sz rd r1 r2 => data_res_eq dr (SingleReg r1) \/ data_res_eq dr (SingleReg r2)                               (**r minimum *)
-   (** Floating-point comparison *)
-   | Pfcmp sz r1 r2 => data_res_eq dr (SingleReg r1) \/ data_res_eq dr (SingleReg r2)                                   (**r compare [r1] and [r2] *)
-   | Pfcmp0 sz r1 => data_res_eq dr (SingleReg r1)                                      (**r compare [r1] and [+0.0] *)
-   (** Floating-point conditional select *)
-   (*TODO: figure out cond*)
-   | Pfsel rd r1 r2 cond => data_res_eq dr (SingleReg r1) \/ data_res_eq dr (SingleReg r2)
-   (** Pseudo-instructions *)
-   | Pallocframe sz linkofs => False                              (**r allocate new stack frame *)
-   | Pfreeframe sz linkofs => False                               (**r deallocate stack frame and restore previous frame *)
-   | Plabel lbl => False                                                (**r define a code label *)
-   | Ploadsymbol rd id => False                                 (**r load the address of [id] *)
-   | Pcvtsw2x rd r1 => data_res_eq dr (SingleReg r1)                                 (**r sign-extend 32-bit int to 64-bit *)
-   | Pcvtuw2x rd r1 => data_res_eq dr (SingleReg r1)                                  (**r zero-extend 32-bit int to 64-bit *)
-   | Pcvtx2w rd => data_res_eq dr (SingleReg rd)                                                 (**r retype a 64-bit int as a 32-bit int *)
-   | Pbtbl r1 tbl  => False                              (**r N-way branch through a jump table *)
-   | Pbuiltin ef args res => False   (**r built-in function (pseudo) *)
-   | Pnop => False                                                             (**r no operation *)
-   | Pcfi_adjust ofs => False                                           (**r .cfi_adjust debug directive *)
-   | Pcfi_rel_offset ofs  => False                                       (**r .cfi_rel_offset debug directive *)
-   | Pincpc => data_res_eq dr (SingleReg PC) 
-    end.
-
-Definition data_sink(i: instruction) (dr: data_resource) (g: genv) (ers: regset): Prop := 
-    match i with
-    (*actual*)
-    (* Jump to*)
-    | Pb lbl => data_res_eq dr (SingleReg PC)                                                    (**r branch *)
-    | Pbc c lbl  => data_res_eq dr (SingleReg PC)                                    (**r conditional branch *)
-    | Pbl id sg => data_res_eq dr (SingleReg PC) \/ data_res_eq dr (SingleReg RA)                                    (**r jump to function and link *)
-    | Pbs id sg => data_res_eq dr (SingleReg PC)                                   (**r jump to function *)
-    | Pblr r sg  => data_res_eq dr (SingleReg PC)  \/ data_res_eq dr (SingleReg RA)                                (**r indirect jump and link *)
-    | Pbr r sg   => data_res_eq dr (SingleReg PC)                                   (**r indirect jump *)
-    | Pret r => data_res_eq dr (SingleReg PC)                                                     (**r return *)
-    | Pcbnz sz r lbl    => data_res_eq dr (SingleReg PC)                       (**r branch if not zero *)
-    | Pcbz sz r lbl => data_res_eq dr (SingleReg PC)                           (**r branch if zero *)
-    | Ptbnz sz r n lbl   => data_res_eq dr (SingleReg PC)               (**r branch if bit n is not zero *)
-    | Ptbz sz r n lbl => data_res_eq dr (SingleReg PC)                  (**r branch if bit n is zero *)
-    (** Memory loads and stores *)
-    | Pldrw rd a => data_res_eq dr (SingleReg rd)                                 (**r load int32 *)
-    | Pldrw_a rd a => data_res_eq dr (SingleReg rd)                                (**r load int32 as any32 *)
-    | Pldrx rd a => data_res_eq dr (SingleReg rd)                                 (**r load int64 *)
-    | Pldrx_a rd a => data_res_eq dr (SingleReg rd)                                (**r load int64 as any64 *)
-    | Pldrb sz rd a => data_res_eq dr (SingleReg (preg_of_iregsp rd))                        (**r load int8, zero-extend *)
-    | Pldrsb sz rd a => data_res_eq dr (SingleReg (preg_of_iregsp rd))                      (**r load int8, sign-extend *)
-    | Pldrh sz rd a => data_res_eq dr (SingleReg (preg_of_iregsp rd))                       (**r load int16, zero-extend *)
-    | Pldrsh sz rd a => data_res_eq dr (SingleReg (preg_of_iregsp rd))                      (**r load int16, sign-extend *)
-    | Pldrzw rd a  => data_res_eq dr (SingleReg rd)                                 (**r load int32, zero-extend to int64 *)
-    | Pldrsw rd a => data_res_eq dr (SingleReg rd)                                 (**r load int32, sign-extend to int64 *)
-    | Pldp rd1 rd2 a => data_res_eq dr (SingleReg rd1) \/ data_res_eq dr (SingleReg rd2)                               (**r load two int64 *)
-    (*TODO: check this works *)
-    (* explanation: check if r is a memory address and, if so, check if a stores in r. Can check by evaluating both??? *)
-    | Pstrw rs a => data_address_sink a dr g ers                                 (**r store int32 *)
-    | Pstrw_a rs a => data_address_sink a dr g ers                                  (**r store int32 as any32 *)
-    | Pstrx rs a => data_address_sink a dr g ers                                    (**r store int64 *)
-    | Pstrx_a rs a => data_address_sink a dr g ers                                  (**r store int64 as any64 *)
-    | Pstrb rs a => data_address_sink a dr g ers                                   (**r store int8 *)
-    | Pstrh rs a => data_address_sink a dr g ers                                   (**r store int16 *)
-    | Pstp rs1 rs2 a => data_address_sink a dr g ers                                (**r store two int64 *)
-    (** Integer arithmetic, immediate *)
-    | Paddimm sz rd r1 n  => data_res_eq dr (SingleReg (preg_of_iregsp rd))            (**r addition *)
-    | Psubimm sz rd r1 n => data_res_eq dr (SingleReg (preg_of_iregsp rd))               (**r subtraction *)
-    | Pcmpimm sz r1 n => data_res_eq dr (SingleReg (CR CZ))                             (**r compare *)
-    | Pcmnimm sz r1 n => data_res_eq dr (SingleReg (CR CZ))                              (**r compare negative *)
-    (** Move integer register *)
-    | Pmov rd r1 => data_res_eq dr (SingleReg (preg_of_iregsp rd)) 
-    (** Logical, immediate *)
-    | Pandimm sz rd r1 n => data_res_eq dr (SingleReg rd)                  (**r and *)
-    | Peorimm sz rd r1 n => data_res_eq dr (SingleReg rd)                  (**r xor *)
-    | Porrimm sz rd r1 n => data_res_eq dr (SingleReg (preg_of_iregsp rd))                  (**r or *)
-    | Ptstimm sz r1 n => data_res_eq dr (SingleReg (CR CZ))                             (**r and, then set flags *)
-    (** Move wide immediate *)
-    | Pmovz sz rd n pos  => data_res_eq dr (SingleReg rd)                     (**r move [n << pos] to [rd] *)
-    | Pmovn sz rd n pos  => data_res_eq dr (SingleReg rd)                     (**r move [NOT(n << pos)] to [rd] *)
-    | Pmovk sz rd n pos  => data_res_eq dr (SingleReg rd)                     (**r insert 16 bits of [n] at [pos] in rd *)
-    (** PC-relative addressing *)
-    | Padrp rd id ofs => data_res_eq dr (SingleReg rd)                        (**r set [rd] to high address of [id + ofs] *)
-    | Paddadr rd r1 id ofs => data_res_eq dr (SingleReg rd)             (**r add the low address of [id + ofs] *)
-    (** Bit-field operations *)
-    | Psbfiz sz rd r1 r s => data_res_eq dr (SingleReg rd)           (**r sign extend and shift left *)
-    | Psbfx sz rd r1 r s => data_res_eq dr (SingleReg rd)           (**r shift right and sign extend *)
-    | Pubfiz sz rd r1 r s => data_res_eq dr (SingleReg rd)           (**r zero extend and shift left *)
-    | Pubfx sz rd r1 r s => data_res_eq dr (SingleReg rd)           (**r shift right and zero extend *)
-    (** Integer arithmetic, shifted register *)
-    | Padd sz rd r1 r2 s => data_res_eq dr (SingleReg rd)    (**r addition *)
-    | Psub sz rd r1 r2 s => data_res_eq dr (SingleReg rd)   (**r subtraction *)
-    | Pcmp sz r1 r2 s => data_res_eq dr (SingleReg (CR CZ))              (**r compare *)
-    | Pcmn sz r1 r2 s => data_res_eq dr (SingleReg (CR CZ))              (**r compare negative *)
-    (** Integer arithmetic, extending register *)
-    | Paddext rd r1 r2 x => data_res_eq dr (SingleReg (preg_of_iregsp rd))        (**r int64-int32 add *)
-    | Psubext rd r1 r2 x => data_res_eq dr (SingleReg (preg_of_iregsp rd))        (**r int64-int32 sub *)
-    | Pcmpext r1 r2 x => data_res_eq dr (SingleReg (CR CZ))                      (**r int64-int32 cmp *)
-    | Pcmnext r1 r2 x => data_res_eq dr (SingleReg (CR CZ))                       (**r int64-int32 cmn *)
-    (** Logical, shifted register *)
-    | Pand sz rd r1 r2 s => data_res_eq dr (SingleReg rd)   (**r and *)
-    | Pbic sz rd r1 r2 s => data_res_eq dr (SingleReg rd)   (**r and-not *)
-    | Peon sz rd r1 r2 s => data_res_eq dr (SingleReg rd)   (**r xor-not *)
-    | Peor sz rd r1 r2 s => data_res_eq dr (SingleReg rd)   (**r xor *)
-    | Porr sz rd r1 r2 s => data_res_eq dr (SingleReg rd)   (**r or *)
-    | Porn sz rd r1 r2 s => data_res_eq dr (SingleReg rd)   (**r or-not *)
-    | Ptst sz r1 r2 s => data_res_eq dr (SingleReg (CR CZ))                (**r and, then set flags *)
-    (** Variable shifts *)
-    | Pasrv sz rd r1 r2 => data_res_eq dr (SingleReg rd)                         (**r arithmetic right shift *)
-    | Plslv sz rd r1 r2 => data_res_eq dr (SingleReg rd)                         (**r left shift *)
-    | Plsrv sz rd r1 r2 => data_res_eq dr (SingleReg rd)                         (**r logical right shift *)
-    | Prorv sz rd r1 r2 => data_res_eq dr (SingleReg rd)                        (**r rotate right *)
-    (** Bit operations *)
-    | Pcls sz rd r1 => data_res_eq dr (SingleReg rd)                                     (**r count leading sign bits *)
-    | Pclz sz rd r1 => data_res_eq dr (SingleReg rd)                                     (**r count leading zero bits *)
-    | Prev sz rd r1 => data_res_eq dr (SingleReg rd)                                    (**r reverse bytes *)
-    | Prev16 sz rd r1 => data_res_eq dr (SingleReg rd)                                   (**r reverse bytes in each 16-bit word *)
-    | Prbit sz rd r1  => data_res_eq dr (SingleReg rd)                                   (**r reverse bits *)
-    (** Conditional data processing *)
-    | Pcsel rd r1 r2 c  => data_res_eq dr (SingleReg rd)                     (**r int conditional move *)
-    | Pcset rd c => data_res_eq dr (SingleReg rd)                                     (**r set to 1/0 if cond is true/false *)
-    (*
-    | Pcsetm rd c                                   (**r set to -1/0 if cond is true/false *)
-    *)
-    (** Integer multiply/divide *)
-    | Pmadd sz rd r1 r2 r3 => data_res_eq dr (SingleReg rd)             (**r multiply-add *)
-    | Pmsub sz rd r1 r2 r3 => data_res_eq dr (SingleReg rd)             (**r multiply-sub *)
-    | Psmulh rd r1 r2 => data_res_eq dr (SingleReg rd)                                   (**r signed multiply high *)
-    | Pumulh rd r1 r2 => data_res_eq dr (SingleReg rd)                                    (**r unsigned multiply high *)
-    | Psdiv sz rd r1 r2 => data_res_eq dr (SingleReg rd)                        (**r signed division *)
-    | Pudiv sz rd r1 r2 => data_res_eq dr (SingleReg rd)                        (**r unsigned division *)
-    (** Floating-point loads and stores *)
-    | Pldrs rd a => data_res_eq dr (SingleReg rd)                                   (**r load float32 (single precision) *)
-    | Pldrd rd a => data_res_eq dr (SingleReg rd)                                  (**r load float64 (double precision) *)
-    | Pldrd_a rd a => data_res_eq dr (SingleReg rd)                                (**r load float64 as any64 *)
-    | Pstrs rs a => data_address_sink a dr g ers                                   (**r store float32 *)
-    | Pstrd rs a => data_address_sink a dr g ers                                   (**r store float64 *)
-    | Pstrd_a rs a => data_address_sink a dr g ers                                (**r store float64 as any64 *)
-    (** Floating-point move *)
-    | Pfmov rd r1 => data_res_eq dr (SingleReg rd) 
-    | Pfmovimms rd f  => data_res_eq dr (SingleReg rd)                                (**r load float32 constant *)
-    | Pfmovimmd rd f  => data_res_eq dr (SingleReg rd)                                  (**r load float64 constant *)
-    | Pfmovi fsz rd r1 => data_res_eq dr (SingleReg rd)                         (**r copy int reg to FP reg *)
-    (** Floating-point conversions *)
-    | Pfcvtds rd r1  => data_res_eq dr (SingleReg rd)                                            (**r convert float32 to float64 *)
-    | Pfcvtsd rd r1  => data_res_eq dr (SingleReg rd)                                           (**r convert float64 to float32 *)
-    | Pfcvtzs isz fsz rd r1 => data_res_eq dr (SingleReg rd)            (**r convert float to signed int *)
-    | Pfcvtzu isz fsz rd r1 => data_res_eq dr (SingleReg rd)           (**r convert float to unsigned int *)
-    | Pscvtf fsz isz rd r1 => data_res_eq dr (SingleReg rd)             (**r convert signed int to float *)
-    | Pucvtf fsz isz rd r1 => data_res_eq dr (SingleReg rd)            (**r convert unsigned int to float *)
-    (** Floating-point arithmetic *)
-    | Pfabs sz rd r1 => data_res_eq dr (SingleReg rd)                                    (**r absolute value *)
-    | Pfneg sz rd r1 => data_res_eq dr (SingleReg rd)                                    (**r negation *)
-    | Pfsqrt sz rd r1 => data_res_eq dr (SingleReg rd)                                   (**r square root *)
-    | Pfadd sz rd r1 r2 => data_res_eq dr (SingleReg rd)                                (**r addition *)
-    | Pfdiv sz rd r1 r2  => data_res_eq dr (SingleReg rd)                                (**r division *)
-    | Pfmul sz rd r1 r2  => data_res_eq dr (SingleReg rd)                               (**r multiplication *)
-    | Pfnmul sz rd r1 r2 => data_res_eq dr (SingleReg rd)                               (**r multiply-negate *)
-    | Pfsub sz rd r1 r2 => data_res_eq dr (SingleReg rd)                                 (**r subtraction *)
-    | Pfmadd sz rd r1 r2 r3 => data_res_eq dr (SingleReg rd)                             (**r [rd = r3 + r1 * r2] *)
-    | Pfmsub sz rd r1 r2 r3 => data_res_eq dr (SingleReg rd)                             (**r [rd = r3 - r1 * r2] *)
-    | Pfnmadd sz rd r1 r2 r3 => data_res_eq dr (SingleReg rd)                            (**r [rd = - r3 - r1 * r2] *)
-    | Pfnmsub sz rd r1 r2 r3 => data_res_eq dr (SingleReg rd)                           (**r [rd = - r3 + r1 * r2] *)
-    | Pfmax sz rd r1 r2 => data_res_eq dr (SingleReg rd)                                (**r maximum *)
-    | Pfmin sz rd r1 r2 => data_res_eq dr (SingleReg rd)                                (**r minimum *)
-    (** Floating-point comparison *)
-    | Pfcmp sz r1 r2 => data_res_eq dr (SingleReg (CR CZ))                                   (**r compare [r1] and [r2] *)
-    | Pfcmp0 sz r1 => data_res_eq dr (SingleReg (CR CZ))                                      (**r compare [r1] and [+0.0] *)
-    (** Floating-point conditional select *)
-    | Pfsel rd r1 r2 cond => data_res_eq dr (SingleReg rd) 
-    (** Pseudo-instructions *)
-    | Pallocframe sz linkofs => False                            (**r allocate new stack frame *)
-    | Pfreeframe sz linkofs => False                             (**r deallocate stack frame and restore previous frame *)
-    | Plabel lbl => False                                              (**r define a code label *)
-    | Ploadsymbol rd id => data_res_eq dr (SingleReg rd)                                (**r load the address of [id] *)
-    | Pcvtsw2x rd r1 => data_res_eq dr (SingleReg rd)                                    (**r sign-extend 32-bit int to 64-bit *)
-    | Pcvtuw2x rd r1 => data_res_eq dr (SingleReg rd)                                    (**r zero-extend 32-bit int to 64-bit *)
-    | Pcvtx2w rd => data_res_eq dr (SingleReg rd)                                                 (**r retype a 64-bit int as a 32-bit int *)
-    | Pbtbl r1 tbl  => False                            (**r N-way branch through a jump table *)
-    | Pbuiltin ef args res => False (**r built-in function (pseudo) *)
-    | Pnop => False                                                           (**r no operation *)
-    | Pcfi_adjust ofs => False                                         (**r .cfi_adjust debug directive *)
-    | Pcfi_rel_offset ofs  => False                                     (**r .cfi_rel_offset debug directive *)
-    | Pincpc => data_res_eq dr (SingleReg PC) 
-end.
-
-
-
-Definition data_dependence(i1 i2: instruction) g rs: Prop :=
-    (exists r, data_sink i1 r g rs /\ data_source i2 r) \/ (exists r, data_sink i2 r g rs /\ data_source i1 r) \/ (exists r, data_sink i2 r g rs /\ data_sink i1 r g rs).
-
-
-Remark not_or_and : forall A B : Prop, ~(A \/ B) -> ~A /\ ~B.
-Proof.
-  intros A B H. split.
-    - intro. apply H. left. assumption.
-    - intro. apply H. right. assumption.
-Qed.
-
-Remark not_or_or_and : forall A B C : Prop, ~(A \/ B \/ C) -> ~A /\ ~B /\ ~C.
-Proof.
-  intros A B C H. split; [|split].
-  - intro HA. apply H. left. assumption.
-  - intro HB. apply H. right. left. assumption.
-  - intro HC. apply H. right. right. assumption.
-Qed.
-
-Lemma hazard_elimination_identity: forall r1, ~(exists r2: data_resource, data_res_eq r2 r1 /\ True)  -> False.
-Proof. intros. apply H. exists r1. split. apply data_res_isomorphism. reflexivity. Qed.
-
-Lemma hazard_elimination: forall (d: data_resource), ~ (exists r : data_resource, data_res_eq r (d) /\ data_res_eq r (d)) -> False.
-Proof. intros. apply H. exists d. split; apply data_res_isomorphism. 
-Qed.
-
-
- Remark regs_are_different_resources: forall r1 r2, ~
- (exists r : data_resource, data_res_eq r (SingleReg r1) /\ data_res_eq r (SingleReg r2)) -> r1 <> r2.
- Proof.
- unfold not. intros. apply H. exists (SingleReg r1). 
- split. try apply data_res_isomorphism. 
-rewrite <- H0; apply data_res_isomorphism.
-Qed.
-
-Remark resources_are_different_resources: forall r1 r2,  ~
- (exists r : data_resource, data_res_eq r r1 /\ data_res_eq r r2) ->  r1 <> r2.
- Proof.
- unfold not. intros. apply H. exists r1. 
- split. try apply data_res_isomorphism. auto. 
-  try (rewrite <- H0; apply data_res_isomorphism).
-Qed.
-
-Remark VInt_eq: forall i1 i2, Vint i1 = Vint i2 -> i1 = i2.
-Proof. intros. inv H. reflexivity. Qed.
-
-(* Theorem reorder: forall  g (f: function) (i1 i2: instruction)  (rs_i rs_t1 rs_t2 rs_f: regset)  (m_i m_t1 m_t2 m_f: mem), ~data_dependence i1 i2 g rs_i -> exec_instr g f i1 rs_i m_i = Next rs_t1 m_t1 -> exec_instr g f i2 rs_i m_i = Next rs_t2 m_t2 -> exec_instr g f i2 rs_t1 m_t1 = Next rs_f m_f -> exec_instr g f i1 rs_t2 m_t2 = Next rs_f m_f. *)
-(* Theorem reorder: forall g (f: function) (i1 i2: instruction) (rs_i: regset) (m_i: mem), ~data_dependence i1 i2 g rs_i -> i1 = exec_instr g f i2 (exec_instr g f i1 (Next rs_i m_i)) = exec_instr g f i1 (exec_instr g f i2 (Next rs_i m_i)). *)
-
-
-(** ** Simplify matches when possible *)
-
-Ltac simpl_match :=
-  let repl_match_goal d d' :=
-      replace d with d';
-      lazymatch goal with
-      | [ |- context[match d' with _ => _ end] ] => fail
-      | _ => idtac
-      end in
-  let repl_match_hyp H d d' :=
-      replace d with d' in H;
-      lazymatch type of H with
-      | context[match d' with _ => _ end] => fail
-      | _ => idtac
-      end in
-  match goal with
-  | [ Heq: ?d = ?d' |- context[match ?d with _ => _ end] ] =>
-    repl_match_goal d d'
-  | [ Heq: ?d' = ?d |- context[match ?d with _ => _ end] ] =>
-    repl_match_goal d d'
-  | [ Heq: ?d = ?d', H: context[match ?d with _ => _ end] |- _ ] =>
-    repl_match_hyp H d d'
-  | [ Heq: ?d' = ?d, H: context[match ?d with _ => _ end] |- _ ] =>
-    repl_match_hyp H d d'
-  end.
-
-(** ** Find and destruct matches *)
-
-Ltac destruct_matches_in e :=
-  lazymatch e with
-  | context[match ?d with | _ => _ end] =>
-    destruct_matches_in d
-  | _ => destruct e eqn:?; intros
-  end.
-
-Ltac destruct_all_matches :=
-  repeat (try simpl_match;
-          try match goal with
-              | [ |- context[match ?d with | _ => _ end] ] =>
-                destruct_matches_in d
-              | [ H: context[match ?d with | _ => _ end] |- _ ] =>
-                destruct_matches_in d
-              end);
-  subst;
-  try congruence;
-  auto.
-
-Ltac destruct_nongoal_matches :=
-  repeat (try simpl_match;
-           try match goal with
-           | [ H: context[match ?d with | _ => _ end] |- _ ] =>
-             destruct_matches_in d
-               end);
-  subst;
-  try congruence;
-  auto.
-
-Ltac destruct_goal_matches :=
-  repeat (try simpl_match;
-           match goal with
-           | [ |- context[match ?d with | _ => _ end] ] =>
-              destruct_matches_in d
-           end);
-  try congruence;
-  auto.
-
-Ltac destruct_tuple :=
-  match goal with
-  | [ H: context[let '(a, b) := ?p in _] |- _ ] =>
-    let a := fresh a in
-    let b := fresh b in
-    destruct p as [a b]
-  | [ |- context[let '(a, b) := ?p in _] ] =>
-    let a := fresh a in
-    let b := fresh b in
-    destruct p as [a b]
-  end.
-
-Tactic Notation "destruct" "matches" "in" "*" := destruct_all_matches.
-Tactic Notation "destruct" "matches" "in" "*|-" := destruct_nongoal_matches.
-Tactic Notation "destruct" "matches" := destruct_goal_matches.
-
-Ltac Super_Equalities :=
-  match goal with
-  | [ H_gso: ?a # ?b <- (?a ?c) ?d = ?e |- _ ] =>
-    rewrite -> Pregmap.gso in H_gso; Equalities
-  | [ H1: Vint ?a = Vint ?b, H2: Vint ?a = Vint ?c |- _ ] =>
-    rewrite H1 in H2; apply VInt_eq; Equalities
-  | [ H1: ?a = ?b, H2: ?a = ?c |- _ ] =>
-      rewrite H1 in H2; inv H2; Equalities
-  | [ H_destroy: ?a = ?b |- _] => subst a; Equalities
-  | _ => idtac
-  end.
-
-
-Theorem reorder: forall g (f: function) arg11 arg12 (i2: instruction) (rs_i: regset) (m_i: mem), ~data_dependence (Pmov arg11 arg12) i2 g rs_i -> exec_instr g f i2  (exec_instr g f (Pmov arg11 arg12)  (Next rs_i m_i)) = exec_instr g f (Pmov arg11 arg12)  (exec_instr g f i2  (Next rs_i m_i)).
-Proof. intros. 
-(* Definition unwrapping*)
-unfold data_dependence in H. unfold data_sink, data_source in H. apply not_or_or_and in H; destruct H; destruct H0. destruct i2.
-(* unfold data_dependence in H. unfold data_sink, data_source in H. destruct i1. destruct i2; apply not_or_or_and in H; destruct H; destruct H0; *)
-(* Remove data hazards that hit the same singleton register (eg PC, CR)*)
-try (apply hazard_elimination in H1;  contradiction +  unfold not;  intros;  discriminate H2);
-try (apply hazard_elimination in H;  contradiction +  unfold not;  intros;  discriminate H2);
-try (apply hazard_elimination in H0;  contradiction +  unfold not;  intros;  discriminate H2);
-
-
-
-(* Remove data hazards that hit True - maybe WIP?*)
-try (apply hazard_elimination_identity in H; contradiction + unfold not; intros; discriminate H2);
-
-try (apply hazard_elimination_identity in H0; contradiction + unfold not; intros; discriminate H2);
-
-try (apply hazard_elimination_identity in H1; contradiction + unfold not; intros; discriminate H2); auto;
-
-auto;
-
-(*Prove data vals different*)
-(* apply regs_are_different_resources in H1 || clear H1; apply regs_are_different_resources in H0 || clear H0; apply regs_are_different_resources in H || clear H; *)
-try apply regs_are_different_resources; try apply regs_are_different_resources in H0; try apply regs_are_different_resources in H;  
-unfold exec_instr; unfold nextinstr; unfold goto_label; unfold eval_testcond; destruct matches; auto; 
-(* Changing the order will not change the end result (Stuck/Next)*)
-Super_Equalities; auto.
-
-(* 
-(*breakdown mov*)
-
-
-(* Expression should be in the form Next ... = Next...*)
--apply inverse_outcome_equality; split. rewrite -> Pregmap.gso. rewrite -> Heqv in Heqv0. inversion Heqv0. apply Pregmap.gscsc. auto. auto. auto.
-- rewrite -> Pregmap.gso in Heqv0. rewrite -> Heqv0 in Heqv2. discriminate. assumption.
-
-
-(* 
-try (rewrite -> Pregmap.gso in Heqv; rewrite -> Heqv in Heqv0; try discriminate + assumption). Qed.
-
-
-(*breakdown goto*)
-unfold goto_label. destruct matches; rewrite -> Pregmap.gso in Heqv; try rewrite -> Heqv in Heqv0; try discriminate;
-try apply regs_are_different_resources in H1; try apply regs_are_different_resources in H0; try apply regs_are_different_resources in H; auto.
-
-apply inverse_outcome_equality. split. rewrite -> Pregmap.gso. inversion Heqv0. rewrite <- H3. apply Pregmap.gscsc. assumption. auto. reflexivity. 
-
-
-
-contradiction.
-destruct (label_pos lbl 0 (fn_code f)); try reflexivity.  try rewrite -> Pregmap.gso; try destruct (rs_i PC); try reflexivity; try (apply inverse_outcome_equality; rewrite -> Pregmap.gso; try split; try apply Pregmap.gscsc);
-
-
-(*breakdown testcond*)
-unfold eval_testcond.  destruct c;  try rewrite -> Pregmap.gso.
-
-
-(*breakdown exec_add*)
-
-(*breakdown exec_load*)
-
-
-auto.  try apply regs_are_different_resources in H1. apply regs_are_different_resources in H0. auto.
-inversion H0. unfold nextinstr. rewrite H2. reflexivity.
-unfold nextinstr. split. Unset Printing Notations.  rewrite -> Pregmap.gso.  rewrite -> Pregmap.gso. apply Pregmap.gscsc. assumption. auto. auto. reflexivity. Qed.
-
-apply regs_are_different_resources in H, H0, H1.
-(*solves Pmov*)
-unfold exec_instr. apply inverse_outcome_equality. unfold nextinstr. split. Unset Printing Notations.  rewrite -> Pregmap.gso.  rewrite -> Pregmap.gso. apply Pregmap.gscsc. assumption. auto. auto. reflexivity. Qed.  *)
-(* 
- unfold exec_instr. unfold goto_label. unfold exec_load.
-  destruct (rs_i PC). destruct (label_pos lbl 0 (fn_code f)).
- destruct (Mem.loadv Mint32 m (eval_addressing g a rs)).  inversion H2.
- destruct (Mem.loadv Mint32 m_i (eval_addressing g a rs_i)). inversion H1. unfold nextinstr in H6, H8.
- destruct (label_pos lbl 0 (fn_code f)). destruct (rs_i PC); try discriminate. inversion H0. unfold nextinstr. rewrite -> H8. 
- 
- destruct (rs_i # rd <- v0 PC); try discriminate. contradiction. unfold eval_addressing in H1, H2. *)
-
-Qed.
