aarch64/Asm_MemSim.v
@@ -1,0 +1,1805 @@
+(* *********************************************************************)
+(*                                                                     *)
+(*              The Compcert verified compiler                         *)
+(*                                                                     *)
+(*         Xavier Leroy, Collège de France and INRIA Paris             *)
+(*                                                                     *)
+(*  Copyright Institut National de Recherche en Informatique et en     *)
+(*  Automatique.  All rights reserved.  This file is distributed       *)
+(*  under the terms of the INRIA Non-Commercial License Agreement.     *)
+(*                                                                     *)
+(* *********************************************************************)
+
+(** Abstract syntax and semantics for AArch64 assembly language *)
+
+Require Import Coqlib Zbits Maps.
+Require Import AST Integers Floats.
+Require Import Values Memory Events Globalenvs Smallstep.
+Require Import Locations Conventions Asm.
+Require Import Coq.Lists.List.
+Import ListNotations.
+Require Stacklayout.
+
+(** * Abstract syntax *)
+
+
+Definition processor_id := Z.
+Definition processor_reg := (processor_id * preg) % type.
+(* 
+Definition preg_uri: Type := (processor_id * preg) % type.
+Definition ireg_uri: Type := (processor_id * ireg) % type.
+Definition freg_uri: Type := (processor_id * freg) % type. *)
+(* 
+Definition preg_comp_to_uri: (processor_id * preg) % type -> preg_uri := fun x => x.
+
+Coercion preg_comp_to_uri: (processor_id * preg) % type >-> preg_uri.
+
+Inductive processor_reg : Type :=
+ | preg_to_proc_reg: preg_uri -> processor_reg
+ | ireg_to_proc_reg: ireg_uri -> processor_reg
+ | freg_to_proc_reg: freg_uri -> processor_reg. 
+
+
+Coercion preg_to_proc_reg: preg_uri>-> processor_reg.
+Coercion ireg_to_proc_reg: ireg_uri>-> processor_reg.
+Coercion freg_to_proc_reg: freg_uri>-> processor_reg. *)
+
+Remark pr_eq:
+  forall (r1 r2: processor_reg), {r1 = r2} + {r1 <> r2}.
+Proof.
+    (* decide equality. destruct p; destruct p0; decide equality. apply preg_eq. apply Z.eq_dec.
+    decide equality. destruct p. apply ireg_eq; destruct a; apply ireg_eq. apply ireg_eq.
+    decide equality. apply Z.eq_dec.
+    decide equality. apply freg_eq. apply Z.eq_dec.  *)
+
+    decide equality. apply preg_eq. apply Z.eq_dec.
+Qed.
+
+Remark pr_eq_identity:
+    forall (r: processor_reg), r = r.
+Proof. reflexivity. Qed.
+
+Module PREq.
+  Definition t := processor_reg.
+  Definition eq := pr_eq.
+End PREq. 
+
+
+
+Module PRmap := EMap(PREq).
+
+Inductive instruction: Type :=
+  (** Branches *)
+  | Pb (lbl: label) (pid: processor_id)                                            (**r branch *)
+  | Pbc (c: testcond) (lbl: label) (pid: processor_id)                             (**r conditional branch *)
+  | Pbl (id: ident) (sg: signature) (pid: processor_id)                            (**r jump to function and link *)
+  | Pbs (id: ident) (sg: signature) (pid: processor_id)                            (**r jump to function *)
+  | Pblr (r: ireg) (sg: signature) (pid: processor_id)                             (**r indirect jump and link *)
+  | Pbr (r: ireg) (sg: signature) (pid: processor_id)                              (**r indirect jump *)
+  | Pret (r: ireg) (pid: processor_id)                                             (**r return *)
+  | Pcbnz (sz: isize) (r: ireg) (lbl: label) (pid: processor_id)                   (**r branch if not zero *)
+  | Pcbz (sz: isize) (r: ireg) (lbl: label) (pid: processor_id)                    (**r branch if zero *)
+  | Ptbnz (sz: isize) (r: ireg) (n: int) (lbl: label) (pid: processor_id)          (**r branch if bit n is not zero *)
+  | Ptbz (sz: isize) (r: ireg) (n: int) (lbl: label) (pid: processor_id)           (**r branch if bit n is zero *)
+  (** Memory loads and stores *)
+  | Pldrw (rd: ireg) (a: addressing) (pid: processor_id)                           (**r load int32 *)
+  | Pldrw_a (rd: ireg) (a: addressing) (pid: processor_id)                         (**r load int32 as any32 *)
+  | Pldrx (rd: ireg) (a: addressing) (pid: processor_id)                           (**r load int64 *)
+  | Pldrx_a (rd: ireg) (a: addressing) (pid: processor_id)                         (**r load int64 as any64 *)
+  | Pldrb (sz: isize) (rd: ireg) (a: addressing) (pid: processor_id)               (**r load int8, zero-extend *)
+  | Pldrsb (sz: isize) (rd: ireg) (a: addressing) (pid: processor_id)              (**r load int8, sign-extend *)
+  | Pldrh (sz: isize) (rd: ireg) (a: addressing) (pid: processor_id)               (**r load int16, zero-extend *)
+  | Pldrsh (sz: isize) (rd: ireg) (a: addressing) (pid: processor_id)              (**r load int16, sign-extend *)
+  | Pldrzw (rd: ireg) (a: addressing) (pid: processor_id)                          (**r load int32, zero-extend to int64 *)
+  | Pldrsw (rd: ireg) (a: addressing) (pid: processor_id)                          (**r load int32, sign-extend to int64 *)
+  | Pldp (rd1 rd2: ireg) (a: addressing) (pid: processor_id)                        (**r load two int64 *)
+  | Pstrw (rs: ireg) (a: addressing) (pid: processor_id)                           (**r store int32 *)
+  | Pstrw_a (rs: ireg) (a: addressing) (pid: processor_id)                         (**r store int32 as any32 *)
+  | Pstrx (rs: ireg) (a: addressing) (pid: processor_id)                           (**r store int64 *)
+  | Pstrx_a (rs: ireg) (a: addressing) (pid: processor_id)                         (**r store int64 as any64 *)
+  | Pstrb (rs: ireg) (a: addressing) (pid: processor_id)                           (**r store int8 *)
+  | Pstrh (rs: ireg) (a: addressing) (pid: processor_id)                           (**r store int16 *)
+  | Pstp (rs1 rs2: ireg) (a: addressing) (pid: processor_id)                       (**r store two int64 *)
+  (** Integer arithmetic, immediate *)
+  | Paddimm (sz: isize) (rd: iregsp) (r1: iregsp) (n: Z) (pid: processor_id)       (**r addition *)
+  | Psubimm (sz: isize) (rd: iregsp) (r1: iregsp) (n: Z) (pid: processor_id)       (**r subtraction *)
+  | Pcmpimm (sz: isize) (r1: ireg) (n: Z) (pid: processor_id)                      (**r compare *)
+  | Pcmnimm (sz: isize) (r1: ireg) (n: Z) (pid: processor_id)                      (**r compare negative *)
+  (** Move integer register *)
+  | Pmov (rd: iregsp) (r1: iregsp) (pid: processor_id) 
+  (** Logical, immediate *)
+  | Pandimm (sz: isize) (rd: ireg) (r1: ireg0) (n: Z) (pid: processor_id)          (**r and *)
+  | Peorimm (sz: isize) (rd: ireg) (r1: ireg0) (n: Z) (pid: processor_id)          (**r xor *)
+  | Porrimm (sz: isize) (rd: ireg) (r1: ireg0) (n: Z) (pid: processor_id)          (**r or *)
+  | Ptstimm (sz: isize) (r1: ireg) (n: Z) (pid: processor_id)                      (**r and, then set flags *)
+  (** Move wide immediate *)
+  | Pmovz (sz: isize) (rd: ireg) (n: Z) (pos: Z) (pid: processor_id)               (**r move [n << pos] to [rd] *)
+  | Pmovn (sz: isize) (rd: ireg) (n: Z) (pos: Z) (pid: processor_id)               (**r move [NOT(n << pos)] to [rd] *)
+  | Pmovk (sz: isize) (rd: ireg) (n: Z) (pos: Z) (pid: processor_id)               (**r insert 16 bits of [n] at [pos] in rd *)
+  (** PC-relative addressing *)
+  | Padrp (rd: ireg) (id: ident) (ofs: ptrofs) (pid: processor_id)                 (**r set [rd] to high address of [id + ofs] *)
+  | Paddadr (rd: ireg) (r1: ireg) (id: ident) (ofs: ptrofs) (pid: processor_id)    (**r add the low address of [id + ofs] *)
+  (** Bit-field operations *)
+  | Psbfiz (sz: isize) (rd: ireg) (r1: ireg) (r: int) (s: Z) (pid: processor_id)   (**r sign extend and shift left *)
+  | Psbfx (sz: isize) (rd: ireg) (r1: ireg) (r: int) (s: Z) (pid: processor_id)    (**r shift right and sign extend *)
+  | Pubfiz (sz: isize) (rd: ireg) (r1: ireg) (r: int) (s: Z) (pid: processor_id)   (**r zero extend and shift left *)
+  | Pubfx (sz: isize) (rd: ireg) (r1: ireg) (r: int) (s: Z) (pid: processor_id)    (**r shift right and zero extend *)
+  (** Integer arithmetic, shifted register *)
+  | Padd (sz: isize) (rd: ireg) (r1: ireg0) (r2: ireg) (s: shift_op) (pid: processor_id)  (**r addition *)
+  | Psub (sz: isize) (rd: ireg) (r1: ireg0) (r2: ireg) (s: shift_op) (pid: processor_id)  (**r subtraction *)
+  | Pcmp (sz: isize) (r1: ireg0) (r2: ireg) (s: shift_op) (pid: processor_id)      (**r compare *)
+  | Pcmn (sz: isize) (r1: ireg0) (r2: ireg) (s: shift_op) (pid: processor_id)      (**r compare negative *)
+  (** Integer arithmetic, extending register *)
+  | Paddext (rd: iregsp) (r1: iregsp) (r2: ireg) (x: extend_op) (pid: processor_id)(**r int64-int32 add *)
+  | Psubext (rd: iregsp) (r1: iregsp) (r2: ireg) (x: extend_op) (pid: processor_id)(**r int64-int32 sub *)
+  | Pcmpext (r1: ireg) (r2: ireg) (x: extend_op) (pid: processor_id)               (**r int64-int32 cmp *)
+  | Pcmnext (r1: ireg) (r2: ireg) (x: extend_op) (pid: processor_id)               (**r int64-int32 cmn *)
+  (** Logical, shifted register *)
+  | Pand (sz: isize) (rd: ireg) (r1: ireg0) (r2: ireg) (s: shift_op) (pid: processor_id)  (**r and *)
+  | Pbic (sz: isize) (rd: ireg) (r1: ireg0) (r2: ireg) (s: shift_op) (pid: processor_id)  (**r and-not *)
+  | Peon (sz: isize) (rd: ireg) (r1: ireg0) (r2: ireg) (s: shift_op) (pid: processor_id)  (**r xor-not *)
+  | Peor (sz: isize) (rd: ireg) (r1: ireg0) (r2: ireg) (s: shift_op) (pid: processor_id)  (**r xor *)
+  | Porr (sz: isize) (rd: ireg) (r1: ireg0) (r2: ireg) (s: shift_op) (pid: processor_id)  (**r or *)
+  | Porn (sz: isize) (rd: ireg) (r1: ireg0) (r2: ireg) (s: shift_op) (pid: processor_id)   (**r or-not *)
+  | Ptst (sz: isize) (r1: ireg0) (r2: ireg) (s: shift_op) (pid: processor_id)      (**r and, then set flags *)
+  (** Variable shifts *)
+  | Pasrv (sz: isize) (rd: ireg) (r1 r2: ireg) (pid: processor_id)                 (**r arithmetic right shift *)
+  | Plslv (sz: isize) (rd: ireg) (r1 r2: ireg) (pid: processor_id)                 (**r left shift *)
+  | Plsrv (sz: isize) (rd: ireg) (r1 r2: ireg) (pid: processor_id)                 (**r logical right shift *)
+  | Prorv (sz: isize) (rd: ireg) (r1 r2: ireg) (pid: processor_id)                 (**r rotate right *)
+  (** Bit operations *)
+  | Pcls (sz: isize) (rd r1: ireg) (pid: processor_id)                             (**r count leading sign bits *)
+  | Pclz (sz: isize) (rd r1: ireg) (pid: processor_id)                             (**r count leading zero bits *)
+  | Prev (sz: isize) (rd r1: ireg) (pid: processor_id)                             (**r reverse bytes *)
+  | Prev16 (sz: isize) (rd r1: ireg) (pid: processor_id)                           (**r reverse bytes in each 16-bit word *)
+  | Prbit (sz: isize) (rd r1: ireg) (pid: processor_id)                            (**r reverse bits *)
+  (** Conditional data processing *)
+  | Pcsel (rd: ireg) (r1 r2: ireg) (c: testcond) (pid: processor_id)               (**r int conditional move *)
+  | Pcset (rd: ireg) (c: testcond) (pid: processor_id)                             (**r set to 1/0 if cond is true/false *)
+(*
+  | Pcsetm (rd: ireg) (c: testcond) (pid: processor_id)                            (**r set to -1/0 if cond is true/false *)
+*)
+  (** Integer multiply/divide *)
+  | Pmadd (sz: isize) (rd: ireg) (r1 r2: ireg) (r3: ireg0) (pid: processor_id)     (**r multiply-add *)
+  | Pmsub (sz: isize) (rd: ireg) (r1 r2: ireg) (r3: ireg0) (pid: processor_id)     (**r multiply-sub *)
+  | Psmulh (rd: ireg) (r1 r2: ireg) (pid: processor_id)                            (**r signed multiply high *)
+  | Pumulh (rd: ireg) (r1 r2: ireg) (pid: processor_id)                            (**r unsigned multiply high *)
+  | Psdiv (sz: isize) (rd: ireg) (r1 r2: ireg) (pid: processor_id)                 (**r signed division *)
+  | Pudiv (sz: isize) (rd: ireg) (r1 r2: ireg) (pid: processor_id)                 (**r unsigned division *)
+  (** Floating-point loads and stores *)
+  | Pldrs (rd: freg) (a: addressing) (pid: processor_id)                           (**r load float32 (single precision) *)
+  | Pldrd (rd: freg) (a: addressing) (pid: processor_id)                           (**r load float64 (double precision) *)
+  | Pldrd_a (rd: freg) (a: addressing) (pid: processor_id)                         (**r load float64 as any64 *)
+  | Pstrs (rs: freg) (a: addressing) (pid: processor_id)                           (**r store float32 *)
+  | Pstrd (rs: freg) (a: addressing) (pid: processor_id)                           (**r store float64 *)
+  | Pstrd_a (rs: freg) (a: addressing) (pid: processor_id)                         (**r store float64 as any64 *)
+  (** Floating-point move *)
+  | Pfmov (rd r1: freg) (pid: processor_id) 
+  | Pfmovimms (rd: freg) (f: float32) (pid: processor_id)                          (**r load float32 constant *)
+  | Pfmovimmd (rd: freg) (f: float) (pid: processor_id)                            (**r load float64 constant *)
+  | Pfmovi (fsz: fsize) (rd: freg) (r1: ireg0) (pid: processor_id)                 (**r copy int reg to FP reg *)
+  (** Floating-point conversions *)
+  | Pfcvtds (rd r1: freg) (pid: processor_id)                                      (**r convert float32 to float64 *)
+  | Pfcvtsd (rd r1: freg) (pid: processor_id)                                      (**r convert float64 to float32 *)
+  | Pfcvtzs (isz: isize) (fsz: fsize) (rd: ireg) (r1: freg) (pid: processor_id)    (**r convert float to signed int *)
+  | Pfcvtzu (isz: isize) (fsz: fsize) (rd: ireg) (r1: freg) (pid: processor_id)    (**r convert float to unsigned int *)
+  | Pscvtf (fsz: fsize) (isz: isize) (rd: freg) (r1: ireg) (pid: processor_id)     (**r convert signed int to float *)
+  | Pucvtf (fsz: fsize) (isz: isize) (rd: freg) (r1: ireg) (pid: processor_id)     (**r convert unsigned int to float *)
+  (** Floating-point arithmetic *)
+  | Pfabs (sz: fsize) (rd r1: freg) (pid: processor_id)                            (**r absolute value *)
+  | Pfneg (sz: fsize) (rd r1: freg) (pid: processor_id)                            (**r negation *)
+  | Pfsqrt (sz: fsize) (rd r1: freg) (pid: processor_id)                           (**r square root *)
+  | Pfadd (sz: fsize) (rd r1 r2: freg) (pid: processor_id)                         (**r addition *)
+  | Pfdiv (sz: fsize) (rd r1 r2: freg) (pid: processor_id)                         (**r division *)
+  | Pfmul (sz: fsize) (rd r1 r2: freg) (pid: processor_id)                         (**r multiplication *)
+  | Pfnmul (sz: fsize) (rd r1 r2: freg) (pid: processor_id)                        (**r multiply-negate *)
+  | Pfsub (sz: fsize) (rd r1 r2: freg) (pid: processor_id)                         (**r subtraction *)
+  | Pfmadd (sz: fsize) (rd r1 r2 r3: freg) (pid: processor_id)                     (**r [rd = r3 + r1 * r2] *)
+  | Pfmsub (sz: fsize) (rd r1 r2 r3: freg) (pid: processor_id)                     (**r [rd = r3 - r1 * r2] *)
+  | Pfnmadd (sz: fsize) (rd r1 r2 r3: freg) (pid: processor_id)                    (**r [rd = - r3 - r1 * r2] *)
+  | Pfnmsub (sz: fsize) (rd r1 r2 r3: freg) (pid: processor_id)                    (**r [rd = - r3 + r1 * r2] *)
+  | Pfmax (sz: fsize) (rd r1 r2: freg) (pid: processor_id)                         (**r maximum *)
+  | Pfmin (sz: fsize) (rd r1 r2: freg) (pid: processor_id)                         (**r minimum *)
+  (** Floating-point comparison *)
+  | Pfcmp (sz: fsize) (r1 r2: freg) (pid: processor_id)                            (**r compare [r1] and [r2] *)
+  | Pfcmp0 (sz: fsize) (r1: freg) (pid: processor_id)                              (**r compare [r1] and [+0.0] *)
+  (** Floating-point conditional select *)
+  | Pfsel (rd r1 r2: freg) (cond: testcond) (pid: processor_id) 
+  (** Pseudo-instructions *)
+  | Pallocframe (sz: Z) (linkofs: ptrofs) (pid: processor_id)                      (**r allocate new stack frame *)
+  | Pfreeframe (sz: Z) (linkofs: ptrofs) (pid: processor_id)                       (**r deallocate stack frame and restore previous frame *)
+  | Plabel (lbl: label) (pid: processor_id)                                        (**r define a code label *)
+  | Ploadsymbol (rd: ireg) (id: ident) (pid: processor_id)                         (**r load the address of [id] *)
+  | Pcvtsw2x (rd: ireg) (r1: ireg) (pid: processor_id)                             (**r sign-extend 32-bit int to 64-bit *)
+  | Pcvtuw2x (rd: ireg) (r1: ireg) (pid: processor_id)                             (**r zero-extend 32-bit int to 64-bit *)
+  | Pcvtx2w (rd: ireg) (pid: processor_id)                                         (**r retype a 64-bit int as a 32-bit int *)
+  | Pbtbl (r1: ireg) (tbl: list label) (pid: processor_id)                         (**r N-way branch through a jump table *)
+  | Pbuiltin (ef: external_function)
+             (args: list (builtin_arg preg)) (res: builtin_res preg) (pid: processor_id)   (**r built-in function (pseudo) *)
+  | Pnop (pid: processor_id)                                                            (**r no operation *)
+  | Pcfi_adjust (ofs: int) (pid: processor_id)                                     (**r .cfi_adjust debug directive *)
+  | Pcfi_rel_offset (ofs: int) (pid: processor_id)                                 (**r .cfi_rel_offset debug directive *)
+  | Pincpc (pid: processor_id) (** my own thing, represents incrementing PC*)
+.
+
+
+(** * Operational semantics *)
+
+(** The semantics operates over a single mapping from registers
+  (type [preg]) to values.  We maintain (but do not enforce)
+  the convention that integer registers are mapped to values of
+  type [Tint], float registers to values of type [Tfloat],
+  and condition bits to either [Vzero] or [Vone]. *)
+
+
+(** Map of processor id + regcode to val for that processor*)
+Definition allregsets := PRmap.t val.
+
+
+
+(* Bidirectionality hint -> helps convert processor_id, preg -> PRMap.t*)
+Arguments pair {_ _} & _ _.
+
+Definition ir0w (ars: allregsets) (r: ireg0) (pid: processor_id) : val :=
+  match r with RR0 r => ars (pid, (IR r)) | XZR => Vint Int.zero end.
+Definition ir0x (ars: allregsets) (r: ireg0) (pid: processor_id) : val :=
+  match r with RR0 r => ars (pid, (IR r)) | XZR => Vlong Int64.zero end.
+
+(** Concise notations for accessing and updating the values of registers. *)
+Notation "a @ b" := (a b) (at level 1, only parsing).
+Notation "a @ b <- c" := (PRmap.set b c a) (at level 1, b at next level).
+Notation "a @@ c @@> b" := (ir0w a b c) (at level 1, only parsing).
+Notation "a @@@ c @@@> b" := (ir0x a b c) (at level 1, only parsing).
+
+Inductive outcome: Type := 
+    | MemSimNext: allregsets -> mem -> outcome
+    | MemSimJumpOut: allregsets -> mem -> outcome
+    | MemSimStuck: outcome.
+
+
+Definition goto_label (f: function) (lbl: label) (ars: allregsets) (pid: processor_id) (m: mem) :=
+    match label_pos lbl 0 (fn_code f) with
+    | None => MemSimStuck
+    | Some pos =>
+        match ars@(pid, PC) with
+        | Vptr b ofs => MemSimJumpOut (ars@(pid, PC ) <- (Vptr b (Ptrofs.repr pos))) m
+        | _ => MemSimStuck
+        end
+    end.
+
+Definition eval_testcond (c: testcond) (ars: allregsets) (pid: processor_id): option bool :=
+    match c with
+    | TCeq =>                             (**r equal *)
+        match ars@(pid, CZ) with
+        | Vint n => Some (Int.eq n Int.one)
+        | _ => None
+        end
+    | TCne =>                             (**r not equal *)
+        match ars@(pid, CZ) with
+        | Vint n => Some (Int.eq n Int.zero)
+        | _ => None
+        end
+    | TClo =>                             (**r unsigned less than  *)
+        match ars@(pid, CC) with
+        | Vint n => Some (Int.eq n Int.zero)
+        | _ => None
+        end
+    | TCls =>                             (**r unsigned less or equal *)
+        match ars@(pid, CC), ars@(pid, CZ) with
+        | Vint c, Vint z => Some (Int.eq c Int.zero || Int.eq z Int.one)
+        | _, _ => None
+        end
+    | TChs =>                             (**r unsigned greater or equal *)
+        match ars@(pid, CC) with
+        | Vint n => Some (Int.eq n Int.one)
+        | _ => None
+        end
+    | TChi =>                             (**r unsigned greater *)
+        match ars@(pid, CC), ars@(pid, CZ) with
+        | Vint c, Vint z => Some (Int.eq c Int.one && Int.eq z Int.zero)
+        | _, _ => None
+        end
+    | TClt =>                             (**r signed less than *)
+        match ars@(pid, CV), ars@(pid, CN) with
+        | Vint o, Vint s => Some (Int.eq (Int.xor o s) Int.one)
+        | _, _ => None
+        end
+    | TCle =>                             (**r signed less or equal *)
+        match ars@(pid, CV), ars@(pid, CN), ars@(pid, CZ) with
+        | Vint o, Vint s, Vint z => Some (Int.eq (Int.xor o s) Int.one || Int.eq z Int.one)
+        | _, _, _ => None
+        end
+    | TCge =>                             (**r signed greater or equal *)
+        match ars@(pid, CV), ars@(pid, CN) with
+        | Vint o, Vint s => Some (Int.eq (Int.xor o s) Int.zero)
+        | _, _ => None
+        end
+    | TCgt =>                             (**r signed greater *)
+        match ars@(pid, CV), ars@(pid, CN), ars@(pid, CZ) with
+        | Vint o, Vint s, Vint z => Some (Int.eq (Int.xor o s) Int.zero && Int.eq z Int.zero)
+        | _, _, _ => None
+        end
+    | TCpl =>                             (**r positive *)
+        match ars@(pid, CN) with
+        | Vint n => Some (Int.eq n Int.zero)
+        | _ => None
+        end
+    | TCmi =>                             (**r negative *)
+        match ars@(pid, CN) with
+        | Vint n => Some (Int.eq n Int.one)
+        | _ => None
+        end
+    end.
+
+Section RELSEM.
+Variable ge: genv.
+
+
+Definition eval_addressing (a: addressing) (ars: allregsets) (pid: processor_id): val :=
+  match a with
+  | ADimm base n => Val.addl ars@(pid, base) (Vlong n)
+  | ADreg base r => Val.addl ars@(pid, base)  ars@(pid, r)
+  | ADlsl base r n => Val.addl ars@(pid, base) (Val.shll ars@(pid, r) (Vint n))
+  | ADsxt base r n => Val.addl ars@(pid, base) (Val.shll (Val.longofint ars@(pid, r)) (Vint n))
+  | ADuxt base r n => Val.addl ars@(pid, base) (Val.shll (Val.longofintu ars@(pid, r)) (Vint n))
+  | ADadr base id ofs => Val.addl ars@(pid, base) (symbol_low ge id ofs)
+  | ADpostincr base n => Vundef (* not modeled yet *)
+  end.
+
+Definition exec_load (chunk: memory_chunk) (transf: val -> val)
+    (a: addressing) (r: preg) (ars: allregsets) (pid: processor_id) (m: mem)  :=
+    match Mem.loadv chunk m (eval_addressing a ars pid) with
+    | None => MemSimStuck
+    | Some v => MemSimNext (ars@(pid, r) <- (transf v)) m
+    end.
+
+Definition exec_store (chunk: memory_chunk)
+    (a: addressing) (v: val)
+    (ars: allregsets) (pid: processor_id) (m: mem) :=
+match Mem.storev chunk m (eval_addressing a ars pid) v with
+| None => MemSimStuck
+| Some m' => MemSimNext ars m'
+end.
+
+Definition compare_int (ars: allregsets) (v1 v2: val) (m: mem) (pid: processor_id) :=
+  ars@(pid, CN) <- (Val.negative (Val.sub v1 v2))
+  @(pid, CZ)  <- (Val.cmpu (Mem.valid_pointer m) Ceq v1 v2)
+  @(pid, CC)  <- (Val.cmpu (Mem.valid_pointer m) Cge v1 v2)
+  @(pid, CV)  <- (Val.sub_overflow v1 v2).
+
+Definition compare_long (ars: allregsets) (v1 v2: val) (m: mem) (pid: processor_id) :=
+  ars@(pid, CN) <- (Val.negativel (Val.subl v1 v2))
+  @(pid, CZ)  <- (Val.maketotal (Val.cmplu (Mem.valid_pointer m) Ceq v1 v2))
+  @(pid, CC)  <- (Val.maketotal (Val.cmplu (Mem.valid_pointer m) Cge v1 v2))
+  @(pid, CV)  <- (Val.subl_overflow v1 v2).
+
+  Definition compare_float (ars: allregsets) (v1 v2: val) (pid: processor_id) :=
+  match v1, v2 with
+  | Vfloat f1, Vfloat f2 =>
+      ars@(pid, CN) <- (Val.of_bool (Float.cmp Clt f1 f2))
+        @(pid, CZ) <- (Val.of_bool (Float.cmp Ceq f1 f2))
+        @(pid, CC) <- (Val.of_bool (negb (Float.cmp Clt f1 f2)))
+        @(pid, CV) <- (Val.of_bool (negb (Float.ordered f1 f2)))
+  | _, _ =>
+      ars@(pid, CN) <- Vundef
+      @(pid, CZ) <- Vundef
+      @(pid, CC) <- Vundef
+      @(pid, CV) <- Vundef
+  end.
+
+Definition compare_single (ars: allregsets) (v1 v2: val) (pid: processor_id) :=
+  match v1, v2 with
+  | Vsingle f1, Vsingle f2 =>
+      ars@(pid, CN) <- (Val.of_bool (Float32.cmp Clt f1 f2))
+      @(pid, CZ) <- (Val.of_bool (Float32.cmp Ceq f1 f2))
+      @(pid, CC) <- (Val.of_bool (negb (Float32.cmp Clt f1 f2)))
+      @(pid, CV) <- (Val.of_bool (negb (Float32.ordered f1 f2)))
+  | _, _ =>
+      ars@(pid, CN) <- Vundef
+      @(pid, CZ) <- Vundef
+      @(pid, CC) <- Vundef
+      @(pid, CV) <- Vundef
+  end.
+
+Definition eval_memsim_instr (f: function) (i: instruction) (ars: allregsets) (m: mem) : outcome :=
+    match i with
+    (** Branches *)
+    | Pb lbl pid =>
+        goto_label f lbl ars pid m
+    | Pbc cond lbl pid =>
+        match eval_testcond cond ars pid with
+        | Some true => goto_label f lbl ars pid m
+        | Some false => MemSimNext ars m
+        | None => MemSimStuck
+        end
+    | Pbl id sg pid =>
+        MemSimNext (ars@ (pid, RA)  <- (Val.offset_ptr ars@ (pid, PC)  Ptrofs.one) @ (pid, PC) <- (Genv.symbol_address ge id Ptrofs.zero)) m
+    | Pbs id sg pid =>
+        MemSimNext (ars@ (pid , PC)  <- (Genv.symbol_address ge id Ptrofs.zero)) m
+    | Pblr r sg pid =>
+        MemSimNext (ars@ (pid , RA)  <- (Val.offset_ptr ars@ (pid , PC)  Ptrofs.one) @ (pid, PC) <- (ars@ (pid , r)) ) m
+    | Pbr r sg pid =>
+        MemSimNext (ars@ (pid , PC)  <- (ars@ (pid , r)) ) m
+    | Pret r pid =>
+        MemSimNext (ars@ (pid , PC)  <- (ars@ (pid , r)) ) m
+    | Pcbnz sz r lbl pid =>
+        match eval_testzero sz ars@ (pid , r ) m with
+        | Some true => MemSimNext ars m
+        | Some false => goto_label f lbl ars pid m
+        | None => MemSimStuck
+        end
+    | Pcbz sz r lbl pid =>
+        match eval_testzero sz ars@ (pid , r ) m with
+        | Some true => goto_label f lbl ars pid m
+        | Some false => MemSimNext ars m
+        | None => MemSimStuck
+        end
+    | Ptbnz sz r n lbl pid =>
+        match eval_testbit sz ars@ (pid , r ) n with
+        | Some true => goto_label f lbl ars pid m
+        | Some false => MemSimNext ars m
+        | None => MemSimStuck
+        end
+    | Ptbz sz r n lbl pid =>
+        match eval_testbit sz ars@ (pid , r ) n with
+        | Some true => MemSimNext ars m
+        | Some false => goto_label f lbl ars pid m
+        | None => MemSimStuck
+        end
+    (** Memory loads and stores *)
+    | Pldrw rd a pid =>
+        exec_load Mint32 (fun v => v) a rd ars pid m
+    | Pldrw_a rd a pid =>
+        exec_load Many32 (fun v => v) a rd ars pid m
+    | Pldrx rd a pid =>
+        exec_load Mint64 (fun v => v) a rd ars pid m
+    | Pldrx_a rd a pid =>
+        exec_load Many64 (fun v => v) a rd ars pid m
+    | Pldrb W rd a pid =>
+        exec_load Mint8unsigned (fun v => v) a rd ars pid m
+    | Pldrb X rd a pid =>
+        exec_load Mint8unsigned Val.longofintu a rd ars pid m
+    | Pldrsb W rd a pid =>
+        exec_load Mint8signed (fun v => v) a rd ars pid m
+    | Pldrsb X rd a pid =>
+        exec_load Mint8signed Val.longofint a rd ars pid m
+    | Pldrh W rd a pid =>
+        exec_load Mint16unsigned (fun v => v) a rd ars pid m
+    | Pldrh X rd a pid =>
+        exec_load Mint16unsigned Val.longofintu a rd ars pid m
+    | Pldrsh W rd a pid =>
+        exec_load Mint16signed (fun v => v) a rd ars pid m
+    | Pldrsh X rd a pid =>
+        exec_load Mint16signed Val.longofint a rd ars pid m
+    | Pldrzw rd a pid =>
+        exec_load Mint32 Val.longofintu a rd ars pid m
+    | Pldrsw rd a pid =>
+        exec_load Mint32 Val.longofint a rd ars pid m
+    | Pstrw r a pid =>
+        exec_store Mint32 a ars@(pid, r) ars pid m
+    | Pstrw_a r a pid =>
+        exec_store Many32 a  ars@(pid, r) ars pid m
+    | Pstrx r a pid =>
+        exec_store Mint64 a  ars@(pid, r) ars pid m
+    | Pstrx_a r a pid =>
+        exec_store Many64 a  ars@(pid, r) ars pid m
+    | Pstrb r a pid =>
+        exec_store Mint8unsigned a ars@(pid, r) ars pid m
+    | Pstrh r a pid =>
+        exec_store Mint16unsigned a ars@(pid, r) ars pid m
+    (** Integer arithmetic, immediate *)
+    | Paddimm W rd r1 n pid =>
+        MemSimNext ((ars@ (pid, rd)  <- (Val.add ars@ (pid, r1)  (Vint (Int.repr n))))) m
+    | Paddimm X rd r1 n pid =>
+        MemSimNext ((ars@ (pid, rd)  <- (Val.addl ars@ (pid, r1)  (Vlong (Int64.repr n))))) m
+    | Psubimm W rd r1 n pid =>
+        MemSimNext ((ars@ (pid, rd)  <- (Val.sub ars@ (pid, r1)  (Vint (Int.repr n))))) m
+    | Psubimm X rd r1 n pid =>
+        MemSimNext ((ars@ (pid, rd)  <- (Val.subl ars@ (pid, r1)  (Vlong (Int64.repr n))))) m
+    | Pcmpimm W r1 n pid =>
+        MemSimNext ((compare_int ars ars@(pid, r1)  (Vint (Int.repr n)) m) pid ) m
+    | Pcmpimm X r1 n pid =>
+        MemSimNext ((compare_long ars ars@ (pid, r1)  (Vlong (Int64.repr n)) m) pid ) m
+    | Pcmnimm W r1 n pid =>
+        MemSimNext ((compare_int ars ars@ (pid, r1)  (Vint (Int.neg (Int.repr n))) m) pid) m
+    | Pcmnimm X r1 n pid =>
+        MemSimNext ((compare_long ars ars@ (pid, r1)  (Vlong (Int64.neg (Int64.repr n))) m) pid) m
+    (** Move integer register *)
+    | Pmov rd r1 pid =>
+        MemSimNext ( (ars@ (pid, rd)  <- (ars@ (pid, r1) ))) m
+    (** Logical, immediate *)
+    | Pandimm W rd r1 n pid =>
+        MemSimNext ((ars@(pid, rd)  <- (Val.and (ars@@ pid @@> r1) (Vint (Int.repr n))))) m
+    | Pandimm X rd r1 n pid =>
+        MemSimNext ((ars@ (pid, rd)  <- (Val.andl (ars@@@ pid @@@> r1) (Vlong (Int64.repr n))))) m
+    | Peorimm W rd r1 n pid =>
+        MemSimNext ((ars@ (pid, rd)  <- (Val.xor (ars@@ pid @@> r1)  (Vint (Int.repr n))))) m
+    | Peorimm X rd r1 n pid =>
+        MemSimNext ((ars@ (pid, rd)  <- (Val.xorl (ars@@@ pid @@@> r1) (Vlong (Int64.repr n))))) m
+    | Porrimm W rd r1 n pid =>
+        MemSimNext ((ars@ (pid, rd)  <- (Val.or (ars@@ pid @@> r1) (Vint (Int.repr n))))) m
+    | Porrimm X rd r1 n pid =>
+        MemSimNext ((ars@ (pid, rd)  <- (Val.orl (ars@@ pid @@> r1) (Vlong (Int64.repr n))))) m
+    | Ptstimm W r1 n pid =>
+        MemSimNext (compare_int ars (Val.and ars@ (pid, r1)  (Vint (Int.repr n))) (Vint Int.zero) m pid) m
+    | Ptstimm X r1 n pid =>
+        MemSimNext ((compare_long ars (Val.andl ars@ (pid, r1)  (Vlong (Int64.repr n))) (Vlong Int64.zero) m pid)) m
+    (** Move wide immediate *)
+    | Pmovz W rd n pos pid =>
+        MemSimNext ((ars@ (pid, rd)  <- (Vint (Int.repr (Z.shiftl n pos))))) m
+    | Pmovz X rd n pos pid =>
+        MemSimNext ((ars@ (pid, rd)  <- (Vlong (Int64.repr (Z.shiftl n pos))))) m
+    | Pmovn W rd n pos pid =>
+        MemSimNext ((ars@ (pid, rd)  <- (Vint (Int.repr (Z.lnot (Z.shiftl n pos)))))) m
+    | Pmovn X rd n pos pid =>
+        MemSimNext ((ars@ (pid, rd)  <- (Vlong (Int64.repr (Z.lnot (Z.shiftl n pos)))))) m
+    | Pmovk W rd n pos pid =>
+        MemSimNext ((ars@ (pid, rd)  <- (insert_in_int ars@ (pid, rd)  n pos 16))) m
+    | Pmovk X rd n pos pid =>
+        MemSimNext ((ars@ (pid, rd)  <- (insert_in_long ars@ (pid, rd)  n pos 16))) m
+    (** PC-relative addressing *)
+    | Padrp rd id ofs pid =>
+        MemSimNext ((ars@ (pid, rd)  <- (symbol_high ge id ofs))) m
+    | Paddadr rd r1 id ofs pid =>
+        MemSimNext ((ars@ (pid, rd)  <- (Val.addl ars@ (pid, r1)  (symbol_low ge id ofs)))) m
+    (** Bit-field operations *)
+    | Psbfiz W rd r1 r s pid =>
+        MemSimNext ((ars@ (pid, rd)  <- (Val.shl (Val.sign_ext s ars@ (pid, r1) ) (Vint r)))) m
+    | Psbfiz X rd r1 r s pid =>
+        MemSimNext ((ars@ (pid, rd)  <- (Val.shll (Val.sign_ext_l s ars@ (pid, r1) ) (Vint r)))) m
+    | Psbfx W rd r1 r s pid =>
+        MemSimNext ((ars@ (pid, rd)  <- (Val.sign_ext s (Val.shr ars@ (pid, r1)  (Vint r))))) m
+    | Psbfx X rd r1 r s pid =>
+        MemSimNext ((ars@ (pid, rd)  <- (Val.sign_ext_l s (Val.shrl ars@ (pid, r1)  (Vint r))))) m
+    | Pubfiz W rd r1 r s pid =>
+        MemSimNext ((ars@ (pid, rd)  <- (Val.shl (Val.zero_ext s ars@ (pid, r1) ) (Vint r)))) m
+    | Pubfiz X rd r1 r s pid =>
+        MemSimNext ((ars@ (pid, rd)  <- (Val.shll (Val.zero_ext_l s ars@ (pid, r1) ) (Vint r)))) m
+    | Pubfx W rd r1 r s pid =>
+        MemSimNext ((ars@ (pid, rd)  <- (Val.zero_ext s (Val.shru ars@ (pid, r1)  (Vint r))))) m
+    | Pubfx X rd r1 r s pid =>
+        MemSimNext ((ars@ (pid, rd)  <- (Val.zero_ext_l s (Val.shrlu ars@ (pid, r1)  (Vint r))))) m
+    (** Integer arithmetic, shifted register *)
+    | Padd W rd r1 r2 s pid =>
+        MemSimNext (ars@ (pid, rd)  <- (Val.add ars@@ pid @@> r1 (eval_shift_op_int ars@ (pid, r2)  s))) m
+    | Padd X rd r1 r2 s pid =>
+        MemSimNext (ars@ (pid, rd)  <- (Val.addl ars@@@pid @@@> r1 (eval_shift_op_long ars@ (pid, r2)  s))) m
+    | Psub W rd r1 r2 s pid =>
+        MemSimNext ((ars@ (pid, rd)  <- (Val.sub ars@@pid @@> r1 (eval_shift_op_int ars@ (pid, r2)  s)))) m
+    | Psub X rd r1 r2 s pid =>
+        MemSimNext ((ars@ (pid, rd)  <- (Val.subl ars@@@ pid@@@> r1 (eval_shift_op_long ars@ (pid, r2)  s)))) m
+    | Pcmp W r1 r2 s pid =>
+        MemSimNext (compare_int ars (ars@@pid@@>r1) (eval_shift_op_int ars@(pid, r2)  s) m pid) m
+    | Pcmp X r1 r2 s pid =>
+        MemSimNext ((compare_long ars ars@@@pid@@@>r1) (eval_shift_op_long ars@ (pid, r2)  s) m pid) m
+    | Pcmn W r1 r2 s pid =>
+        MemSimNext (compare_int ars ars@@pid@@>r1 (Val.neg (eval_shift_op_int ars@ (pid, r2)  s)) m pid) m
+    | Pcmn X r1 r2 s pid =>
+        MemSimNext ((compare_long ars ars@@@pid@@@>r1 (Val.negl (eval_shift_op_long ars@ (pid, r2)  s)) m pid)) m
+    (** Integer arithmetic, extending register *)
+    | Paddext rd r1 r2 x pid =>
+        MemSimNext ((ars@ (pid, rd)  <- (Val.addl ars@ (pid, r1)  (eval_extend ars@ (pid, r2)  x)))) m
+    | Psubext rd r1 r2 x pid =>
+        MemSimNext ((ars@ (pid, rd)  <- (Val.subl ars@ (pid, r1)  (eval_extend ars@ (pid, r2)  x)))) m
+    | Pcmpext r1 r2 x pid =>
+        MemSimNext ((compare_long ars ars@ (pid, r1)  (eval_extend ars@ (pid, r2)  x) m pid)) m
+    | Pcmnext r1 r2 x pid =>
+        MemSimNext ((compare_long ars ars@ (pid, r1)  (Val.negl (eval_extend ars@ (pid, r2)  x)) m pid)) m
+    (** Logical, shifted register *)
+    | Pand W rd r1 r2 s pid =>
+        MemSimNext ((ars@ (pid , rd)  <- (Val.and ars@@pid@@>r1 (eval_shift_op_int ars@ (pid , r2)  s)))) m
+    | Pand X rd r1 r2 s pid =>
+        MemSimNext ((ars@ (pid , rd)  <- (Val.andl ars@@@pid@@@>r1 (eval_shift_op_long ars@ (pid , r2)  s)))) m
+    | Pbic W rd r1 r2 s pid =>
+        MemSimNext ((ars@ (pid , rd)  <- (Val.and ars@@pid@@>r1 (Val.notint (eval_shift_op_int ars@ (pid , r2)  s))))) m
+    | Pbic X rd r1 r2 s pid =>
+        MemSimNext ((ars@ (pid , rd)  <- (Val.andl ars@@@pid@@@>r1 (Val.notl (eval_shift_op_long ars@ (pid , r2)  s))))) m
+    | Peon W rd r1 r2 s pid =>
+        MemSimNext ((ars@ (pid , rd)  <- (Val.xor ars@@pid@@>r1 (Val.notint (eval_shift_op_int ars@ (pid , r2)  s))))) m
+    | Peon X rd r1 r2 s pid =>
+        MemSimNext ((ars@ (pid , rd)  <- (Val.xorl ars@@@pid@@@>r1 (Val.notl (eval_shift_op_long ars@ (pid , r2)  s))))) m
+    | Peor W rd r1 r2 s pid =>
+        MemSimNext ((ars@ (pid , rd)  <- (Val.xor ars@@pid@@>r1 (eval_shift_op_int ars@ (pid , r2)  s)))) m
+    | Peor X rd r1 r2 s pid =>
+        MemSimNext ((ars@ (pid , rd)  <- (Val.xorl ars@@@pid@@@>r1 (eval_shift_op_long ars@ (pid , r2)  s)))) m
+    | Porr W rd r1 r2 s pid =>
+        MemSimNext ((ars@ (pid , rd)  <- (Val.or ars@@pid@@>r1 (eval_shift_op_int ars@ (pid , r2)  s)))) m
+    | Porr X rd r1 r2 s pid =>
+        MemSimNext ((ars@ (pid , rd)  <- (Val.orl ars@@@pid@@@>r1 (eval_shift_op_long ars@ (pid , r2)  s)))) m
+    | Porn W rd r1 r2 s pid =>
+        MemSimNext ((ars@ (pid , rd)  <- (Val.or ars@@pid@@>r1 (Val.notint (eval_shift_op_int ars@ (pid , r2)  s))))) m
+    | Porn X rd r1 r2 s pid =>
+        MemSimNext ((ars@ (pid , rd)  <- (Val.orl ars@@@pid@@@>r1 (Val.notl (eval_shift_op_long ars@ (pid , r2)  s))))) m
+    | Ptst W r1 r2 s pid =>
+        MemSimNext ((compare_int ars (Val.and ars@@pid@@>r1 (eval_shift_op_int ars@ (pid , r2)  s)) (Vint Int.zero) m pid)) m
+    | Ptst X r1 r2 s pid =>
+        MemSimNext ((compare_long ars (Val.andl ars@@@pid@@@>r1 (eval_shift_op_long ars@ (pid , r2)  s)) (Vlong Int64.zero) m pid)) m
+    (*** Variable shifts *)
+    | Pasrv W rd r1 r2 pid =>
+        MemSimNext ((ars@ (pid, rd)  <- (Val.shr ars@ (pid, r1)  ars@ (pid, r2) ))) m
+    | Pasrv X rd r1 r2 pid =>
+        MemSimNext ((ars@ (pid, rd)  <- (Val.shrl ars@ (pid, r1)  ars@ (pid, r2) ))) m
+    | Plslv W rd r1 r2 pid =>
+        MemSimNext ((ars@ (pid, rd)  <- (Val.shl ars@ (pid, r1)  ars@ (pid, r2) ))) m
+    | Plslv X rd r1 r2 pid =>
+        MemSimNext ((ars@ (pid, rd)  <- (Val.shll ars@ (pid, r1)  ars@ (pid, r2) ))) m
+    | Plsrv W rd r1 r2 pid =>
+        MemSimNext ((ars@ (pid, rd)  <- (Val.shru ars@ (pid, r1)  ars@ (pid, r2) ))) m
+    | Plsrv X rd r1 r2 pid =>
+        MemSimNext ((ars@ (pid, rd)  <- (Val.shrlu ars@ (pid, r1)  ars@ (pid, r2) ))) m
+    | Prorv W rd r1 r2 pid =>
+        MemSimNext ((ars@ (pid, rd)  <- (Val.ror ars@ (pid, r1)  ars@ (pid, r2) ))) m
+    | Prorv X rd r1 r2 pid =>
+        MemSimNext ((ars@ (pid, rd)  <- (Val.rorl ars@ (pid, r1)  ars@ (pid, r2) ))) m
+    (** Conditional data processing *)
+    | Pcsel rd r1 r2 cond pid =>
+        let v :=
+            match eval_testcond cond ars pid with
+            | Some true => ars@ (pid, r1) 
+            | Some false => ars@ (pid, r2) 
+            | None => Vundef
+            end in
+        MemSimNext ((ars@ (pid, rd)  <- v)) m
+    | Pcset rd cond pid =>
+        let v :=
+            match eval_testcond cond ars pid with
+            | Some true => Vint Int.one
+            | Some false => Vint Int.zero
+            | None => Vundef
+            end in
+        MemSimNext ((ars@ (pid, rd)  <- v)) m
+    (** Integer multiply/divide *)
+    | Pmadd W rd r1 r2 r3 pid =>
+        MemSimNext ((ars@ (pid, rd)  <- (Val.add ars@@pid@@>r3 (Val.mul ars@ (pid, r1)  ars@ (pid, r2) )))) m
+    | Pmadd X rd r1 r2 r3 pid =>
+        MemSimNext ((ars@ (pid, rd)  <- (Val.addl ars@@@pid@@@>r3 (Val.mull ars@ (pid, r1)  ars@ (pid, r2) )))) m
+    | Pmsub W rd r1 r2 r3 pid =>
+        MemSimNext ((ars@ (pid, rd)  <- (Val.sub ars@@pid@@>r3 (Val.mul ars@ (pid, r1)  ars@ (pid, r2) )))) m
+    | Pmsub X rd r1 r2 r3 pid =>
+        MemSimNext ((ars@ (pid, rd)  <- (Val.subl ars@@@pid@@@>r3 (Val.mull ars@ (pid, r1)  ars@ (pid, r2) )))) m
+    | Psmulh rd r1 r2 pid =>
+        MemSimNext ((ars@ (pid, rd)  <- (Val.mullhs ars@ (pid, r1)  ars@ (pid, r2) ))) m
+    | Pumulh rd r1 r2 pid =>
+        MemSimNext ((ars@ (pid, rd)  <- (Val.mullhu ars@ (pid, r1)  ars@ (pid, r2) ))) m
+    | Psdiv W rd r1 r2 pid =>
+        MemSimNext ((ars@ (pid, rd)  <- (Val.maketotal (Val.divs ars@ (pid, r1)  ars@ (pid, r2) )))) m
+    | Psdiv X rd r1 r2 pid =>
+        MemSimNext ((ars@ (pid, rd)  <- (Val.maketotal (Val.divls ars@ (pid, r1)  ars@ (pid, r2) )))) m
+    | Pudiv W rd r1 r2 pid =>
+        MemSimNext ((ars@ (pid, rd)  <- (Val.maketotal (Val.divu ars@ (pid, r1)  ars@ (pid, r2) )))) m
+    | Pudiv X rd r1 r2 pid =>
+        MemSimNext ((ars@ (pid, rd)  <- (Val.maketotal (Val.divlu ars@ (pid, r1)  ars@ (pid, r2) )))) m
+    (** Floating-point loads and stores *)
+    | Pldrs rd a pid =>
+        exec_load Mfloat32 (fun v => v) a rd ars pid m
+    | Pldrd rd a pid =>
+        exec_load Mfloat64 (fun v => v) a rd ars pid m
+    | Pldrd_a rd a pid =>
+        exec_load Many64 (fun v => v) a rd ars pid m
+    | Pstrs r a pid =>
+        exec_store Mfloat32 a ars@ (pid, r ) ars pid m
+    | Pstrd r a pid =>
+        exec_store Mfloat64 a ars@ (pid, r ) ars pid m
+    | Pstrd_a r a pid =>
+        exec_store Many64 a ars@ (pid, r ) ars pid m
+    (** Floating-point move *)
+    | Pfmov rd r1 pid =>
+        MemSimNext ((ars@ (pid, rd)  <- (ars@ (pid, r1) ))) m
+    | Pfmovimms rd f pid =>
+        MemSimNext ((ars@ (pid, X16) <- Vundef @(pid, rd) <- (Vsingle f))) m
+    | Pfmovimmd rd f pid =>
+        MemSimNext ((ars@ (pid, X16) <- Vundef @(pid, rd) <- (Vfloat f))) m
+    | Pfmovi S rd r1 pid =>
+        MemSimNext ((ars@ (pid, rd)  <- (float32_of_bits ars@@pid@@>r1))) m
+    | Pfmovi D rd r1 pid =>
+        MemSimNext ((ars@ (pid, rd)  <- (float64_of_bits ars@@@pid@@@>r1))) m
+    (** Floating-point conversions *)
+    | Pfcvtds rd r1 pid =>
+        MemSimNext ((ars@ (pid, rd)  <- (Val.floatofsingle ars@ (pid, r1) ))) m
+    | Pfcvtsd rd r1 pid =>
+        MemSimNext ((ars@ (pid, rd)  <- (Val.singleoffloat ars@ (pid, r1) ))) m
+    | Pfcvtzs W S rd r1 pid =>
+        MemSimNext ((ars@ (pid, rd)  <- (Val.maketotal (Val.intofsingle ars@ (pid, r1) )))) m
+    | Pfcvtzs W D rd r1 pid =>
+        MemSimNext ((ars@ (pid, rd)  <- (Val.maketotal (Val.intoffloat ars@ (pid, r1) )))) m
+    | Pfcvtzs X S rd r1 pid =>
+        MemSimNext ((ars@ (pid, rd)  <- (Val.maketotal (Val.longofsingle ars@ (pid, r1) )))) m
+    | Pfcvtzs X D rd r1 pid =>
+        MemSimNext ((ars@ (pid, rd)  <- (Val.maketotal (Val.longoffloat ars@ (pid, r1) )))) m
+    | Pfcvtzu W S rd r1 pid =>
+        MemSimNext ((ars@ (pid, rd)  <- (Val.maketotal (Val.intuofsingle ars@ (pid, r1) )))) m
+    | Pfcvtzu W D rd r1 pid =>
+        MemSimNext ((ars@ (pid, rd)  <- (Val.maketotal (Val.intuoffloat ars@ (pid, r1) )))) m
+    | Pfcvtzu X S rd r1 pid =>
+        MemSimNext ((ars@ (pid, rd)  <- (Val.maketotal (Val.longuofsingle ars@ (pid, r1) )))) m
+    | Pfcvtzu X D rd r1 pid =>
+        MemSimNext ((ars@ (pid, rd)  <- (Val.maketotal (Val.longuoffloat ars@ (pid, r1) )))) m
+    | Pscvtf S W rd r1 pid =>
+        MemSimNext ((ars@ (pid, rd)  <- (Val.maketotal (Val.singleofint ars@ (pid, r1) )))) m
+    | Pscvtf D W rd r1 pid =>
+        MemSimNext ((ars@ (pid, rd)  <- (Val.maketotal (Val.floatofint ars@ (pid, r1) )))) m
+    | Pscvtf S X rd r1 pid =>
+        MemSimNext ((ars@ (pid, rd)  <- (Val.maketotal (Val.singleoflong ars@ (pid, r1) )))) m
+    | Pscvtf D X rd r1 pid =>
+        MemSimNext ((ars@ (pid, rd)  <- (Val.maketotal (Val.floatoflong ars@ (pid, r1) )))) m
+    | Pucvtf S W rd r1 pid =>
+        MemSimNext ((ars@ (pid, rd)  <- (Val.maketotal (Val.singleofintu ars@ (pid, r1) )))) m
+    | Pucvtf D W rd r1 pid =>
+        MemSimNext ((ars@ (pid, rd)  <- (Val.maketotal (Val.floatofintu ars@ (pid, r1) )))) m
+    | Pucvtf S X rd r1 pid =>
+        MemSimNext ((ars@ (pid, rd)  <- (Val.maketotal (Val.singleoflongu ars@ (pid, r1) )))) m
+    | Pucvtf D X rd r1 pid =>
+        MemSimNext ((ars@ (pid, rd)  <- (Val.maketotal (Val.floatoflongu ars@ (pid, r1) )))) m
+    (** Floating-point arithmetic *)
+    | Pfabs S rd r1 pid =>
+        MemSimNext ((ars@ (pid, rd)  <- (Val.absfs ars@ (pid, r1) ))) m
+    | Pfabs D rd r1 pid =>
+        MemSimNext ((ars@ (pid, rd)  <- (Val.absf ars@ (pid, r1) ))) m
+    | Pfneg S rd r1 pid =>
+        MemSimNext ((ars@ (pid, rd)  <- (Val.negfs ars@ (pid, r1) ))) m
+    | Pfneg D rd r1 pid =>
+        MemSimNext ((ars@ (pid, rd)  <- (Val.negf ars@ (pid, r1) ))) m
+    | Pfadd S rd r1 r2 pid =>
+        MemSimNext ((ars@ (pid, rd)  <- (Val.addfs ars@ (pid, r1)  ars@ (pid, r2) ))) m
+    | Pfadd D rd r1 r2 pid =>
+        MemSimNext ((ars@ (pid, rd)  <- (Val.addf ars@ (pid, r1)  ars@ (pid, r2) ))) m
+    | Pfdiv S rd r1 r2 pid =>
+        MemSimNext ((ars@ (pid, rd)  <- (Val.divfs ars@ (pid, r1)  ars@ (pid, r2) ))) m
+    | Pfdiv D rd r1 r2 pid =>
+        MemSimNext ((ars@ (pid, rd)  <- (Val.divf ars@ (pid, r1)  ars@ (pid, r2) ))) m
+    | Pfmul S rd r1 r2 pid =>
+        MemSimNext ((ars@ (pid, rd)  <- (Val.mulfs ars@ (pid, r1)  ars@ (pid, r2) ))) m
+    | Pfmul D rd r1 r2 pid =>
+        MemSimNext ((ars@ (pid, rd)  <- (Val.mulf ars@ (pid, r1)  ars@ (pid, r2) ))) m
+    | Pfnmul S rd r1 r2 pid =>
+        MemSimNext ((ars@ (pid, rd)  <- (Val.negfs (Val.mulfs ars@ (pid, r1)  ars@ (pid, r2) )))) m
+    | Pfnmul D rd r1 r2 pid =>
+        MemSimNext ((ars@ (pid, rd)  <- (Val.negf (Val.mulf ars@ (pid, r1)  ars@ (pid, r2) )))) m
+    | Pfsub S rd r1 r2 pid =>
+        MemSimNext ((ars@ (pid, rd)  <- (Val.subfs ars@ (pid, r1)  ars@ (pid, r2) ))) m
+    | Pfsub D rd r1 r2 pid =>
+        MemSimNext ((ars@ (pid, rd)  <- (Val.subf ars@ (pid, r1)  ars@ (pid, r2) ))) m
+    (** Floating-point comparison *)
+    | Pfcmp S r1 r2 pid =>
+        MemSimNext ((compare_single ars ars@ (pid, r1)  ars@ (pid, r2) pid )) m
+    | Pfcmp D r1 r2 pid =>
+        MemSimNext ((compare_float ars ars@ (pid, r1)  ars@ (pid, r2) pid )) m
+    | Pfcmp0 S r1 pid =>
+        MemSimNext ((compare_single ars ars@ (pid, r1)  (Vsingle Float32.zero) pid)) m
+    | Pfcmp0 D r1 pid =>
+        MemSimNext ((compare_float ars ars@ (pid, r1)  (Vfloat Float.zero) pid)) m
+    (** Floating-point conditional select *)
+    | Pfsel rd r1 r2 cond pid =>
+        let v :=
+            match eval_testcond cond ars pid with
+            | Some true => ars@ (pid, r1) 
+            | Some false => ars@ (pid, r2) 
+            | None => Vundef
+            end in
+        MemSimNext ((ars@ (pid, rd)  <- v)) m
+    (** Pseudo-instructions *)
+    | Pallocframe sz pos pid =>
+        let (m1, stk) := Mem.alloc m 0 sz in
+        let sp := (Vptr stk Ptrofs.zero) in
+        match Mem.storev Mint64 m1 (Val.offset_ptr sp pos) ars@ (pid, SP)  with
+        | None => MemSimStuck
+        | Some m2 => MemSimNext ((ars @ (pid, X15) <- (ars@ (pid, SP) ) @(pid, SP) <- sp @(pid, X16) <- Vundef)) m2
+        end
+    | Pfreeframe sz pos pid =>
+        match Mem.loadv Mint64 m (Val.offset_ptr ars@ (pid, SP)  pos) with
+        | None => MemSimStuck
+        | Some v =>
+            match ars@ (pid, SP)  with
+            | Vptr stk ofs =>
+                match Mem.free m stk 0 sz with
+                | None => MemSimStuck
+                | Some m' => MemSimNext ((ars@ (pid, SP)  <- v @(pid, X16) <- Vundef)) m'
+                end
+            | _ => MemSimStuck
+            end
+        end
+    | Plabel lbl pid =>
+        MemSimNext ars m
+    | Ploadsymbol rd id pid =>
+        MemSimNext ((ars@ (pid, rd)  <- (Genv.symbol_address ge id Ptrofs.zero))) m
+    | Pcvtsw2x rd r1 pid =>
+        MemSimNext ((ars@ (pid, rd)  <- (Val.longofint ars@ (pid, r1) ))) m
+    | Pcvtuw2x rd r1 pid =>
+        MemSimNext ((ars@ (pid, rd)  <- (Val.longofintu ars@ (pid, r1) ))) m
+    | Pcvtx2w rd pid =>
+        MemSimNext ((ars@ (pid, rd)  <- (Val.loword ars@ (pid, rd) ))) m
+    | Pbtbl r tbl pid =>
+        match (ars@ (pid, X16)  <- Vundef)@(pid, r) with
+        | Vint n =>
+            match list_nth_z tbl (Int.unsigned n) with
+            | None => MemSimStuck
+            | Some lbl => goto_label f lbl (ars@ (pid, X16) <- Vundef) pid m
+            end
+        | _ => MemSimStuck
+        end
+    | Pcfi_rel_offset _ pid =>
+        MemSimNext ars m
+    | Pbuiltin ef args res pid => MemSimStuck    (**r treated specially below *)
+    (** The following instructions and directives are not generated directly
+        by Asmgen, so we do not model them. *)
+    | Pldp _ _ _ _ => MemSimStuck
+    | Pstp _ _ _ _  => MemSimStuck
+    | Pcls _ _ _ _ => MemSimStuck
+    | Pclz _ _ _ _ => MemSimStuck
+    | Prev _ _ _ _ => MemSimStuck
+    | Prev16 _ _ _ _ => MemSimStuck
+    | Prbit _ _ _ _ => MemSimStuck
+    | Pfsqrt _ _ _ _ => MemSimStuck
+    | Pfmadd _ _ _ _ _ _ => MemSimStuck
+    | Pfmsub _ _ _ _ _ _ => MemSimStuck
+    | Pfnmadd _ _ _ _ _ _ => MemSimStuck
+    | Pfnmsub _ _ _ _ _ _ => MemSimStuck
+    | Pfmax _ _ _ _ _ => MemSimStuck
+    | Pfmin _ _ _ _ _ => MemSimStuck
+    | Pnop _ => MemSimStuck
+    | Pincpc pid => MemSimNext (ars@(pid, PC) <- (Val.offset_ptr ars@(pid,PC) Ptrofs.one)) m
+    | Pcfi_adjust _ _ =>
+        MemSimStuck
+    end.
+
+
+(** Execution of the instruction at [rs@PC]. *)
+
+End RELSEM.
+
+
+
+
+
+
+(** asm to mem sim - turns ISA into a series of memsim semantics*)
+(** separates most operations into the actual operation and incrementing the PC - this lets us reorder more easily since we 
+dont update the PC in every operation*)
+
+(** translates loads/stores into memory dispatches and acknowledgements*)
+(** Takes in a processor id*)
+Definition asm_to_memsim (asm_i: Asm.instruction) (pid: processor_id): list instruction := 
+    match asm_i with 
+    | Asm.Pb lbl    => [Pb lbl pid]                                               (**r branch *)
+    | Asm.Pbc c lbl  => [Pbc c lbl pid; Pincpc pid]                             (**r conditional branch *)
+    | Asm.Pbl id sg  => [Pbl id sg pid]                              (**r jump to function and link *)
+    | Asm.Pbs id sg => [Pbs id sg pid]                                  (**r jump to function *)
+    | Asm.Pblr r sg => [Pblr r sg pid]                                 (**r indirect jump and link *)
+    | Asm.Pbr r sg => [Pbr r sg pid]                                   (**r indirect jump *)
+    | Asm.Pret r => [Pret r pid]                                        (**r return *)
+    | Asm.Pcbnz sz r lbl => [Pcbnz sz r lbl pid; Pincpc pid]                       (**r branch if not zero *)
+    | Asm.Pcbz sz r lbl => [Pcbz sz r lbl pid; Pincpc pid]                         (**r branch if zero *)
+    | Asm.Ptbnz sz r n lbl => [Ptbnz sz r n lbl pid; Pincpc pid]                   (**r branch if bit n is not zero *)
+    | Asm.Ptbz sz r n lbl => [Ptbz sz r n lbl pid; Pincpc pid]                     (**r branch if bit n is zero *)
+    | Asm.Pldrw rd a => [Pldrw rd a pid; Pincpc pid]                               (**r load int32 *)
+    | Asm.Pldrw_a rd a => [Pldrw_a rd a pid; Pincpc pid]                           (**r load int32 as any32 *)
+    | Asm.Pldrx rd a => [Pldrx rd a pid; Pincpc pid]                               (**r load int64 *)
+    | Asm.Pldrx_a rd a => [Pldrx_a rd a pid; Pincpc pid]                           (**r load int64 as any64 *)
+    | Asm.Pldrb sz rd a => [Pldrb sz rd a pid; Pincpc pid]                         (**r load int8, zero-extend *)
+    | Asm.Pldrsb sz rd a => [Pldrsb sz rd a pid; Pincpc pid]                       (**r load int8, sign-extend *)
+    | Asm.Pldrh sz rd a => [Pldrh sz rd a pid; Pincpc pid]                         (**r load int16, zero-extend *)
+    | Asm.Pldrsh sz rd a => [Pldrsh sz rd a pid; Pincpc pid]                       (**r load int16, sign-extend *)
+    | Asm.Pldrzw rd a => [Pldrzw rd a pid; Pincpc pid]                             (**r load int32, zero-extend to int64 *)
+    | Asm.Pldrsw rd a => [Pldrsw rd a pid; Pincpc pid]                             (**r load int32, sign-extend to int64 *)
+    | Asm.Pldp rd1 rd2 a => [Pldp rd1 rd2 a pid; Pincpc pid]                       (**r load two int64 *)
+    | Asm.Pstrw rs a => [Pstrw rs a pid; Pincpc pid]                               (**r store int32 *)
+    | Asm.Pstrw_a rs a => [Pstrw_a rs a pid; Pincpc pid]                           (**r store int32 as any32 *)
+    | Asm.Pstrx rs a => [Pstrx rs a pid; Pincpc pid]                               (**r store int64 *)
+    | Asm.Pstrx_a rs a => [Pstrx_a rs a pid; Pincpc pid]                           (**r store int64 as any64 *)
+    | Asm.Pstrb rs a => [Pstrb rs a pid; Pincpc pid]                               (**r store int8 *)
+    | Asm.Pstrh rs a => [Pstrh rs a pid; Pincpc pid]                               (**r store int16 *)
+    | Asm.Pstp rs1 rs2 a => [Pstp rs1 rs2 a pid; Pincpc pid]                       (**r store two int64 *)
+    | Asm.Paddimm sz rd r1 n => [Paddimm sz rd r1 n pid; Pincpc pid]               (**r addition *)
+    | Asm.Psubimm sz rd r1 n => [Psubimm sz rd r1 n pid; Pincpc pid]               (**r subtraction *)
+    | Asm.Pcmpimm sz r1 n => [Pcmpimm sz r1 n pid; Pincpc pid]                     (**r compare *)
+    | Asm.Pcmnimm sz r1 n => [Pcmnimm sz r1 n pid; Pincpc pid]                     (**r compare negative *)
+    | Asm.Pmov rd r1 => [Pmov rd r1 pid; Pincpc pid]                               (**r move integer register *)
+    | Asm.Pandimm sz rd r1 n => [Pandimm sz rd r1 n pid; Pincpc pid]               (**r and *)
+    | Asm.Peorimm sz rd r1 n => [Peorimm sz rd r1 n pid; Pincpc pid]               (**r xor *)
+    | Asm.Porrimm sz rd r1 n => [Porrimm sz rd r1 n pid; Pincpc pid]               (**r or *)
+    | Asm.Ptstimm sz r1 n => [Ptstimm sz r1 n pid; Pincpc pid]                     (**r and, then set flags *)
+    | Asm.Pmovz sz rd n pos => [Pmovz sz rd n pos pid; Pincpc pid]                 (**r move wide immediate *)
+    | Asm.Pmovn sz rd n pos => [Pmovn sz rd n pos pid; Pincpc pid]
+    | Asm.Pmovk sz rd n pos => [Pmovk sz rd n pos pid; Pincpc pid]
+    | Asm.Padrp rd id ofs => [Padrp rd id ofs pid; Pincpc pid]                     (**r PC-relative addressing *)
+    | Asm.Paddadr rd r1 id ofs => [Paddadr rd r1 id ofs pid; Pincpc pid]
+    | Asm.Psbfiz sz rd r1 r s => [Psbfiz sz rd r1 r s pid; Pincpc pid]              (**r Bit-field operations *)
+    | Asm.Psbfx sz rd r1 r s => [Psbfx sz rd r1 r s pid; Pincpc pid]
+    | Asm.Pubfiz sz rd r1 r s => [Pubfiz sz rd r1 r s pid; Pincpc pid]
+    | Asm.Pubfx sz rd r1 r s => [Pubfx sz rd r1 r s pid; Pincpc pid]
+    | Asm.Padd sz rd r1 r2 s => [Padd sz rd r1 r2 s pid; Pincpc pid]                (**r Integer arithmetic, shifted register *)
+    | Asm.Psub sz rd r1 r2 s => [Psub sz rd r1 r2 s pid; Pincpc pid]
+    | Asm.Pcmp sz r1 r2 s => [Pcmp sz r1 r2 s pid; Pincpc pid]
+    | Asm.Pcmn sz r1 r2 s => [Pcmn sz r1 r2 s pid; Pincpc pid]
+    | Asm.Paddext rd r1 r2 x => [Paddext rd r1 r2 x pid; Pincpc pid]                (**r Integer arithmetic, extending register *)
+    | Asm.Psubext rd r1 r2 x => [Psubext rd r1 r2 x pid; Pincpc pid]
+    | Asm.Pcmpext r1 r2 x => [Pcmpext r1 r2 x pid; Pincpc pid]
+    | Asm.Pcmnext r1 r2 x => [Pcmnext r1 r2 x pid; Pincpc pid]
+    | Asm.Pand sz rd r1 r2 s => [Pand sz rd r1 r2 s pid; Pincpc pid]                (**r Logical, shifted register *)
+    | Asm.Pbic sz rd r1 r2 s => [Pbic sz rd r1 r2 s pid; Pincpc pid]
+    | Asm.Peon sz rd r1 r2 s => [Peon sz rd r1 r2 s pid; Pincpc pid]
+    | Asm.Peor sz rd r1 r2 s => [Peor sz rd r1 r2 s pid; Pincpc pid]
+    | Asm.Porr sz rd r1 r2 s => [Porr sz rd r1 r2 s pid; Pincpc pid]
+    | Asm.Porn sz rd r1 r2 s => [Porn sz rd r1 r2 s pid; Pincpc pid]
+    | Asm.Ptst sz r1 r2 s => [Ptst sz r1 r2 s pid; Pincpc pid]                      (**r and, then set flags *)
+    | Asm.Pasrv sz rd r1 r2 => [Pasrv sz rd r1 r2 pid; Pincpc pid]                  (**r Variable shifts *)
+    | Asm.Plslv sz rd r1 r2 => [Plslv sz rd r1 r2 pid; Pincpc pid]
+    | Asm.Plsrv sz rd r1 r2 => [Plsrv sz rd r1 r2 pid; Pincpc pid]
+    | Asm.Prorv sz rd r1 r2 => [Prorv sz rd r1 r2 pid; Pincpc pid]
+    | Asm.Pcls sz rd r1 => [Pcls sz rd r1 pid; Pincpc pid]                          (**r Bit operations *)
+    | Asm.Pclz sz rd r1 => [Pclz sz rd r1 pid; Pincpc pid]
+    | Asm.Prev sz rd r1 => [Prev sz rd r1 pid; Pincpc pid]
+    | Asm.Prev16 sz rd r1 => [Prev16 sz rd r1 pid; Pincpc pid]
+    | Asm.Prbit sz rd r1 => [Prbit sz rd r1 pid; Pincpc pid]
+    | Asm.Pcsel rd r1 r2 c => [Pcsel rd r1 r2 c pid; Pincpc pid]                    (**r Conditional data processing *)
+    | Asm.Pcset rd c => [Pcset rd c pid; Pincpc pid]
+    | Asm.Pmadd sz rd r1 r2 r3 => [Pmadd sz rd r1 r2 r3 pid; Pincpc pid]            (**r Integer multiply/divide *)
+    | Asm.Pmsub sz rd r1 r2 r3 => [Pmsub sz rd r1 r2 r3 pid; Pincpc pid]
+    | Asm.Psmulh rd r1 r2 => [Psmulh rd r1 r2 pid; Pincpc pid]
+    | Asm.Pumulh rd r1 r2 => [Pumulh rd r1 r2 pid; Pincpc pid]
+    | Asm.Psdiv sz rd r1 r2 => [Psdiv sz rd r1 r2 pid; Pincpc pid]
+    | Asm.Pudiv sz rd r1 r2 => [Pudiv sz rd r1 r2 pid; Pincpc pid]
+    | Asm.Pldrs rd a => [Pldrs rd a pid; Pincpc pid]                                (**r Floating-point loads and stores *)
+    | Asm.Pldrd rd a => [Pldrd rd a pid; Pincpc pid]
+    | Asm.Pldrd_a rd a => [Pldrd_a rd a pid; Pincpc pid]
+    | Asm.Pstrs rs a => [Pstrs rs a pid; Pincpc pid]
+    | Asm.Pstrd rs a => [Pstrd rs a pid; Pincpc pid]
+    | Asm.Pstrd_a rs a => [Pstrd_a rs a pid; Pincpc pid]
+    | Asm.Pfmov rd r1 => [Pfmov rd r1 pid; Pincpc pid]                              (**r Floating-point move *)
+    | Asm.Pfmovimms rd f => [Pfmovimms rd f pid; Pincpc pid]
+    | Asm.Pfmovimmd rd f => [Pfmovimmd rd f pid; Pincpc pid]
+    | Asm.Pfmovi fsz rd r1 => [Pfmovi fsz rd r1 pid; Pincpc pid]
+    | Asm.Pfcvtds rd r1 => [Pfcvtds rd r1 pid; Pincpc pid]                          (**r Floating-point conversions *)
+    | Asm.Pfcvtsd rd r1 => [Pfcvtsd rd r1 pid; Pincpc pid]
+    | Asm.Pfcvtzs isz fsz rd r1 => [Pfcvtzs isz fsz rd r1 pid; Pincpc pid]
+    | Asm.Pfcvtzu isz fsz rd r1 => [Pfcvtzu isz fsz rd r1 pid; Pincpc pid]
+    | Asm.Pscvtf fsz isz rd r1 => [Pscvtf fsz isz rd r1 pid; Pincpc pid]
+    | Asm.Pucvtf fsz isz rd r1 => [Pucvtf fsz isz rd r1 pid; Pincpc pid]
+    | Asm.Pfabs sz rd r1 => [Pfabs sz rd r1 pid; Pincpc pid]                        (**r Floating-point arithmetic *)
+    | Asm.Pfneg sz rd r1 => [Pfneg sz rd r1 pid; Pincpc pid]
+    | Asm.Pfsqrt sz rd r1 => [Pfsqrt sz rd r1 pid; Pincpc pid]
+    | Asm.Pfadd sz rd r1 r2 => [Pfadd sz rd r1 r2 pid; Pincpc pid]
+    | Asm.Pfdiv sz rd r1 r2 => [Pfdiv sz rd r1 r2 pid; Pincpc pid]
+    | Asm.Pfmul sz rd r1 r2 => [Pfmul sz rd r1 r2 pid; Pincpc pid]
+    | Asm.Pfnmul sz rd r1 r2 => [Pfnmul sz rd r1 r2 pid; Pincpc pid]
+    | Asm.Pfsub sz rd r1 r2 => [Pfsub sz rd r1 r2 pid; Pincpc pid]
+    | Asm.Pfmadd sz rd r1 r2 r3 => [Pfmadd sz rd r1 r2 r3 pid; Pincpc pid]
+    | Asm.Pfmsub sz rd r1 r2 r3 => [Pfmsub sz rd r1 r2 r3 pid; Pincpc pid]
+    | Asm.Pfnmadd sz rd r1 r2 r3 => [Pfnmadd sz rd r1 r2 r3 pid; Pincpc pid]
+    | Asm.Pfnmsub sz rd r1 r2 r3 => [Pfnmsub sz rd r1 r2 r3 pid; Pincpc pid]
+    | Asm.Pfmax sz rd r1 r2 => [Pfmax sz rd r1 r2 pid; Pincpc pid]
+    | Asm.Pfmin sz rd r1 r2 => [Pfmin sz rd r1 r2 pid; Pincpc pid]
+    | Asm.Pfcmp sz r1 r2 => [Pfcmp sz r1 r2 pid; Pincpc pid]                        (**r Floating-point comparison *)
+    | Asm.Pfcmp0 sz r1 => [Pfcmp0 sz r1 pid; Pincpc pid]
+    | Asm.Pfsel rd r1 r2 cond => [Pfsel rd r1 r2 cond pid; Pincpc pid]              (**r Floating-point conditional select *)
+    | Asm.Pallocframe sz linkofs => [Pallocframe sz linkofs pid; Pincpc pid]       (**r Pseudo-instructions *)
+    | Asm.Pfreeframe sz linkofs => [Pfreeframe sz linkofs pid; Pincpc pid]
+    | Asm.Plabel lbl => [Plabel lbl pid; Pincpc pid]
+    | Asm.Ploadsymbol rd id => [Ploadsymbol rd id pid; Pincpc pid]
+    | Asm.Pcvtsw2x rd r1 => [Pcvtsw2x rd r1 pid; Pincpc pid]
+    | Asm.Pcvtuw2x rd r1 => [Pcvtuw2x rd r1 pid; Pincpc pid]
+    | Asm.Pcvtx2w rd => [Pcvtx2w rd pid; Pincpc pid]
+    | Asm.Pbtbl r1 tbl => [Pbtbl r1 tbl pid; Pincpc pid]
+    | Asm.Pbuiltin ef args res => [Pbuiltin ef args res pid; Pincpc pid]
+    | Asm.Pnop => [Pnop pid; Pincpc pid]                                              (**r no operation *)
+    | Asm.Pcfi_adjust ofs => [Pcfi_adjust ofs pid; Pincpc pid]
+    | Asm.Pcfi_rel_offset ofs => [Pcfi_rel_offset ofs pid; Pincpc pid]                                
+end.
+
+(** What to do if a goto forces early abort of a list? have the individual eval_memsim_instr return a state for early abort*)
+Fixpoint eval_memsim_chain (g: genv)(f: function)(instrs: list instruction)  (ars: allregsets)  (m: mem): outcome := 
+    match instrs with
+    | nil => MemSimNext ars m
+    | instr :: chain' =>
+        match eval_memsim_instr g f instr ars m with
+        | MemSimNext ars' m' => eval_memsim_chain g f chain' ars' m'
+        | MemSimJumpOut ars' m' => MemSimJumpOut ars' m'
+        | MemSimStuck => MemSimStuck
+        end
+    end.
+
+(** Proof boilerplate: move to another file asap*)
+
+(** ** Simplify matches when possible *)
+
+Ltac simpl_match :=
+  let repl_match_goal d d' :=
+      replace d with d';
+      lazymatch goal with
+      | [ |- context[match d' with _ => _ end] ] => fail
+      | _ => idtac
+      end in
+  let repl_match_hyp H d d' :=
+      replace d with d' in H;
+      lazymatch type of H with
+      | context[match d' with _ => _ end] => fail
+      | _ => idtac
+      end in
+  match goal with
+  | [ Heq: ?d = ?d' |- context[match ?d with _ => _ end] ] =>
+    repl_match_goal d d'
+  | [ Heq: ?d' = ?d |- context[match ?d with _ => _ end] ] =>
+    repl_match_goal d d'
+  | [ Heq: ?d = ?d', H: context[match ?d with _ => _ end] |- _ ] =>
+    repl_match_hyp H d d'
+  | [ Heq: ?d' = ?d, H: context[match ?d with _ => _ end] |- _ ] =>
+    repl_match_hyp H d d'
+  end.
+
+
+(** ** Find and destruct matches *)
+
+Ltac destruct_matches_in e :=
+  lazymatch e with
+  | context[match ?d with | _ => _ end] =>
+    destruct_matches_in d
+  | _ => destruct e eqn:?; intros
+  end.
+
+Ltac destruct_all_matches :=
+  repeat (try simpl_match;
+          try match goal with
+              | [ |- context[match ?d with | _ => _ end] ] =>
+                destruct_matches_in d
+              | [ H: context[match ?d with | _ => _ end] |- _ ] =>
+                destruct_matches_in d
+              end);
+  subst;
+  try congruence;
+  auto.
+
+Ltac destruct_nongoal_matches :=
+  repeat (try simpl_match;
+           try match goal with
+           | [ H: context[match ?d with | _ => _ end] |- _ ] =>
+             destruct_matches_in d
+               end);
+  subst;
+  try congruence;
+  auto.
+
+Ltac destruct_goal_matches :=
+  repeat (try simpl_match;
+           match goal with
+           | [ |- context[match ?d with | _ => _ end] ] =>
+              destruct_matches_in d
+           end);
+  try congruence;
+  auto.
+
+Ltac destruct_tuple :=
+  match goal with
+  | [ H: context[let '(a, b) := ?p in _] |- _ ] =>
+    let a := fresh a in
+    let b := fresh b in
+    destruct p as [a b]
+  | [ |- context[let '(a, b) := ?p in _] ] =>
+    let a := fresh a in
+    let b := fresh b in
+    destruct p as [a b]
+  end.
+
+Tactic Notation "destruct" "matches" "in" "*" := destruct_all_matches.
+Tactic Notation "destruct" "matches" "in" "*|-" := destruct_nongoal_matches.
+Tactic Notation "destruct" "matches" := destruct_goal_matches.
+
+
+Definition regs_identical (ars: allregsets) (pid: processor_id) (rs: regset): Prop :=
+    forall r, rs r = ars@(pid, r).
+
+Remark vptr_equality: forall b1 b2 o1 o2, b1=b2 /\ o1 = o2 -> Vptr b1 o1 = Vptr b2 o2.
+Proof. intros. destruct H. rewrite H. rewrite H0. reflexivity. Qed.
+
+Remark inverse_vptr_equality: forall b1 b2 o1 o2,  Vptr b1 o1 = Vptr b2 o2 -> b1=b2 /\ o1 = o2.
+Proof. intros. inversion H. split; reflexivity. Qed.
+
+
+Remark tup_equal: forall (a c: processor_id) (b d: preg), a = c /\ b = d -> (a, b) = (c, d).
+Proof. intros. destruct H. rewrite H. rewrite H0. reflexivity. Qed.
+
+Remark preg_neq: forall (a b: preg), a <> b -> a = b -> False.
+Proof.
+    intros. rewrite H0 in H. apply H. reflexivity.
+Qed.
+
+Remark set_method_semantic_equality: forall rs (pid: processor_id) (r1 r2: preg) (v: val)  ars, 
+    regs_identical ars pid rs ->  regs_identical ars@(pid, r1)<-v pid rs#r1<-v.
+    Proof. 
+    intros. unfold regs_identical in H. unfold regs_identical. intro.
+    
+    unfold Asm.Pregmap.set. unfold PRmap.set. 
+    destruct (PregEq.eq r r1).
+    - subst. destruct (PREq.eq (pid, r1)(pid, r1)). reflexivity. contradiction.
+    - destruct (PREq.eq (pid, r) (pid, r1)). inversion e. contradiction. apply H.
+Qed.
+
+Remark set_method_sem_eq_form2: forall (pid: processor_id)(pr k: preg)(rs: regset)(ars: allregsets)(v: val),
+ regs_identical ars pid rs -> rs # k <- v pr = ars @ (pid, k) <- v (pid, pr).
+ Proof.
+    intros. unfold regs_identical in H. unfold Asm.Pregmap.set. unfold PRmap.set. destruct (PregEq.eq k pr).
+    - subst. destruct (PREq.eq (pid, pr) (pid, pr)). destruct (PregEq.eq pr pr). reflexivity. contradiction.
+    unfold not in n. contradiction.
+    -destruct (PregEq.eq pr k). rewrite <- e in n. contradiction. destruct (PREq.eq (pid, pr) (pid, k)).
+    inversion e. contradiction. apply H.
+ Qed.
+
+ Remark set_method_sem_eq_form3: forall (pid: processor_id)(pr k: preg)(rs: regset)(ars: allregsets)(v1 v2: val),
+ regs_identical ars pid rs -> v1 = v2 -> rs # k <- v1 pr = ars @ (pid, k) <- v2 (pid, pr).
+ Proof.
+    intros. unfold regs_identical in H. unfold Asm.Pregmap.set. rewrite <- H0. unfold PRmap.set. destruct (PregEq.eq k pr).
+    - subst. destruct (PREq.eq (pid, pr) (pid, pr)). destruct (PregEq.eq pr pr). reflexivity. contradiction.
+    unfold not in n. contradiction.
+    -destruct (PregEq.eq pr k). rewrite <- e in n. contradiction. destruct (PREq.eq (pid, pr) (pid, k)).
+    inversion e. contradiction. apply H.
+ Qed.
+
+
+
+(** Definition of the end state of an asm instruction in terms of the memsim outcome*)
+
+Definition end_state_equals_asm_memsim (r: preg)(asm_o: Asm.outcome) (memsim_o: outcome) (pid: processor_id): Prop :=
+    match asm_o, memsim_o with
+    | Next rs m1, MemSimNext ars m2 => rs r = (ars @ (pid, r)) /\ m1 = m2
+    | Next rs m1, MemSimJumpOut ars m2 => rs r = (ars @ (pid, r)) /\ m1 = m2
+    | Stuck, MemSimStuck => True
+    | _, _ => False
+    end.
+
+(* Ltac sem_eq_solver :=
+    match goal with
+    | [ H : regs_identical ?ars ?pid ?rs
+        |- Pregmap.set ?write_reg _ ?rs ?read_reg = PRmap.set (?pid, ?write_reg) _ ?ars (?pid, ?read_reg)
+    ] => apply set_method_sem_eq_form3; [ apply H | unfold regs_identical in H; specialize (H write_reg) as H_store_eq; sem_eq_solver]
+    | [H1 : ?rs ?reg = Vptr ?b1 ?i1, H2: ?ars (?pid, ?reg) = Vptr ?b2 ?i2, H_store_eq: ?rs ?reg = ?ars (?pid, ?reg) 
+        |- Vptr ?b1 ?z = Vptr ?b2 ?z] => rewrite -> H_store_eq in H1; rewrite -> H2 in H1; inversion H1; reflexivity
+    | [H_store_eq: ?rs ?reg = ?ars (?pid, ?reg) 
+        |- ?a (?rs ?reg) ?c = ?a (?ars (?pid, ?reg)) ?c] => rewrite -> H_store_eq; reflexivity
+    end. *)
+
+Remark cancel_dual_ptr_increments: forall (rs: regset) (ars: allregsets) (pid: processor_id) (v: ptrofs)(r: preg),
+   rs # r = ars @ (pid, r) -> Val.offset_ptr (rs r) v = Val.offset_ptr (ars (pid, r)) v.
+   Proof.
+   intros. rewrite <- H. reflexivity.
+   Qed.
+
+Remark eq_implies_set_eq: forall  (rs: regset) (ars: allregsets) (pid: processor_id) (write_reg read_reg: preg) (v1 v2: val),
+    rs read_reg = ars (pid, read_reg) -> v1 = v2 -> (rs # write_reg <- v1) read_reg = (ars @ (pid, write_reg) <- v2) (pid, read_reg).
+    Proof. intros. rewrite <- H0. unfold Asm.Pregmap.set. unfold PRmap.set. rewrite H. destruct (PregEq.eq read_reg write_reg); destruct (PREq.eq (pid, read_reg)(pid, write_reg)).
+      reflexivity. destruct n. rewrite <- e. reflexivity. destruct n. inversion e. reflexivity. reflexivity.
+Qed.
+
+Remark invert_shll: forall (rs: regset) (v1 v2: val) (r: preg) (pid: processor_id) (ars: allregsets),
+    (rs r) = (ars (pid, r)) -> v1 = v2 -> Val.shll (rs r) v1 = Val.shll (ars (pid, r)) v2.
+    Proof. intros. rewrite H. rewrite H0. reflexivity. Qed. 
+
+Remark long_of_int: forall (v1 v2: val),
+    v1 = v2 -> Val.longofintu v1 = Val.longofintu v2.
+    Proof. intros. rewrite H. reflexivity. Qed. 
+
+(* Ltac sem_eq_solver := 
+    match goal with
+    | [ |- ?x = ?x ] => reflexivity (*Terminal*)
+    | [H: regs_identical ?ars ?pid ?rs |- regs_identical ?ars ?pid ?rs] => apply H (*Terminal*)
+    | [Hri: forall r: PregEq.t, ?rs r = ?ars (?pid, r)    |- ?rs ?r = ?ars (?pid, ?r) ] => apply Hri (*Terminal*)
+    | [H1 : ?rs ?reg = Vptr ?b1 ?i1, H2: ?ars (?pid, ?reg) = Vptr ?b2 ?i2, Hri: forall r: PregEq.t, ?rs r = ?ars (?pid, r) 
+        |- Vptr ?b1 ?z = Vptr ?b2 ?z] => specialize (Hri reg); rewrite -> Hri in H1; rewrite -> H2 in H1; inversion H1; reflexivity  (*Terminal*)
+    | [ |- Val.offset_ptr _ ?v = Val.offset_ptr _ ?v] => apply cancel_dual_ptr_increments; sem_eq_solver
+    | [ |- regs_identical _ _ _] => unfold regs_identical; intro; sem_eq_solver
+    | [ |- Pregmap.set ?r1 _ ?rs ?r2 = PRmap.set (?pid, ?r1) _ ?ars (?pid, ?r2)] => apply eq_implies_set_eq; sem_eq_solver
+    | [ H: forall r: PregEq.t, ?rs r = ?ars (?pid, r),
+    Ha1: Val.addl (?rs ?r1) _ = Vptr ?b1 ?i1, 
+    Ha2: Val.addl (?ars (?pid, ?r1)) _ = Vptr ?b2 ?i2
+    |- ?v1 = ?v2] => pose proof H as Hdup; specialize (Hdup r1); rewrite <- Hdup in Ha2; sem_eq_solver
+    | [ H: forall r: PregEq.t, ?rs r = ?ars (?pid, r),
+    Ha1: Val.addl _ (?rs ?r1) = Vptr ?b1 ?i1, 
+    Ha2: Val.addl _ (?ars (?pid, ?r1)) = Vptr ?b2 ?i2
+    |- ?v1 = ?v2] => pose proof H as Hdupdup; specialize (Hdupdup r1); rewrite <- Hdupdup in Ha2; sem_eq_solver
+    | [ Ha1: ?op ?e1 ?e2 = Vptr ?b1 ?i1, 
+        Ha2: ?op ?e1 ?e2 = Vptr ?b2 ?i2,
+        Ha3: _ _ ?m ?b1 (Ptrofs.unsigned ?i1) = Some ?v1,
+        Ha4:  _ _ ?m ?b2 (Ptrofs.unsigned ?i2) = Some ?v2
+    |- ?v1 = ?v2] => rewrite -> Ha1 in Ha2; inversion Ha2; subst; rewrite -> Ha3 in Ha4; inversion Ha4; reflexivity (*Terminal*)
+    | [ |- Val.shll _ ?v1 = Val.shll _ ?v2] => apply invert_shll; sem_eq_solver
+    | _ => idtac
+    end. *)
+
+(* Ltac sem_eq_solver := 
+    match goal with
+    | [ |- ?x = ?x ] => reflexivity (*Terminal*)
+    | [H: regs_identical ?ars ?pid ?rs |- regs_identical ?ars ?pid ?rs] => apply H (*Terminal*)
+    | [Hri: forall r: PregEq.t, ?rs r = ?ars (?pid, r)    |- ?rs ?r = ?ars (?pid, ?r) ] => apply Hri (*Terminal*)
+    | [H1 : ?rs ?reg = Vptr ?b1 ?i1, H2: ?ars (?pid, ?reg) = Vptr ?b2 ?i2, Hri: forall r: PregEq.t, ?rs r = ?ars (?pid, r) 
+        |- Vptr ?b1 ?z = Vptr ?b2 ?z] => specialize (Hri reg); rewrite -> Hri in H1; rewrite -> H2 in H1; inversion H1; reflexivity  (*Terminal*)
+    | [ |- Val.offset_ptr _ ?v = Val.offset_ptr _ ?v] => apply cancel_dual_ptr_increments; sem_eq_solver
+    | [ |- regs_identical _ _ _] => unfold regs_identical; intro; sem_eq_solver
+    | [ |- Pregmap.set ?r1 _ ?rs ?r2 = PRmap.set (?pid, ?r1) _ ?ars (?pid, ?r2)] => apply eq_implies_set_eq; sem_eq_solver
+    | [ Ha1: ?op ?e1 ?e2 = Vptr ?b1 ?i1, 
+        Ha2: ?op ?e1 ?e2 = Vptr ?b2 ?i2,
+        Ha3: _ _ ?m ?b1 (Ptrofs.unsigned ?i1) = Some ?v1,
+        Ha4:  _ _ ?m ?b2 (Ptrofs.unsigned ?i2) = Some ?v2
+    |- ?v1 = ?v2] => rewrite -> Ha1 in Ha2; inversion Ha2; subst; rewrite -> Ha3 in Ha4; inversion Ha4; reflexivity (*Terminal*)
+    | [ Ha1: ?op ?e1 ?e2 = Vptr ?b1 ?i1, 
+    Ha2: ?op ?e1 ?e2 = Vptr ?b2 ?i2,
+    Ha3: _ _ ?m ?b1 (Ptrofs.unsigned ?i1) = Some ?v1,
+    Ha4:  _ _ ?m ?b2 (Ptrofs.unsigned ?i2) = Some ?v2
+    |- _ ?v1 = _ ?v2] => rewrite -> Ha1 in Ha2; inversion Ha2; subst; rewrite -> Ha3 in Ha4; inversion Ha4; reflexivity (*Terminal*)
+    | [ |- Val.shll _ ?v1 = Val.shll _ ?v2] => apply invert_shll; sem_eq_solver
+    | _ => idtac
+    end. *)
+
+Remark set_sem_eq : 
+    forall (rs: regset) (ars: allregsets) (pid: processor_id) (r read_reg: preg) (v: val),
+    regs_identical ars pid rs -> (rs # r <- v) read_reg = (ars @ (pid, r) <- v) (pid, read_reg).
+    Proof. intros. unfold regs_identical in H. unfold Asm.Pregmap.set. unfold PRmap.set. destruct PregEq.eq; destruct PREq.eq. reflexivity. 
+    destruct n. rewrite e. reflexivity. destruct n. inversion e. reflexivity.
+    apply H. 
+    Qed.
+
+Ltac sem_eq_solver :=
+    match goal with
+    (*Identity*)
+    [ |- ?x = ?x ] => reflexivity (*Terminal*)
+    (*Prereq of a proof we already did upon entry*)
+    | [H: regs_identical ?ars ?pid ?rs |- regs_identical ?ars ?pid ?rs] => apply H (*Terminal*)
+    (*Gradually replace memsim regs with Asm regs*)
+    | [H: forall r: PregEq.t, ?rs r = ?ars (?pid, r), 
+          H2: context[?ars (?pid, ?r2)],
+          H3: context[?rs ?r2] |- _] => pose proof H as Hdup3;  specialize (Hdup3 r2); rewrite <- Hdup3 in H2; clear Hdup3; sem_eq_solver (*Nonterminal*)
+    (*Replace in goal as well*)
+    | [H: forall r: PregEq.t, ?rs r = ?ars (?pid, r)
+        |- context[?ars (?pid, ?r2)]] => pose proof H as Hdup3;  specialize (Hdup3 r2); rewrite <- Hdup3; clear Hdup3; sem_eq_solver (*Nonterminal*)
+    (* Set equivalent*)
+    | [ |- Pregmap.set ?r ?v ?rs ?r2 = PRmap.set (?pid, ?r) ?v ?ars (?pid, ?r2)] => apply set_sem_eq; sem_eq_solver (*Nonterminal*)
+    (*Replace like hypotheses*)
+    | [H1: ?x = ?y, H2: ?x = ?z |- _ ] => rewrite H1 in H2; sem_eq_solver (*Nonterminal*)
+    (*Break apart optional*)
+    | [H: Some ?v = Some ?v2 |- _] => inversion H; clear H; subst; sem_eq_solver (*Nonterminal*) 
+    (*Pointer inversion*)
+    | [H1: ?x = Vptr ?b1 ?i1,
+       H2: ?x = Vptr ?b2 ?i2
+       |- _ ] => rewrite -> H1 in H2; inversion H2; clear H2; subst; sem_eq_solver (*Nonterminal*)
+    (*Pointer inversion*)
+    | [H1: Vptr ?b1 ?i1 = Vptr ?b2 ?i2 |- _] => inversion H1; clear H1; subst; sem_eq_solver (*Nonterminal*)
+    | [ |- Val.offset_ptr ?v1 ?n = Val.offset_ptr ?v2 ?n] => apply cancel_dual_ptr_increments; sem_eq_solver (*Nonterminal*)
+    | _ => idtac
+    end.
+
+Theorem asm_identical_to_forward_sim: forall (pr: preg) (g: genv)(f: function) (i: Asm.instruction) (rs: regset) (ars: allregsets) (m: mem) (pid: processor_id), 
+    regs_identical ars pid rs -> end_state_equals_asm_memsim pr (exec_instr g f i rs  m)  (eval_memsim_chain g f (asm_to_memsim i pid) ars m) pid.
+Proof.
+intros. pose proof H as ri. unfold regs_identical in H.  unfold end_state_equals_asm_memsim. destruct i; simpl; try unfold Asm.goto_label; try unfold goto_label; try unfold Asm.eval_testcond; try unfold eval_testcond; try unfold Asm.exec_load; try unfold exec_load; try unfold Asm.exec_store; try unfold exec_store; try unfold Mem.loadv; try unfold eval_addressing; try unfold Asm.eval_addressing; unfold Asm.compare_long; unfold compare_long; unfold Asm.compare_int; unfold compare_int; unfold Asm.ir0w; unfold ir0w; unfold Asm.ir0x; unfold ir0x; destruct matches; try split; try unfold nextinstr; try apply set_method_sem_eq_form3; try unfold regs_identical; try intro; sem_eq_solver.
+Unset Printing Notations.
+Qed.
+
+
+      
+
+(** Classification functions for processor registers (used in Asmgenproof). *)
+
+Definition data_preg (r: preg) : bool :=
+  match r with
+  | IR X16 => false
+  | IR X30 => false
+  | IR _ => true
+  | FR _ => true
+  | CR _ => false
+  | SP => true
+  | PC => false
+  end.
+
+
+Lemma outcome_equality: forall (rs1 rs2: regset)(m1 m2: mem),  Next rs1 m1 = Next rs2 m2 -> rs1 = rs2 /\ m1 = m2. 
+    Proof. intros. inversion H. split; reflexivity. Qed.
+
+Lemma inverse_outcome_equality: forall (rs1 rs2: regset)(m1 m2: mem), rs1 = rs2 /\ m1 = m2 -> Next rs1 m1 = Next rs2 m2.
+Proof. intros. destruct H. rewrite H. rewrite H0. reflexivity. Qed.
+
+(* need some way of abstracting 
+for a given instruction if an argument is a data source/data sink*)
+Inductive data_resource: Type :=
+    | SingleReg: preg -> data_resource
+    | SingleMemAddr: memory_chunk -> val -> data_resource.
+Definition data_res_eq (d1 d2: data_resource): Prop :=
+    match d1, d2 with
+    | SingleReg r1, SingleReg r2 => r1 = r2
+    | SingleMemAddr c1 a1, SingleMemAddr c2 a2 => c1 = c2 /\ a1 = a2
+    | _, _ => False
+    end.
+
+Definition iregz_same_resource (dr: data_resource) (r: ireg0) : Prop :=
+    match r with 
+    | RR0 r1 => data_res_eq dr (SingleReg r1) 
+    | XZR => False
+    end.
+    
+    
+Remark data_res_isomorphism: forall r, data_res_eq r r.
+Proof.
+    intros. destruct r. unfold data_res_eq. reflexivity. unfold data_res_eq. split; reflexivity. 
+Qed.
+
+Lemma symb_data_eq: forall (x y: data_resource), {x=y} + {x<>y}.
+Proof. decide equality. apply preg_eq. apply Val.eq. apply AST.chunk_eq.
+Qed.
+
+(* TODO Check if data resource d is an input for address a. Requires checking the regs of A*)
+Definition data_address_src(a: addressing) (d: data_resource) : Prop := 
+   match a with
+   | ADimm base n => data_res_eq d (SingleReg (preg_of_iregsp base))
+   | ADreg base r => data_res_eq d (SingleReg (preg_of_iregsp base)) \/  data_res_eq d (SingleReg r) 
+   | ADlsl base r n => data_res_eq d  ( SingleReg (preg_of_iregsp base)) \/ data_res_eq d (SingleReg r) 
+   | ADsxt base r n => data_res_eq d (SingleReg (preg_of_iregsp base)) \/ data_res_eq d (SingleReg r) 
+   | ADuxt base r n => data_res_eq d (SingleReg (preg_of_iregsp base)) \/ data_res_eq d (SingleReg r) 
+   | ADadr base id ofs => data_res_eq d (SingleReg (preg_of_iregsp base))
+   | ADpostincr base n => True (* not modeled in CompCert*) 
+   end.
+
+
+
+ (* Check if data resource d is overwritten by a. Requires checking the evaluated expr*)
+ Definition data_address_sink (a: addressing) (d: data_resource) (g: genv) (r: regset): Prop := 
+    match d with
+    | SingleMemAddr _ val => eval_addressing g a r = val
+    | _ => False
+    end.
+
+(* TODO: change all instances of NoResource to false? kinda based*)
+
+(* Get a proposition representing if an instruction has a dependency on dr*)
+Definition data_source(i: instruction) (dr: data_resource): Prop := 
+    match i with 
+   (* Jump to*)
+   | Pb lbl => False                                                    (**r branch *)
+   | Pbc c lbl  => data_res_eq dr (SingleReg (CR CZ))                                    (**r conditional branch *)
+   | Pbl id sg => data_res_eq dr (SingleReg PC)                                  (**r jump to function and link *)
+   | Pbs id sg => False                              (**r jump to function *)
+   | Pblr r sg  => data_res_eq dr (SingleReg PC)                                   (**r indirect jump and link *)
+   | Pbr r sg   => data_res_eq dr (SingleReg PC)                                   (**r indirect jump *)
+   | Pret r => False                                              (**r return *)
+   | Pcbnz sz r lbl    => data_res_eq dr (SingleReg r)                      (**r branch if not zero *)
+   | Pcbz sz r lbl => data_res_eq dr (SingleReg r)                         (**r branch if zero *)
+   | Ptbnz sz r n lbl   => data_res_eq dr (SingleReg r)               (**r branch if bit n is not zero *)
+   | Ptbz sz r n lbl => data_res_eq dr (SingleReg r)                  (**r branch if bit n is zero *)
+   (** Memory loads and stores *)
+   | Pldrw rd a => data_address_src a dr                             (**r load int32 *)
+   | Pldrw_a rd a => data_address_src a dr                                 (**r load int32 as any32 *)
+   | Pldrx rd a => data_address_src a dr                                  (**r load int64 *)
+   | Pldrx_a rd a => data_address_src a dr                                 (**r load int64 as any64 *)
+   | Pldrb sz rd a => data_address_src a dr                         (**r load int8, zero-extend *)
+   | Pldrsb sz rd a => data_address_src a dr                        (**r load int8, sign-extend *)
+   | Pldrh sz rd a => data_address_src a dr                        (**r load int16, zero-extend *)
+   | Pldrsh sz rd a => data_address_src a dr                        (**r load int16, sign-extend *)
+   | Pldrzw rd a  => data_address_src a dr                                  (**r load int32, zero-extend to int64 *)
+   | Pldrsw rd a => data_res_eq dr (SingleReg rd)                                 (**r load int32, sign-extend to int64 *)
+   | Pldp rd1 rd2 a => data_res_eq dr (SingleReg rd1) \/ data_res_eq dr (SingleReg rd2)                               (**r load two int64 *)
+   (** Stores *)
+   | Pstrw rs a => data_res_eq dr (SingleReg rs)                               (**r store int32 *)
+   | Pstrw_a rs a => data_res_eq dr (SingleReg rs)                                     (**r store int32 as any32 *)
+   | Pstrx rs a => data_res_eq dr (SingleReg rs)                                      (**r store int64 *)
+   | Pstrx_a rs a => data_res_eq dr (SingleReg rs)                                   (**r store int64 as any64 *)
+   | Pstrb rs a => data_res_eq dr (SingleReg rs)                                    (**r store int8 *)
+   | Pstrh rs a => data_res_eq dr (SingleReg rs)                                    (**r store int16 *)
+   | Pstp rs1 rs2 a => data_res_eq dr (SingleReg rs1)  \/ data_res_eq dr (SingleReg rs2)                               (**r store two int64 *)
+   (** Integer arithmetic, immediate *)
+   | Paddimm sz rd r1 n  => data_res_eq dr (SingleReg (preg_of_iregsp r1))            (**r addition *)
+   | Psubimm sz rd r1 n => data_res_eq dr (SingleReg (preg_of_iregsp r1))               (**r subtraction *)
+   | Pcmpimm sz r1 n => data_res_eq dr (SingleReg r1)                             (**r compare *)
+   | Pcmnimm sz r1 n => data_res_eq dr (SingleReg r1)                              (**r compare negative *)
+   (** Move integer register *)
+   | Pmov rd r1 => data_res_eq dr (SingleReg (preg_of_iregsp r1)) 
+   (** Logical, immediate *)
+   | Pandimm sz rd r1 n => iregz_same_resource dr r1                 (**r and *)
+   | Peorimm sz rd r1 n => iregz_same_resource dr r1                  (**r xor *)
+   | Porrimm sz rd r1 n => iregz_same_resource dr r1                  (**r or *)
+   | Ptstimm sz r1 n => data_res_eq dr (SingleReg r1)                             (**r and, then set flags *)
+   (** Move wide immediate *)
+   | Pmovz sz rd n pos  => False                (**r move [n << pos] to [rd] *)
+   | Pmovn sz rd n pos  => False                (**r move [NOT(n << pos)] to [rd] *)
+   | Pmovk sz rd n pos  => False                (**r insert 16 bits of [n] at [pos] in rd *)
+   (** PC-relative addressing *)
+   | Padrp rd id ofs => False                   (**r set [rd] to high address of [id + ofs] *)
+   | Paddadr rd r1 id ofs => data_res_eq dr (SingleReg r1)             (**r add the low address of [id + ofs] *)
+   (** Bit-field operations *)
+   | Psbfiz sz rd r1 r s => data_res_eq dr (SingleReg r1)           (**r sign extend and shift left *)
+   | Psbfx sz rd r1 r s => data_res_eq dr (SingleReg r1)           (**r shift right and sign extend *)
+   | Pubfiz sz rd r1 r s => data_res_eq dr (SingleReg r1)           (**r zero extend and shift left *)
+   | Pubfx sz rd r1 r s => data_res_eq dr (SingleReg r1)           (**r shift right and zero extend *)
+   (** Integer arithmetic, shifted register *)
+   | Padd sz rd r1 r2 s => iregz_same_resource dr r1 \/ data_res_eq dr (SingleReg r2)    (**r addition *)
+   | Psub sz rd r1 r2 s => iregz_same_resource dr r1 \/ data_res_eq dr (SingleReg r2)   (**r subtraction *)
+   | Pcmp sz r1 r2 s => iregz_same_resource dr r1 \/ data_res_eq dr (SingleReg r2)              (**r compare *)
+   | Pcmn sz r1 r2 s => iregz_same_resource dr r1 \/ data_res_eq dr (SingleReg r2)              (**r compare negative *)
+   (** Integer arithmetic, extending register *)
+   | Paddext rd r1 r2 x => data_res_eq dr (SingleReg r1) \/ data_res_eq dr (SingleReg r2)        (**r int64-int32 add *)
+   | Psubext rd r1 r2 x => data_res_eq dr (SingleReg r1) \/ data_res_eq dr (SingleReg r2)        (**r int64-int32 sub *)
+   | Pcmpext r1 r2 x => data_res_eq dr (SingleReg r1) \/ data_res_eq dr (SingleReg r2)                     (**r int64-int32 cmp *)
+   | Pcmnext r1 r2 x => data_res_eq dr (SingleReg r1) \/ data_res_eq dr (SingleReg r2)                       (**r int64-int32 cmn *)
+   (** Logical, shifted register *)
+   | Pand sz rd r1 r2 s => iregz_same_resource dr r1 \/ data_res_eq dr (SingleReg r2)   (**r and *)
+   | Pbic sz rd r1 r2 s => iregz_same_resource dr r1 \/ data_res_eq dr (SingleReg r2)   (**r and-not *)
+   | Peon sz rd r1 r2 s => iregz_same_resource dr r1 \/ data_res_eq dr (SingleReg r2)   (**r xor-not *)
+   | Peor sz rd r1 r2 s => iregz_same_resource dr r1 \/ data_res_eq dr (SingleReg r2)   (**r xor *)
+   | Porr sz rd r1 r2 s => iregz_same_resource dr r1 \/ data_res_eq dr (SingleReg r2)   (**r or *)
+   | Porn sz rd r1 r2 s => iregz_same_resource dr r1 \/ data_res_eq dr (SingleReg r2)   (**r or-not *)
+   | Ptst sz r1 r2 s => iregz_same_resource dr r1 \/ data_res_eq dr (SingleReg r2)                (**r and, then set flags *)
+   (** Variable shifts *)
+   | Pasrv sz rd r1 r2 => data_res_eq dr (SingleReg r1) \/ data_res_eq dr (SingleReg r2)                         (**r arithmetic right shift *)
+   | Plslv sz rd r1 r2 => data_res_eq dr (SingleReg r1) \/ data_res_eq dr (SingleReg r2)                         (**r left shift *)
+   | Plsrv sz rd r1 r2 => data_res_eq dr (SingleReg r1) \/ data_res_eq dr (SingleReg r2)                         (**r logical right shift *)
+   | Prorv sz rd r1 r2 => data_res_eq dr (SingleReg r1) \/ data_res_eq dr (SingleReg r2)                        (**r rotate right *)
+   (** Bit operations *)
+   | Pcls sz rd r1 => data_res_eq dr (SingleReg r1)                                    (**r count leading sign bits *)
+   | Pclz sz rd r1 => data_res_eq dr (SingleReg r1)                                     (**r count leading zero bits *)
+   | Prev sz rd r1 => data_res_eq dr (SingleReg r1)                                    (**r reverse bytes *)
+   | Prev16 sz rd r1 => data_res_eq dr (SingleReg r1)                                   (**r reverse bytes in each 16-bit word *)
+   | Prbit sz rd r1  => data_res_eq dr (SingleReg r1)                                   (**r reverse bits *)
+   (** Conditional data processing *)
+   | Pcsel rd r1 r2 c  => data_res_eq dr (SingleReg r1)  \/ data_res_eq dr (SingleReg r2)                      (**r int conditional move *)
+    (*TODO: anything more to handle conditions?*)
+   | Pcset rd c => False                               (**r set to 1/0 if cond is true/false *)
+   (*
+   | Pcsetm rd c                                   (**r set to -1/0 if cond is true/false *)
+   *)
+   (** Integer multiply/divide *)
+   | Pmadd sz rd r1 r2 r3 =>  data_res_eq dr (SingleReg r1) \/ data_res_eq dr (SingleReg r2) \/ iregz_same_resource dr r3              (**r multiply-add *)
+   | Pmsub sz rd r1 r2 r3 => data_res_eq dr (SingleReg r1) \/ data_res_eq dr (SingleReg r2) \/ iregz_same_resource dr r3            (**r multiply-sub *)
+   | Psmulh rd r1 r2 => data_res_eq dr (SingleReg r1) \/ data_res_eq dr (SingleReg r2)                                   (**r signed multiply high *)
+   | Pumulh rd r1 r2 => data_res_eq dr (SingleReg r1) \/ data_res_eq dr (SingleReg r2)                                   (**r unsigned multiply high *)
+   | Psdiv sz rd r1 r2 => data_res_eq dr (SingleReg r1) \/ data_res_eq dr (SingleReg r2)                       (**r signed division *)
+   | Pudiv sz rd r1 r2 => data_res_eq dr (SingleReg r1) \/ data_res_eq dr (SingleReg r2)                       (**r unsigned division *)
+   (** Floating-point loads and stores *)
+   | Pldrs rd a => data_address_src a dr                                   (**r load float32 (single precision) *)
+   | Pldrd rd a => data_address_src a dr                                  (**r load float64 (double precision) *)
+   | Pldrd_a rd a => data_address_src a dr                                (**r load float64 as any64 *)
+   | Pstrs rs a => data_res_eq dr (SingleReg rs)                                   (**r store float32 *)
+   | Pstrd rs a => data_res_eq dr (SingleReg rs)                                   (**r store float64 *)
+   | Pstrd_a rs a => data_res_eq dr (SingleReg rs)                                (**r store float64 as any64 *)
+   (** Floating-point move *)
+   | Pfmov rd r1 => data_res_eq dr (SingleReg r1) 
+   | Pfmovimms rd f  => False                                (**r load float32 constant *)
+   | Pfmovimmd rd f  => False                                  (**r load float64 constant *)
+   | Pfmovi fsz rd r1 => iregz_same_resource dr r1                         (**r copy int reg to FP reg *)
+   (** Floating-point conversions *)
+   | Pfcvtds rd r1  => data_res_eq dr (SingleReg r1)                                            (**r convert float32 to float64 *)
+   | Pfcvtsd rd r1  => data_res_eq dr (SingleReg r1)                                           (**r convert float64 to float32 *)
+   | Pfcvtzs isz fsz rd r1 => data_res_eq dr (SingleReg r1)            (**r convert float to signed int *)
+   | Pfcvtzu isz fsz rd r1 => data_res_eq dr (SingleReg r1)           (**r convert float to unsigned int *)
+   | Pscvtf fsz isz rd r1 => data_res_eq dr (SingleReg r1)             (**r convert signed int to float *)
+   | Pucvtf fsz isz rd r1 => data_res_eq dr (SingleReg r1)            (**r convert unsigned int to float *)
+   (** Floating-point arithmetic *)
+   | Pfabs sz rd r1 => data_res_eq dr (SingleReg r1)                                    (**r absolute value *)
+   | Pfneg sz rd r1 => data_res_eq dr (SingleReg r1)                                    (**r negation *)
+   | Pfsqrt sz rd r1 => data_res_eq dr (SingleReg r1)                                   (**r square root *)
+   | Pfadd sz rd r1 r2 => data_res_eq dr (SingleReg r1) \/ data_res_eq dr (SingleReg r2)                                 (**r addition *)
+   | Pfdiv sz rd r1 r2  => data_res_eq dr (SingleReg r1) \/ data_res_eq dr (SingleReg r2)                               (**r division *)
+   | Pfmul sz rd r1 r2  => data_res_eq dr (SingleReg r1)  \/ data_res_eq dr (SingleReg r2)                             (**r multiplication *)
+   | Pfnmul sz rd r1 r2 => data_res_eq dr (SingleReg r1)  \/ data_res_eq dr (SingleReg r2)                             (**r multiply-negate *)
+   | Pfsub sz rd r1 r2 => data_res_eq dr (SingleReg r1)   \/ data_res_eq dr (SingleReg r2)                              (**r subtraction *)
+   | Pfmadd sz rd r1 r2 r3 => data_res_eq dr (SingleReg r1) \/ data_res_eq dr (SingleReg r2) \/ data_res_eq dr (SingleReg r3)                            (**r [rd = r3 + r1 * r2] *)
+   | Pfmsub sz rd r1 r2 r3 => data_res_eq dr (SingleReg r1) \/ data_res_eq dr (SingleReg r2) \/ data_res_eq dr (SingleReg r3)                            (**r [rd = r3 - r1 * r2] *)
+   | Pfnmadd sz rd r1 r2 r3 => data_res_eq dr (SingleReg r1) \/ data_res_eq dr (SingleReg r2) \/ data_res_eq dr (SingleReg r3)                           (**r [rd = - r3 - r1 * r2] *)
+   | Pfnmsub sz rd r1 r2 r3 => data_res_eq dr (SingleReg r1) \/ data_res_eq dr (SingleReg r2) \/ data_res_eq dr (SingleReg r3)                           (**r [rd = - r3 + r1 * r2] *)
+   | Pfmax sz rd r1 r2 => data_res_eq dr (SingleReg r1) \/ data_res_eq dr (SingleReg r2)                                (**r maximum *)
+   | Pfmin sz rd r1 r2 => data_res_eq dr (SingleReg r1) \/ data_res_eq dr (SingleReg r2)                               (**r minimum *)
+   (** Floating-point comparison *)
+   | Pfcmp sz r1 r2 => data_res_eq dr (SingleReg r1) \/ data_res_eq dr (SingleReg r2)                                   (**r compare [r1] and [r2] *)
+   | Pfcmp0 sz r1 => data_res_eq dr (SingleReg r1)                                      (**r compare [r1] and [+0.0] *)
+   (** Floating-point conditional select *)
+   (*TODO: figure out cond*)
+   | Pfsel rd r1 r2 cond => data_res_eq dr (SingleReg r1) \/ data_res_eq dr (SingleReg r2)
+   (** Pseudo-instructions *)
+   | Pallocframe sz linkofs => False                              (**r allocate new stack frame *)
+   | Pfreeframe sz linkofs => False                               (**r deallocate stack frame and restore previous frame *)
+   | Plabel lbl => False                                                (**r define a code label *)
+   | Ploadsymbol rd id => False                                 (**r load the address of [id] *)
+   | Pcvtsw2x rd r1 => data_res_eq dr (SingleReg r1)                                 (**r sign-extend 32-bit int to 64-bit *)
+   | Pcvtuw2x rd r1 => data_res_eq dr (SingleReg r1)                                  (**r zero-extend 32-bit int to 64-bit *)
+   | Pcvtx2w rd => data_res_eq dr (SingleReg rd)                                                 (**r retype a 64-bit int as a 32-bit int *)
+   | Pbtbl r1 tbl  => False                              (**r N-way branch through a jump table *)
+   | Pbuiltin ef args res => False   (**r built-in function (pseudo) *)
+   | Pnop => False                                                             (**r no operation *)
+   | Pcfi_adjust ofs => False                                           (**r .cfi_adjust debug directive *)
+   | Pcfi_rel_offset ofs  => False                                       (**r .cfi_rel_offset debug directive *)
+   | Pincpc => data_res_eq dr (SingleReg PC) 
+    end.
+
+Definition data_sink(i: instruction) (dr: data_resource) (g: genv) (ers: regset): Prop := 
+    match i with
+    (*actual*)
+    (* Jump to*)
+    | Pb lbl pid => data_res_eq dr (SingleReg PC)                                                    (**r branch *)
+    | Pbc c lbl  pid => data_res_eq dr (SingleReg PC)                                    (**r conditional branch *)
+    | Pbl id sg pid => data_res_eq dr (SingleReg PC) \/ data_res_eq dr (SingleReg RA)                                    (**r jump to function and link *)
+    | Pbs id sg pid => data_res_eq dr (SingleReg PC)                                   (**r jump to function *)
+    | Pblr r sg  pid => data_res_eq dr (SingleReg PC)  \/ data_res_eq dr (SingleReg RA)                                (**r indirect jump and link *)
+    | Pbr r sg   pid => data_res_eq dr (SingleReg PC)                                   (**r indirect jump *)
+    | Pret r pid => data_res_eq dr (SingleReg PC)                                                     (**r return *)
+    | Pcbnz sz r lbl    pid => data_res_eq dr (SingleReg PC)                       (**r branch if not zero *)
+    | Pcbz sz r lbl pid => data_res_eq dr (SingleReg PC)                           (**r branch if zero *)
+    | Ptbnz sz r n lbl   pid => data_res_eq dr (SingleReg PC)               (**r branch if bit n is not zero *)
+    | Ptbz sz r n lbl pid => data_res_eq dr (SingleReg PC)                  (**r branch if bit n is zero *)
+    (** Memory loads and stores *)
+    | Pldrw rd a pid => data_res_eq dr (SingleReg rd)                                 (**r load int32 *)
+    | Pldrw_a rd a pid => data_res_eq dr (SingleReg rd)                                (**r load int32 as any32 *)
+    | Pldrx rd a pid => data_res_eq dr (SingleReg rd)                                 (**r load int64 *)
+    | Pldrx_a rd a pid => data_res_eq dr (SingleReg rd)                                (**r load int64 as any64 *)
+    | Pldrb sz rd a pid => data_res_eq dr (SingleReg (preg_of_iregsp rd))                        (**r load int8, zero-extend *)
+    | Pldrsb sz rd a pid => data_res_eq dr (SingleReg (preg_of_iregsp rd))                      (**r load int8, sign-extend *)
+    | Pldrh sz rd a pid => data_res_eq dr (SingleReg (preg_of_iregsp rd))                       (**r load int16, zero-extend *)
+    | Pldrsh sz rd a pid => data_res_eq dr (SingleReg (preg_of_iregsp rd))                      (**r load int16, sign-extend *)
+    | Pldrzw rd a  pid => data_res_eq dr (SingleReg rd)                                 (**r load int32, zero-extend to int64 *)
+    | Pldrsw rd a pid => data_res_eq dr (SingleReg rd)                                 (**r load int32, sign-extend to int64 *)
+    | Pldp rd1 rd2 a pid => data_res_eq dr (SingleReg rd1) \/ data_res_eq dr (SingleReg rd2)                               (**r load two int64 *)
+    (*TODO: check this works *)
+    (* explanation: check if r is a memory address and, if so, check if a stores in r. Can check by evaluating both??? *)
+    | Pstrw rs a pid => data_address_sink a dr g ers                                 (**r store int32 *)
+    | Pstrw_a rs a pid => data_address_sink a dr g ers                                  (**r store int32 as any32 *)
+    | Pstrx rs a pid => data_address_sink a dr g ers                                    (**r store int64 *)
+    | Pstrx_a rs a pid => data_address_sink a dr g ers                                  (**r store int64 as any64 *)
+    | Pstrb rs a pid => data_address_sink a dr g ers                                   (**r store int8 *)
+    | Pstrh rs a pid => data_address_sink a dr g ers                                   (**r store int16 *)
+    | Pstp rs1 rs2 a pid => data_address_sink a dr g ers                                (**r store two int64 *)
+    (** Integer arithmetic, immediate *)
+    | Paddimm sz rd r1 n  pid => data_res_eq dr (SingleReg (preg_of_iregsp rd))            (**r addition *)
+    | Psubimm sz rd r1 n pid => data_res_eq dr (SingleReg (preg_of_iregsp rd))               (**r subtraction *)
+    | Pcmpimm sz r1 n pid => data_res_eq dr (SingleReg (CR CZ))                             (**r compare *)
+    | Pcmnimm sz r1 n pid => data_res_eq dr (SingleReg (CR CZ))                              (**r compare negative *)
+    (** Move integer register *)
+    | Pmov rd r1 pid => data_res_eq dr (SingleReg (preg_of_iregsp rd)) 
+    (** Logical, immediate *)
+    | Pandimm sz rd r1 n pid => data_res_eq dr (SingleReg rd)                  (**r and *)
+    | Peorimm sz rd r1 n pid => data_res_eq dr (SingleReg rd)                  (**r xor *)
+    | Porrimm sz rd r1 n pid => data_res_eq dr (SingleReg (preg_of_iregsp rd))                  (**r or *)
+    | Ptstimm sz r1 n pid => data_res_eq dr (SingleReg (CR CZ))                             (**r and, then set flags *)
+    (** Move wide immediate *)
+    | Pmovz sz rd n pos  pid => data_res_eq dr (SingleReg rd)                     (**r move [n << pos] to [rd] *)
+    | Pmovn sz rd n pos  pid => data_res_eq dr (SingleReg rd)                     (**r move [NOT(n << pos)] to [rd] *)
+    | Pmovk sz rd n pos  pid => data_res_eq dr (SingleReg rd)                     (**r insert 16 bits of [n] at [pos] in rd *)
+    (** PC-relative addressing *)
+    | Padrp rd id ofs pid => data_res_eq dr (SingleReg rd)                        (**r set [rd] to high address of [id + ofs] *)
+    | Paddadr rd r1 id ofs pid => data_res_eq dr (SingleReg rd)             (**r add the low address of [id + ofs] *)
+    (** Bit-field operations *)
+    | Psbfiz sz rd r1 r s pid => data_res_eq dr (SingleReg rd)           (**r sign extend and shift left *)
+    | Psbfx sz rd r1 r s pid => data_res_eq dr (SingleReg rd)           (**r shift right and sign extend *)
+    | Pubfiz sz rd r1 r s pid => data_res_eq dr (SingleReg rd)           (**r zero extend and shift left *)
+    | Pubfx sz rd r1 r s pid => data_res_eq dr (SingleReg rd)           (**r shift right and zero extend *)
+    (** Integer arithmetic, shifted register *)
+    | Padd sz rd r1 r2 s pid => data_res_eq dr (SingleReg rd)    (**r addition *)
+    | Psub sz rd r1 r2 s pid => data_res_eq dr (SingleReg rd)   (**r subtraction *)
+    | Pcmp sz r1 r2 s pid => data_res_eq dr (SingleReg (CR CZ))              (**r compare *)
+    | Pcmn sz r1 r2 s pid => data_res_eq dr (SingleReg (CR CZ))              (**r compare negative *)
+    (** Integer arithmetic, extending register *)
+    | Paddext rd r1 r2 x pid => data_res_eq dr (SingleReg (preg_of_iregsp rd))        (**r int64-int32 add *)
+    | Psubext rd r1 r2 x pid => data_res_eq dr (SingleReg (preg_of_iregsp rd))        (**r int64-int32 sub *)
+    | Pcmpext r1 r2 x pid => data_res_eq dr (SingleReg (CR CZ))                      (**r int64-int32 cmp *)
+    | Pcmnext r1 r2 x pid => data_res_eq dr (SingleReg (CR CZ))                       (**r int64-int32 cmn *)
+    (** Logical, shifted register *)
+    | Pand sz rd r1 r2 s pid => data_res_eq dr (SingleReg rd)   (**r and *)
+    | Pbic sz rd r1 r2 s pid => data_res_eq dr (SingleReg rd)   (**r and-not *)
+    | Peon sz rd r1 r2 s pid => data_res_eq dr (SingleReg rd)   (**r xor-not *)
+    | Peor sz rd r1 r2 s pid => data_res_eq dr (SingleReg rd)   (**r xor *)
+    | Porr sz rd r1 r2 s pid => data_res_eq dr (SingleReg rd)   (**r or *)
+    | Porn sz rd r1 r2 s pid => data_res_eq dr (SingleReg rd)   (**r or-not *)
+    | Ptst sz r1 r2 s pid => data_res_eq dr (SingleReg (CR CZ))                (**r and, then set flags *)
+    (** Variable shifts *)
+    | Pasrv sz rd r1 r2 pid => data_res_eq dr (SingleReg rd)                         (**r arithmetic right shift *)
+    | Plslv sz rd r1 r2 pid => data_res_eq dr (SingleReg rd)                         (**r left shift *)
+    | Plsrv sz rd r1 r2 pid => data_res_eq dr (SingleReg rd)                         (**r logical right shift *)
+    | Prorv sz rd r1 r2 pid => data_res_eq dr (SingleReg rd)                        (**r rotate right *)
+    (** Bit operations *)
+    | Pcls sz rd r1 pid => data_res_eq dr (SingleReg rd)                                     (**r count leading sign bits *)
+    | Pclz sz rd r1 pid => data_res_eq dr (SingleReg rd)                                     (**r count leading zero bits *)
+    | Prev sz rd r1 pid => data_res_eq dr (SingleReg rd)                                    (**r reverse bytes *)
+    | Prev16 sz rd r1 pid => data_res_eq dr (SingleReg rd)                                   (**r reverse bytes in each 16-bit word *)
+    | Prbit sz rd r1  pid => data_res_eq dr (SingleReg rd)                                   (**r reverse bits *)
+    (** Conditional data processing *)
+    | Pcsel rd r1 r2 c  pid => data_res_eq dr (SingleReg rd)                     (**r int conditional move *)
+    | Pcset rd c pid => data_res_eq dr (SingleReg rd)                                     (**r set to 1/0 if cond is true/false *)
+    (*
+    | Pcsetm rd c                                   (**r set to -1/0 if cond is true/false *)
+    *)
+    (** Integer multiply/divide *)
+    | Pmadd sz rd r1 r2 r3 pid => data_res_eq dr (SingleReg rd)             (**r multiply-add *)
+    | Pmsub sz rd r1 r2 r3 pid => data_res_eq dr (SingleReg rd)             (**r multiply-sub *)
+    | Psmulh rd r1 r2 pid => data_res_eq dr (SingleReg rd)                                   (**r signed multiply high *)
+    | Pumulh rd r1 r2 pid => data_res_eq dr (SingleReg rd)                                    (**r unsigned multiply high *)
+    | Psdiv sz rd r1 r2 pid => data_res_eq dr (SingleReg rd)                        (**r signed division *)
+    | Pudiv sz rd r1 r2 pid => data_res_eq dr (SingleReg rd)                        (**r unsigned division *)
+    (** Floating-point loads and stores *)
+    | Pldrs rd a pid => data_res_eq dr (SingleReg rd)                                   (**r load float32 (single precision) *)
+    | Pldrd rd a pid => data_res_eq dr (SingleReg rd)                                  (**r load float64 (double precision) *)
+    | Pldrd_a rd a pid => data_res_eq dr (SingleReg rd)                                (**r load float64 as any64 *)
+    | Pstrs rs a pid => data_address_sink a dr g ers                                   (**r store float32 *)
+    | Pstrd rs a pid => data_address_sink a dr g ers                                   (**r store float64 *)
+    | Pstrd_a rs a pid => data_address_sink a dr g ers                                (**r store float64 as any64 *)
+    (** Floating-point move *)
+    | Pfmov rd r1 pid => data_res_eq dr (SingleReg rd) 
+    | Pfmovimms rd f  pid => data_res_eq dr (SingleReg rd)                                (**r load float32 constant *)
+    | Pfmovimmd rd f  pid => data_res_eq dr (SingleReg rd)                                  (**r load float64 constant *)
+    | Pfmovi fsz rd r1 pid => data_res_eq dr (SingleReg rd)                         (**r copy int reg to FP reg *)
+    (** Floating-point conversions *)
+    | Pfcvtds rd r1  pid => data_res_eq dr (SingleReg rd)                                            (**r convert float32 to float64 *)
+    | Pfcvtsd rd r1  pid => data_res_eq dr (SingleReg rd)                                           (**r convert float64 to float32 *)
+    | Pfcvtzs isz fsz rd r1 pid => data_res_eq dr (SingleReg rd)            (**r convert float to signed int *)
+    | Pfcvtzu isz fsz rd r1 pid => data_res_eq dr (SingleReg rd)           (**r convert float to unsigned int *)
+    | Pscvtf fsz isz rd r1 pid => data_res_eq dr (SingleReg rd)             (**r convert signed int to float *)
+    | Pucvtf fsz isz rd r1 pid => data_res_eq dr (SingleReg rd)            (**r convert unsigned int to float *)
+    (** Floating-point arithmetic *)
+    | Pfabs sz rd r1 pid => data_res_eq dr (SingleReg rd)                                    (**r absolute value *)
+    | Pfneg sz rd r1 pid => data_res_eq dr (SingleReg rd)                                    (**r negation *)
+    | Pfsqrt sz rd r1 pid => data_res_eq dr (SingleReg rd)                                   (**r square root *)
+    | Pfadd sz rd r1 r2 pid => data_res_eq dr (SingleReg rd)                                (**r addition *)
+    | Pfdiv sz rd r1 r2  pid => data_res_eq dr (SingleReg rd)                                (**r division *)
+    | Pfmul sz rd r1 r2  pid => data_res_eq dr (SingleReg rd)                               (**r multiplication *)
+    | Pfnmul sz rd r1 r2 pid => data_res_eq dr (SingleReg rd)                               (**r multiply-negate *)
+    | Pfsub sz rd r1 r2 pid => data_res_eq dr (SingleReg rd)                                 (**r subtraction *)
+    | Pfmadd sz rd r1 r2 r3 pid => data_res_eq dr (SingleReg rd)                             (**r [rd = r3 + r1 * r2] *)
+    | Pfmsub sz rd r1 r2 r3 pid => data_res_eq dr (SingleReg rd)                             (**r [rd = r3 - r1 * r2] *)
+    | Pfnmadd sz rd r1 r2 r3 pid => data_res_eq dr (SingleReg rd)                            (**r [rd = - r3 - r1 * r2] *)
+    | Pfnmsub sz rd r1 r2 r3 pid => data_res_eq dr (SingleReg rd)                           (**r [rd = - r3 + r1 * r2] *)
+    | Pfmax sz rd r1 r2 pid => data_res_eq dr (SingleReg rd)                                (**r maximum *)
+    | Pfmin sz rd r1 r2 pid => data_res_eq dr (SingleReg rd)                                (**r minimum *)
+    (** Floating-point comparison *)
+    | Pfcmp sz r1 r2 pid => data_res_eq dr (SingleReg (CR CZ))                                   (**r compare [r1] and [r2] *)
+    | Pfcmp0 sz r1 pid => data_res_eq dr (SingleReg (CR CZ))                                      (**r compare [r1] and [+0.0] *)
+    (** Floating-point conditional select *)
+    | Pfsel rd r1 r2 cond pid => data_res_eq dr (SingleReg rd) 
+    (** Pseudo-instructions *)
+    | Pallocframe sz linkofs pid => False                            (**r allocate new stack frame *)
+    | Pfreeframe sz linkofs pid => False                             (**r deallocate stack frame and restore previous frame *)
+    | Plabel lbl pid => False                                              (**r define a code label *)
+    | Ploadsymbol rd id pid => data_res_eq dr (SingleReg rd)                                (**r load the address of [id] *)
+    | Pcvtsw2x rd r1 pid => data_res_eq dr (SingleReg rd)                                    (**r sign-extend 32-bit int to 64-bit *)
+    | Pcvtuw2x rd r1 pid => data_res_eq dr (SingleReg rd)                                    (**r zero-extend 32-bit int to 64-bit *)
+    | Pcvtx2w rd pid => data_res_eq dr (SingleReg rd)                                                 (**r retype a 64-bit int as a 32-bit int *)
+    | Pbtbl r1 tbl  pid => False                            (**r N-way branch through a jump table *)
+    | Pbuiltin ef args res pid => False (**r built-in function (pseudo) *)
+    | Pnop pid => False                                                           (**r no operation *)
+    | Pcfi_adjust ofs pid => False                                         (**r .cfi_adjust debug directive *)
+    | Pcfi_rel_offset ofs  pid => False                                     (**r .cfi_rel_offset debug directive *)
+    | Pincpc pid => data_res_eq dr (SingleReg PC) 
+end.
+
+
+
+Definition data_dependence(i1 i2: instruction) g rs: Prop :=
+    (exists r, data_sink i1 r g rs /\ data_source i2 r) \/ (exists r, data_sink i2 r g rs /\ data_source i1 r) \/ (exists r, data_sink i2 r g rs /\ data_sink i1 r g rs).
+
+
+Remark not_or_and : forall A B : Prop, ~(A \/ B) -> ~A /\ ~B.
+Proof.
+  intros A B H. split.
+    - intro. apply H. left. assumption.
+    - intro. apply H. right. assumption.
+Qed.
+
+Remark not_or_or_and : forall A B C : Prop, ~(A \/ B \/ C) -> ~A /\ ~B /\ ~C.
+Proof.
+  intros A B C H. split; [|split].
+  - intro HA. apply H. left. assumption.
+  - intro HB. apply H. right. left. assumption.
+  - intro HC. apply H. right. right. assumption.
+Qed.
+
+Lemma hazard_elimination_identity: forall r1, ~(exists r2: data_resource, data_res_eq r2 r1 /\ True)  -> False.
+Proof. intros. apply H. exists r1. split. apply data_res_isomorphism. reflexivity. Qed.
+
+Lemma hazard_elimination: forall (d: data_resource), ~ (exists r : data_resource, data_res_eq r (d) /\ data_res_eq r (d)) -> False.
+Proof. intros. apply H. exists d. split; apply data_res_isomorphism. 
+Qed.
+
+
+ Remark regs_are_different_resources: forall r1 r2, ~
+ (exists r : data_resource, data_res_eq r (SingleReg r1) /\ data_res_eq r (SingleReg r2)) -> r1 <> r2.
+ Proof.
+ unfold not. intros. apply H. exists (SingleReg r1). 
+ split. try apply data_res_isomorphism. 
+rewrite <- H0; apply data_res_isomorphism.
+Qed.
+
+Remark resources_are_different_resources: forall r1 r2,  ~
+ (exists r : data_resource, data_res_eq r r1 /\ data_res_eq r r2) ->  r1 <> r2.
+ Proof.
+ unfold not. intros. apply H. exists r1. 
+ split. try apply data_res_isomorphism. auto. 
+  try (rewrite <- H0; apply data_res_isomorphism).
+Qed.
+
+Remark VInt_eq: forall i1 i2, Vint i1 = Vint i2 -> i1 = i2.
+Proof. intros. inv H. reflexivity. Qed.
+
+(* Theorem reorder: forall  g (f: function) (i1 i2: instruction)  (rs_i rs_t1 rs_t2 rs_f: regset)  (m_i m_t1 m_t2 m_f: mem), ~data_dependence i1 i2 g rs_i -> exec_instr g f i1 rs_i m_i = Next rs_t1 m_t1 -> exec_instr g f i2 rs_i m_i = Next rs_t2 m_t2 -> exec_instr g f i2 rs_t1 m_t1 = Next rs_f m_f -> exec_instr g f i1 rs_t2 m_t2 = Next rs_f m_f. *)
+(* Theorem reorder: forall g (f: function) (i1 i2: instruction) (rs_i: regset) (m_i: mem), ~data_dependence i1 i2 g rs_i -> i1 = exec_instr g f i2 (exec_instr g f i1 (Next rs_i m_i)) = exec_instr g f i1 (exec_instr g f i2 (Next rs_i m_i)). *)
+
+Ltac Super_Equalities :=
+  match goal with
+  | [ H_gso: ?a @ ?b <- (?a ?c) ?d = ?e |- _ ] =>
+    rewrite -> Pregmap.gso in H_gso; Super_Equalities
+  | [ H1: Vint ?a = Vint ?b, H2: Vint ?a = Vint ?c |- _ ] =>
+    rewrite H1 in H2; apply VInt_eq; Super_Equalities
+  | [ H1: ?a = ?b, H2: ?a = ?c |- _ ] =>
+      rewrite H1 in H2; inv H2; Super_Equalities
+  | [ H_destroy: ?a = ?b |- _] => subst a; Super_Equalities
+  | _ => idtac
+  end.
+
+
+Theorem reorder: forall g (f: function) arg11 arg12 (i2: instruction) (rs_i: regset) (m_i: mem), ~data_dependence (Pmov arg11 arg12) i2 g rs_i -> exec_instr g f i2  (exec_instr g f (Pmov arg11 arg12)  (Next rs_i m_i)) = exec_instr g f (Pmov arg11 arg12)  (exec_instr g f i2  (Next rs_i m_i)).
+Proof. intros. 
+(* Definition unwrapping*)
+unfold data_dependence in H. unfold data_sink, data_source in H. apply not_or_or_and in H; destruct H; destruct H0. destruct i2.
+(* unfold data_dependence in H. unfold data_sink, data_source in H. destruct i1. destruct i2; apply not_or_or_and in H; destruct H; destruct H0; *)
+(* Remove data hazards that hit the same singleton register (eg PC, CR)*)
+try (apply hazard_elimination in H1;  contradiction +  unfold not;  intros;  discriminate H2);
+try (apply hazard_elimination in H;  contradiction +  unfold not;  intros;  discriminate H2);
+try (apply hazard_elimination in H0;  contradiction +  unfold not;  intros;  discriminate H2);
+
+
+
+(* Remove data hazards that hit True - maybe WIP?*)
+try (apply hazard_elimination_identity in H; contradiction + unfold not; intros; discriminate H2);
+
+try (apply hazard_elimination_identity in H0; contradiction + unfold not; intros; discriminate H2);
+
+try (apply hazard_elimination_identity in H1; contradiction + unfold not; intros; discriminate H2); auto;
+
+auto;
+
+(*Prove data vals different*)
+(* apply regs_are_different_resources in H1 || clear H1; apply regs_are_different_resources in H0 || clear H0; apply regs_are_different_resources in H || clear H; *)
+try apply regs_are_different_resources; try apply regs_are_different_resources in H0; try apply regs_are_different_resources in H;  
+unfold exec_instr; unfold nextinstr; unfold goto_label; unfold eval_testcond; destruct matches; auto; 
+(* Changing the order will not change the end result (Stuck/Next)*)
+Super_Equalities; auto.
+
+(* 
+(*breakdown mov*)
+
+
+(* Expression should be in the form Next ... = Next...*)
+-apply inverse_outcome_equality; split. rewrite -> Pregmap.gso. rewrite -> Heqv in Heqv0. inversion Heqv0. apply Pregmap.gscsc. auto. auto. auto.
+- rewrite -> Pregmap.gso in Heqv0. rewrite -> Heqv0 in Heqv2. discriminate. assumption.
+
+
+(* 
+try (rewrite -> Pregmap.gso in Heqv; rewrite -> Heqv in Heqv0; try discriminate + assumption). Qed.
+
+
+(*breakdown goto*)
+unfold goto_label. destruct matches; rewrite -> Pregmap.gso in Heqv; try rewrite -> Heqv in Heqv0; try discriminate;
+try apply regs_are_different_resources in H1; try apply regs_are_different_resources in H0; try apply regs_are_different_resources in H; auto.
+
+apply inverse_outcome_equality. split. rewrite -> Pregmap.gso. inversion Heqv0. rewrite <- H3. apply Pregmap.gscsc. assumption. auto. reflexivity. 
+
+
+
+contradiction.
+destruct (label_pos lbl 0 (fn_code f)); try reflexivity.  try rewrite -> Pregmap.gso; try destruct (rs_i PC); try reflexivity; try (apply inverse_outcome_equality; rewrite -> Pregmap.gso; try split; try apply Pregmap.gscsc);
+
+
+(*breakdown testcond*)
+unfold eval_testcond.  destruct c;  try rewrite -> Pregmap.gso.
+
+
+(*breakdown exec_add*)
+
+(*breakdown exec_load*)
+
+
+auto.  try apply regs_are_different_resources in H1. apply regs_are_different_resources in H0. auto.
+inversion H0. unfold nextinstr. rewrite H2. reflexivity.
+unfold nextinstr. split. Unset Printing Notations.  rewrite -> Pregmap.gso.  rewrite -> Pregmap.gso. apply Pregmap.gscsc. assumption. auto. auto. reflexivity. Qed.
+
+apply regs_are_different_resources in H, H0, H1.
+(*solves Pmov*)
+unfold exec_instr. apply inverse_outcome_equality. unfold nextinstr. split. Unset Printing Notations.  rewrite -> Pregmap.gso.  rewrite -> Pregmap.gso. apply Pregmap.gscsc. assumption. auto. auto. reflexivity. Qed.  *)
+(* 
+ unfold exec_instr. unfold goto_label. unfold exec_load.
+  destruct (rs_i PC). destruct (label_pos lbl 0 (fn_code f)).
+ destruct (Mem.loadv Mint32 m (eval_addressing g a rs)).  inversion H2.
+ destruct (Mem.loadv Mint32 m_i (eval_addressing g a rs_i)). inversion H1. unfold nextinstr in H6, H8.
+ destruct (label_pos lbl 0 (fn_code f)). destruct (rs_i PC); try discriminate. inversion H0. unfold nextinstr. rewrite -> H8. 
+ 
+ destruct (rs_i @ rd <- v0 PC); try discriminate. contradiction. unfold eval_addressing in H1, H2. *)
+
+Qed.
